---
tags:
  - seminar
  - 2nd-semester
  - 2025-02-12
---
$$\begin{gather}
\mathbb{F}_{3} = \{ 0,1,2 \} = \{ 0,1,-1 \} \\
f(x) = x^{4} + x^{3}+ x = x(x^{3} + x^{2} + 1) \\
g(x) = x^{4} + x^{2} + x = x(x^{3} + x + 1) \\ 
f(0) = 0, \ f(1) = 0 \\
\frac{x^{3} + x^{2} + 1}{x-1} = x^{2} + 2x + 2 \implies \\
\implies f(x) = x(x-1)(x^{2}+2x+2) \\
\pi: \mathbb{F}_{3}[x] \overset{эпи}{\longrightarrow} \mathbb{F}_{3}[x] / (x^{2} - x - 1) = \mathbb{F}_{3}[\alpha] = \{ a + b\alpha \ | \ a , b \in \mathbb{F}_{3} \} \\
\pi
\end{gather}$$