---
aliases: 
tags:
  - practice
  - seminar
  - 2nd-semester
---

> Creation time: 10:45

## По поводу второй задачи

R

$$\begin{gather}
A = \begin{pmatrix}
\alpha & \beta \\
\dot{} & \dot{}
\end{pmatrix} = \alpha E + \beta B \\
\{ E, B \} - \text{ базис } \\
\text{ dim }_{\mathbb{F}_{p}} R = 2 \\

B^{2}  \in  R \\
B^{2} + ?B + ?E = 0 \\
deg \ f(x) = 2 \\
f(B) = 0 \\
R = \{ \alpha E + \beta B  \ | \  \alpha, \beta  \in  F_{p} \} \\
F_{p}[x] \underbrace{ \to }_{ \text{ эпиморф. }  }R \\
1 \to E \\
x \to B \\
f(x)  \to f(B) = 0 \\
F_{p}[x] / (f(x)) \underbrace{ \to }_{  \ \cong \   } R
\end{gather}$$


1
$$\begin{gather}
f(x) -\text{ неприводим } \implies R-\text{ поле }  \\
\text{ char } R = p \\
F_{p}  \ \cong \   \{ \alpha E  \ | \  \alpha  \in  F_{p} \}- \text{ простое подполе } 
\end{gather}$$



Обычный контекст:

$$\begin{gather}
\underbrace{ K \subset L }_{ \text{ поля }  }, L = K[\alpha]=K(\alpha) - \text{ простое расширение } \\
\alpha  \in  L, \alpha   \cancel{ \in  }  K
\end{gather}$$

$$\begin{gather}
\alpha - \text{ примитивный элемент } \\
|L| < \infty, K \subset L, \alpha  \cancel{ \in  } K \alpha  \in  L \\
<\alpha> = L^{*}  \setminus \{ 0 \}; \alpha - \text{ примитивный элемент }  \\
K(\alpha) = L 
\end{gather}$$



$$\begin{gather}
R = \mathbb{F}_{p} [B] \\
B - \text{ примитивный элемент }  \\
R^{*} = R \setminus \{ 0 \} \\
R^{*}  \ \cong \  \mathbb{Z}_{p^{2}-1}  \\
m_{B} (x)  \in  F_{p}[x] \\
1.\ \text{ Старший коэф. }  = 1 \\
2.\ m_{B}(B) = 0 - \text{ явл корнем} \\
3.\ \text{ Если }  h(B)=0, \text{ то }, h(x)  \in  (m_{B}(x))
\end{gather}$$

## 2

$$\begin{gather}
a) \ f(x) = (x-a)^{2}, a  \in  F_{p} \\
b) \ f(x) = (x-a)(x-b), a\neq b; a,b  \in  F_{p}
\end{gather}$$

$$\begin{gather}
R  \ \cong \  F_{p}[x] \diagup ((x-a)(x-b)) conf F_{p} [x] \diagup (x-a) \\
\oplus F_{p}[x]  \diagup (x-b)  \ \cong \  F_{p} \oplus F_{p} \\
R^{*}  \ \cong \  F_{p}^{*}  \times F_{p}^{*}  \\
\text{ Rad } R = \{  0 \}
\end{gather}$$

$$\begin{gather}
|R| = p^{2}
\end{gather}$$

$$\begin{gather}
\det A = 0 \\
t = \frac{\alpha}{\beta} \\
t_{1}, t_{2} - \text{ корни }  \\
I_{1}, I_{2} \\
R = \underbrace{ I_{1} }_{ R \cdot e_{1} } \oplus \underbrace{ I_{2}  }_{ R \cdot e_{2} }  \\
e_{1}^{2} = e_{1} \\
e_{2}^{2} = e_{2} \\
e_{1}e_{2} = 0 \\
e_{1} + e_{2} = E
\end{gather}$$


$$\begin{gather}
a) \\
t = \alpha / \beta \\
(t-c)^{2} = 0 \\
\det A = 0 \\
\frac{\alpha}{\beta } = c \implies \alpha = c\beta \\
 I = \text{ Rad R } \\
 R \ \ u  \in  \text{ Rad R } , u^{n} = 0 \\
 (1-u)^{-1} = 1 + u + \dots + u^{n-1} \\
 R^{*} = R \setminus \text{ Rad R } 
\end{gather}$$


## Сюжет Аня

$$\begin{gather}
\mathbb{F}_{7} \\
\begin{cases}
\gamma = - 2\beta  \\
\delta - \alpha = -3\beta \implies \delta = \alpha - 3\beta 
\end{cases} \\
\begin{pmatrix}
\alpha & \beta \\
\gamma & \delta
\end{pmatrix} = \begin{pmatrix}
\alpha & \beta \\
-2\beta & \alpha-3\beta
\end{pmatrix}= \alpha E + \beta B \\
 B = \begin{pmatrix}
0 & 1 \\
-2 & -3
\end{pmatrix} \\
B^{2} = \begin{pmatrix}
0 & 1 \\
-2 & -3
\end{pmatrix} \begin{pmatrix}
0 & 1 \\
-2 & -3
\end{pmatrix} = \begin{pmatrix}
-2 & -3 \\
-1 & 0
\end{pmatrix}  = \\ 
= -2E -3B
\end{gather}$$

$$\begin{gather}
B^{2} + 3B + 2E = 0 \\
\end{gather}$$

$$\begin{gather}
\mathbb{F}_{7}[x] \diagup (x^{2}+3x+2) \\
1 \to E \\
x \to B \\
x^{2} +3x + 2 \to 0 \\
\end{gather}$$

$$\begin{gather}
\det \begin{pmatrix}
\alpha & \beta \\
-2\beta & \alpha-3\beta
\end{pmatrix} = \\ 
= \alpha^{2} -3\alpha \beta + 2\beta^{2} = 0 \ \ t= \frac{\alpha}{\beta} \\
t^{2}-3t+2 = 0 \\
(t-1)(t-2)=0
\end{gather}$$

$$\begin{gather}
t=1 \\
\alpha = \beta \\
I_{1} = \{ \alpha(E+B)  \ | \  \alpha  \in  \mathbb{F}_{7} \} \\
(\alpha (E+B))^{2} = \alpha (E+B) \\
\alpha^{2}(E+B)^{2} = \alpha (E+B) \\
\alpha(E+B)^{2} = E + B \\
\alpha = - 1 \\
\implies -(-E-B) \text{ и есть идемпотент } 
\end{gather}$$

$$\begin{gather}
(E+B)^{2} = \begin{pmatrix}
-1 & -1 \\
2  & 2
\end{pmatrix} \\
e_{1} = -E-B \\
e_{2} = E-e_{1} = 2E +B = \begin{pmatrix}
1 & 1 \\
-2 & -2
\end{pmatrix} + \begin{pmatrix}
1 & 0 \\
0 & 1
\end{pmatrix} = \\ 
= \begin{pmatrix}
2 & 1 \\
-2 & -1
\end{pmatrix} \\
I_{2} = R \cdot e_{2} \\
R = I_{1} \oplus I_{2} = \underbrace{ Re_{1} }_{  \ \cong \ F_{7}  } \oplus Re_{2} \ \ \cong \ \\
F_{7} \oplus F_{7} \\
I_{1} = R \cdot e_{1}
\end{gather}$$

$$\begin{gather}
\implies R^{*}  \ \cong \  F_{7}^{*} \times F_{8}^{*}  \ \cong \  \mathbb{Z}_{6} \times \mathbb{Z}_{6}   
\end{gather}$$

$$\begin{gather}
\text{ Rad R}  = \{ 0 \}
\end{gather}$$


## Сюжет "Андрей"

$$\begin{gather}
F_{5} \\
\begin{pmatrix}
\alpha & \beta  \\
3\beta & \alpha + \beta
\end{pmatrix}= \alpha E + \beta \underbrace{ \begin{pmatrix}
0 & 1 \\
3 & 1
\end{pmatrix} }_{ B } \\
\begin{vmatrix}
\alpha & \beta \\
3\beta & \alpha+\beta
\end{vmatrix} = \alpha^{2} + \alpha\beta - 3\beta^{2} \\
t^{2} + t + 2 = 0 - \text{ неприводим  в}  F_{5} \\
t = \frac{\alpha}{\beta} \\

\end{gather}$$

$$\begin{gather}
R  \ \cong \  F_{5}[x] \diagup (x^{2}-x+2) \\
|R|=25 \\
R^{*} \ \cong \ \mathbb{Z}_{24} \\
\text{ dim } _{F_{5}} R=2 \\
\text{ B примит. элем. }  \\
m_{B}(x)=x^{2}-x+2 \\
\theta  \in  F_{5}[x] \diagup (x^{2}-x+2) \\
\theta^{2} - \theta +2 = 0 \\
\theta^{2} = \theta - 2\\
\theta ^{3} = \theta^{2} -2 \theta^{2} = \theta -2 -2 \theta = -\theta -2 \\
(\theta^{3})^{2} = (-\theta-2)=\theta^{2} +4\theta +4 = 5\theta+2=2 = \theta^{6} \\
\theta^{12} = 2^{2} = 4  \\
\theta^{24}=4^{2} (-1)^{2} = 1 
\end{gather}$$
$$\begin{gather}
\text{ Rad r }  =\{ 0 \} \\
R^{*} = <B>_{24}
\end{gather}$$




$$\begin{gather}

\end{gather}$$