---
tags:
  - seminar
  - 2nd-semester
  - 2024-10-09
---
$$\begin{gather}
A_{4} \lhd S_{4} - ?, \ V_{4} \lhd S_{4} - ? \\
\end{gather}$$

$H$ - нормальная, $H \neq \{ e \}$, $H < A_{4}$.
Пусть $\exists (ijk) \in H \implies \beta(ijk)\beta^{-1} = (\beta(i)\beta(j)\beta(k)) \in H \implies \forall (ijk) \in H \implies H = A_{4}$.
Пусть $\nexists (ijk) \in H, \ \exists (ij)(kl) \in H$, тогда $\beta(ij)(kl)\beta^{-1} = (\beta(i)\beta(j))(\beta(k)\beta(l)) \in H \ \forall \beta \in S_{4} \implies H = V_{4}$.

## Для $A_{4}$

1)

$$\begin{gather}
\exists (ijk) \in H \\
\beta = (ijl) \\
(ijl)(ijk)(ijl)^{-1} = (\beta(i)\beta(j)\beta(k)) = (jlk) \implies \\
\implies (abc) \in H \ \forall a,b,c \implies H = A_{4} \\
\end{gather}$$


2)

$$\begin{gather}
(ij)(kl) \in H, \ \nexists(abc) \in H \\
\beta = (ijl) \\
(ijl)(ij)(kl)(ijl)^{-1} = \beta(ij)(kl)\beta^{-1} = (\beta(i)\beta(j))(\beta(k)\beta(l)) = (jl)(ki) \in V_{4} \implies \\
\implies V_{4} < H \implies V_{4} = H
\end{gather}$$

## $Q_{8}$ - кватернионная группа

$$\begin{gather}
Q_{8} = \{ \pm 1, \pm i, \pm j, \pm k \} \\
i^{2} = j^{2} = k^{2} = ijk = -1 \\
ijk = -1 \\
ijk^{2} = -k \to -ij = -k \implies ij = k \\
ij = -ji \\
jk = -kj \\
ik = -ki \\
i^{-1} = -i \\
(-1)^{-1} = -1 \\
\{ \pm1 \} \lhd Q_{8} \\
Q_{8} / \{ \pm1 \} = \{ \{ \pm 1 \},\{ \pm i \},\{ \pm j \},\{ \pm k \} \}
\end{gather}$$

$$\begin{gather}
G / H = \{ gH \ | \ g \in G \} - \text{фактор-группа} \\
H \lhd G \implies G / H - \text{группа}
\end{gather}$$

$$\begin{gather}
\{ \pm i \}^{2} = i\{ \pm 1 \} \cdot j\{ \pm 1 \} = (-1) \{ \pm 1 \} = \{ \pm 1 \} \implies \\
\implies \mathrm{ord} \ \{ \pm i \} = \mathrm{ord} \  \{ \pm j \}= \mathrm{ord} \  \{ \pm k \}  = 2  \implies Q_{8} / \{ \pm 1 \} \cong V_{4} \\
\{ \pm i \} \cdot \{ \pm j \} = \{ \pm 1 \} i \cdot \{ \pm 1 \}j = \{ \pm 1 \} k = \{ \pm k \} \\
V_{4} = \{ e, (12)(34), (13)(24), (14)(23) \} \\
e \leftrightarrow \{ \pm 1 \} \\
(12)(34) \leftrightarrow \{ \pm i \} \\
(13)(24) \leftrightarrow \{ \pm j \} \\
(14)(23) \leftrightarrow \{ \pm k \}
\end{gather}$$

> [!important] Теорема о гомоморфизме
> $$\begin{gather}
> f : G \to F \\
> f(g_{1}g_{2}) = f(g_{1})f(g_{2}) \\
> \mathrm{Ker} \ f = f^{-1}(e) = \{ x \in G \ | \ f(x) = e \in F \} \\
> \mathrm{Im} \ f = f(G) \\
> G / \mathrm{Ker} \ f \cong \mathrm{Im} \ f \\
> \phi: G / \mathrm{Ker} \ f \overset{\cong }{\to} \mathrm{Im} \ f \\
> \phi (g\cdot \mathrm{Ker} \ f) := f(g)
\end{gather}$$

### Примеры

$$\begin{gather}
\mathbb{R}_{>0} = \{ r \in \mathbb{R} \ | \ r > 0 \} \\
\mathbb{R}_{>0}(\mathbb{R}_{>0}, \cdot, 1) \\
\mathbb{R}_{>0} < \mathbb{C}^{*} \\
\mathbb{R}_{>0} \lhd \mathbb{C}^{*} = \mathbb{C} \setminus \{ 0 \} \\
\mathbb{C}^{*} / \mathbb{R}_{>0} \cong S^{1} = \{ z \in \mathbb{C}^{*} \ | \ |z| = 1 \} \\
f : C^{*} \to S^{1} \\
f(z) = \frac{z}{|z|} \\
f(z_{1} \cdot z_{2}) = \frac{z_{1}z_{2}}{|z_{1}z_{2}|} = \frac{z_{1}}{|z_{1}|}\cdot \frac{z_{2}}{|z_{2}|} = f(z_{1}) \cdot f(z_{2}) - \text{гомоморфизм, сюрьекция} \\
\mathrm{Ker} \ f = \{ z \in \mathbb{C}^{*} \ | \  f(z) = 1 \} \iff \frac{z}{|z|} = 1 \implies z = |z|, z \neq 0 \implies z \in \mathbb{R}_{>0} \\
\mathrm{Im} \ f = S^{1} \\ 
\implies \mathbb{C}^{*} / \mathbb{R}_{>0} \cong S^{1}
\end{gather}$$

$$\begin{gather}
\phi: \mathbb{R}_{>0} \to \mathbb{R} \\
(\cdot, 1) \mapsto (+, 0) \\
\phi(x) = \ln x \implies \phi(x) - \text{биекция} \\
\phi(x_{1}x_{2}) = \ln(x_{1}x_{2}) = \ln x_{1} + \ln x_{2} = \phi(x_{1}) + \phi(x_{2}) \implies \\
\implies (\mathbb{R}_{>0}, \cdot, 1) \cong (\mathbb{R}, +, 0)
\end{gather}$$


## Дз 

1. Построить обратную биекцию и проверить на $\phi_{a}(x) = \log_{a}(x)$.
2. 
$$\begin{gather}
C_{n} = \sqrt[n]{ 1 } \lhd S^{1} \\
\text{Показать, что} \ S^{1} / C_{n}  \cong S^{1} 
\end{gather}$$
3. 
$$\mathbb{C}^{*} / S^{1} \cong  \mathbb{R}_{>0}$$