---
tags:
  - seminar
  - 2nd-semester
  - 2024-09-11
---
## Задача 1

$G: a^{2} = e, \ a^{-1}b^{2}a = b^{3}, \ b^{5}\overset{?}{=}e$

$$\begin{gather}
a^{-1}b^{2}a = b^{3} \\
a^{-1}b^{4}a = b^{6} \\
a^{-1}b^{6}a = b^{9} \\
b^{4} = b^{9} \\
b^{5} = e
\end{gather}$$

## Задача 2

$G: \ b^{-1}a^{2}b = a^{3}, \ a^{-1}b^{2}a = b^{3}, \ \text{Д-ть}: \ a = b = e$

$$\begin{gather}
b^{-1}a^{2k}b = a^{3k} \\
k = 3: \ b^{-1}a^{6}b = a^{9} \\
k = 4: \ b^{-1}a^{8}b = a^{12} \\
k = 6: \ b^{-1}a^{12}b = a^{18} \\
k = 9: \ b^{-1}a^{18}b = a^{27} \\
b^{-2}a^{8}b^{2} = a^{18} \\
b^{-3}a^{8}b^{3} = a^{27} \\
\\
b^{2}a = ab^{3} \\
b^{2}a = ab^{3} \\
\dots
\end{gather}$$

## Доказать, что $\mathrm{ord} \ g = \mathrm{ord} \ g^{-1}$...

$G, \ G^{0} - \text{дуальная группа}, *$
$x * y := yx, \ G \cong G^{0}$

$$\begin{gather}
(x*y)*z = (yx)*z = z(yx) \\
\dots (zy)x = z(yx) \\
e * x = xe = x \\
x * e = ex = x \\
x^{-1} * x = xx^{-1} = e \\
x * x^{-1} = x^{-1}x = e \\
\phi: G^{0} \to G \\
x \mapsto \phi(x) = x^{-1} \\
\phi(x*y) = (x*y)^{-1} = (yx)^{-1} = x^{-1}y^{-1} = \phi(x)\phi(y) \\
\phi(xy) = (xy)^{-1} = y^{-1}x^{-1} = \phi(y)\phi(x) = \phi(x)*\phi(y) \\
\end{gather}$$

## Задача 3

Доказать, что если $g^{2} = e \ \forall g \in G \implies$ группа - коммутативна

$$\begin{gather}
x^{2} = e \implies x = x^{-1} \\
xy = (xy)^{-1} = y^{-1}x^{-1} = yx
\end{gather}$$

## Задача 4

$H_{1} < G, \ H_{2} < G \implies H_{1} \cap H_{2} < G$ - очев.

$$\begin{gather}
H_{1}, H_{2} < G, H_{1} \cup H_{2} \leq G \implies H_{1} < H_{2} \ \text{или} \ H_{2} < H_{1}
\end{gather}$$

От противного:
Тогда $\exists h_{1} \in H_{1} \setminus H_{2}$ и $\exists h_{2} \in H_{2} \setminus H_{1}$. $h_{1}h_{2} \in H_{1}\cup H_{2}$. Если $h_{1}h_{2} \in H_{1}$, то $h_{2} \in H_{1}$, что противоречит условию, аналогично наоборот.

## Задача 5

$x \in G, \ |x| = n$. Доказать, что $|x^{k}| = \frac{n}{(k,n)}$.

$$\begin{gather}
(k,n) = d, \ n = n_{1}d, \ k = k_{1}d, \ (k_{1}, n_{1}) = 1 \\
\end{gather}$$