---
tags:
  - типовой-расчет
  - 2nd-semester
  - 2025-05-03
---

## СГВМ ТР 3

### Ершов Алексей Геннадьевич КМБО-03-23

### Вариант 5

$$\begin{gather}
\begin{cases}
\dot{x} = 2x+y \\
\dot{y} = 4x-y+(2t+1)e^{t}
\end{cases}
\end{gather}$$

### а) Метод вариации произвольных постоянных

$$\begin{gather}
A = \begin{pmatrix}
2 & 1 \\
4 & -1
\end{pmatrix} \\
\det(A - \lambda E) = \begin{vmatrix}
2-\lambda & 1 \\
4 & -1-\lambda
\end{vmatrix} = \lambda^{2}-\lambda-6 = 0 \\
\lambda_{1} = -2, \ \lambda_{2} = 3 \\
\vec{x}_{1} = \begin{pmatrix}
-1 \\
4
\end{pmatrix}, \ \vec{x}_{2} = \begin{pmatrix}
1 \\
1
\end{pmatrix}
\end{gather}$$

$$\begin{gather}
\begin{pmatrix}
x \\
y
\end{pmatrix} = C_{1}e^{-2t}\begin{pmatrix}
-1 \\
4
\end{pmatrix} + C_{2}e^{3t}\begin{pmatrix}
1 \\
1
\end{pmatrix} \\
\begin{pmatrix}
-e^{-2t} & e^{3t} \\
4e^{-2t} & e^{3t}
\end{pmatrix}\begin{pmatrix}
C_{1} \\
C_{2}
\end{pmatrix} = X(t)\mathbf{C} \\
X_{он} = X(t)\mathbf{C}(t) \\
\dot{\mathbf{C}} = X^{-1}\mathbf{f}
\end{gather}$$

$$\begin{gather}
\mathbf{f} = \begin{pmatrix}
0 \\
(2t+1)e^{t}
\end{pmatrix} \\
\det X = -e^{3t - 2t} - 4e^{3t - 2t} = -5e^{t} \\
X^{-1} = -\frac{1}{5e^{t}}\begin{pmatrix}
e^{3t} & -e^{3t} \\
-4e^{-2t} & -e^{-2t}
\end{pmatrix} = \frac{1}{5}\begin{pmatrix}
-e^{2t} & e^{2t} \\
4e^{-3t} & e^{-3t}
\end{pmatrix} \\
\dot{\mathbf{C}} = (2t+1)\begin{pmatrix}
e^{3t} \\
e^{-2t}
\end{pmatrix} \\
\end{gather}$$

$$\begin{gather}
\mathbf{C} = \begin{pmatrix}
\frac{1}{9}e^{3t}(6t+1) + \tilde{C}_{1} \\
-e^{-2t}(t+1) + \tilde{C}_{2}
\end{pmatrix} \\
X_{он} = X_{оо}\mathbf{C} \\
\end{gather}$$

$$\begin{gather}
X_{он} = \begin{pmatrix}
-e^{-2t} & e^{3t} \\
4e^{-2t} & e^{3t}
\end{pmatrix}\begin{pmatrix}
\frac{1}{9}e^{3t}(6t+1) + \tilde{C}_{1} \\
-e^{-2t}(t+1) + \tilde{C}_{2}
\end{pmatrix} = \\
= \begin{pmatrix}
-\tilde{C}_{1}e^{-2t} + \tilde{C}_{2}e^{3t} + e^{t}\left[ -\frac{1}{9}(6t+1) -(t+1) \right] \\
4\tilde{C}_{1}e^{-2t} + \tilde{C}_{2}e^{3t} + e^{t}\left[ \frac{4}{9}(6t+1) - (t+1) \right]
\end{pmatrix} = \\
\end{gather}$$

$$\begin{gather}
= \begin{pmatrix}
-\tilde{C}_{1}e^{-2t} + \tilde{C}_{2}e^{3t} + e^{t}\left( -\frac{5}{3}t - \frac{10}{9} \right) \\
4\tilde{C}_{1}e^{-2t} + \tilde{C}_{2}e^{3t} + e^{t}\left( \frac{5}{3}t - \frac{5}{9} \right)
\end{pmatrix}
\end{gather}$$

### б) Метод неопределенных коэффициентов

$$\begin{gather}
\mathbf{f} = \begin{pmatrix}
0 \\
e^{t}(2t+1)
\end{pmatrix} \implies X_{чн} = \mathbf{Q}(t)e^{t}, \ \mathrm{deg} \ \mathbf{Q} \leq 1 \\
X_{чн} = \begin{pmatrix}
e^{t}(at+b) \\
e^{t}(ct+d)
\end{pmatrix}
\end{gather}$$

$$\begin{gather}
\begin{cases}
(e^{t}(at+b))' = 2e^{t}(at + b) + e^{t}(ct+d) \\
(e^{t}(ct+d))' = 4e^{t}(at + b) - e^{t}(ct+d) + e^{t}(2t+1) \\
\end{cases} \\
\begin{cases}
e^{t}(at+b) + ae^{t} = e^{t}[(2a+c)t + (2b+d)] \\
e^{t}(ct+d) + ce^{t} = 4e^{t}((4a)t + 4b) - e^{t}(ct+d) + e^{t}(2t+1) \\
\end{cases}
\end{gather}$$