---
tags:
  - типовой-расчет
  - 2nd-semester
  - 2025-05-17
---

## СГВМ ТР 6

### Ершов Алексей Геннадьевич КМБО-03-23

### Вариант 5

$$\begin{gather}
\begin{cases}
\dot{x} = \sqrt{ \cos x - 6y } - 2\ln (x+y+1) - 1 \\
\dot{y} = 2e^{x+2y} - 2\cos x
\end{cases}
\end{gather}$$

Найдем первое приближение системы при помощи эквивалентностей:

$$\begin{gather}
\sqrt{ \cos x - 6y } - 2\ln (x+y+1) - 1 = \\
= \sqrt{ 1 - (1 -\cos x) - 6y } - 2\ln (x+y+1) - 1 = \\
= \left( 1+ \left( -\frac{x^{2}}{2} - 6y \right) \right)^{1/2} - 1 - 2(x+y) = \\
= \frac{1}{2}\left( -\frac{x^{2}}{2} - 6y \right) - 2x-2y = \\
\end{gather}$$

$$\begin{gather}
-\frac{x^{2}}{}
\end{gather}$$