---
tags:
  - seminar
  - 2nd-semester
  - 2024-10-24
---

$$\begin{gather}
\sum_{n=1}^{\infty} x^{n}\sin \frac{1}{2^{n}} , \ \text{а}) \ x \in (-2,2), \text{б}) \ x \in [-1, 1] \\
\end{gather}$$

$$\begin{gather}
\sum_{n=1}^{\infty} \frac{x^{3}}{(1+x^{3})^{n}}, \ x \in (0, +\infty) \\
\exists \epsilon_{0} >0 \ | \ \forall N \ \exists n > N \ \text{и} \ \exists \tilde{x} \in (0; +\infty) \ | \  |R_{n}(\tilde{x}) \geq \epsilon_{0}| \\
S_{n}(x) = \frac{x^{3}}{(1+x^{3})} + \frac{x^{3}}{(1+x^{3})^{2}} + \dots + \frac{x^{3}}{(1+x^{3})^{n}} = \\
= \frac{x^{3}}{1+x^{3}} \left( 1+ \frac{1}{x^{3}+1}+ \frac{1}{(1+x^{3})^{2}} + \dots \right) = \begin{bmatrix}
\text{геом. прог.}
\end{bmatrix} = \\
= 1 - \frac{1}{(x^{3}+1)^{n}} \implies S(x) = \lim_{ n \to \infty } S_{n}(x) = \lim_{ n \to \infty } \left( 1-\frac{1}{1+x^{3}} \right) = 1 \\
R_{n}(x) = S(x) - S_{n}(x) = 1- \left( 1-\frac{1}{(1+x^{3})^{n}} \right) = \frac{1}{(1+x^{3})^{n}} \\
\text{возьмем} \ n = N+1 \\
\tilde{x} = (\sqrt[n]{ 2 })^{1/3} \in (0; +\infty) \\
R_{n}(\tilde{x}) = \frac{1}{(1 + \tilde{x}^{3})^{n}} = \frac{1}{((\sqrt[n]{ 2 }-1)+1)^{n}} = \frac{1}{2} > \frac{1}{4} = \epsilon_{0} \\
\text{Показали, что } \exists \epsilon_{0} = \frac{1}{4} > 0 \ | \  \forall N \ \exists n = N+1 > N \ \text{и} \ \exists \tilde{x} = \\
= (\sqrt[n]{ 2 })^{1/3} \in (0; +\infty) \text{для которых} \\
|R_{n}(\tilde{x})| = R_{n}(\tilde{x}) \geq \epsilon_{0} \\
\implies \text{ряд неравн. по определению}
\end{gather}$$

$$\begin{gather}
\sum_{n=1}^{\infty} \ln\left( 1+\frac{x^{2}}{n^{2}} \right)
\end{gather}$$