---
tags:
  - homework
  - 2nd-semester
  - 2024-11-20
---

### 5

$$\begin{gather}
f(x) = \sin 2x + 2x \cos 2x \\
\begin{bmatrix}
u = 2x
\end{bmatrix} = \sum_{n=0}^{\infty} \frac{(-1)^{n}u^{2n+1}}{(2n+1)!} + u\sum_{n=0}^{\infty} \frac{(-1)^{n}u^{2n}}{(2n)!} = \\
= \sum_{n=0}^{\infty} \frac{(-1)^{n}u^{2n+1}(1+2n+1)}{(2n+1)!} = \\
= \sum_{n=0}^{\infty} \frac{(-1)^{n}2^{2n+2}(n+1)}{(2n+1)!}x^{2n+1}, \ x \in (-\infty, + \infty)
\end{gather}$$

### 8

$$\begin{gather}
f(x) = \frac{1}{(1-x^{3})^{2}} = \begin{bmatrix}
u = -x^{3}
\end{bmatrix} = \frac{1}{(1+u)^{2}} = (1+u)^{-2} \\
(1+u)^{\alpha} = \sum_{n=0}^{\infty} \frac{\alpha(\alpha-1)\dots(\alpha-n+1)}{n!}u^{n}, \ u \in (-1, 1) \\
(1+u)^{-2} = \sum_{n=0}^{\infty} \frac{(-2)(-3)\dots(-1-n)}{n!}u^{n} = \sum_{n=0}^{\infty} \frac{(-1)^{n}(n+1)!}{n!}u^{n} = \\
= \sum_{n=0}^{\infty} (-1)^{n}(n+1)(-x^{3})^{n} = \sum_{n=0}^{\infty} (-1)^{2n}(n+1)x^{3n} = \\
= \sum_{n=0}^{\infty} (n+1)x^{3n} \\
|u| < 1 \implies |-x^{3}| < 1 \implies -1 < x^{3} < 1 \implies -1 < x < 1 \\
\sum_{n=0}^{\infty} (n+1)x^{3n}, \ x \in (-1, 1) \\
\end{gather}$$

### 9

$$\begin{gather}
f(x) = \sqrt{ 1-x^{2} } = \begin{bmatrix}
u = -x^{2}
\end{bmatrix} = (1 + u)^{1/2} \\
f(x) = \sum_{n=0}^{\infty} \frac{\frac{1}{2}\left( \frac{1}{2} - 1 \right)\dots\left( \frac{1}{2} - n + 1 \right)}{n!}u^{n} = \\
= \sum_{n=0}^{\infty} \frac{\frac{1}{2}\cdot \left( -\frac{1}{2} \right)\cdot \left( -\frac{3}{2} \right)\dots\left( -\frac{2n-3}{2} \right)}{n!}u^{n} = \\
= 1 + \sum_{n=1}^{\infty} \frac{\overbrace{\frac{1}{2}\cdot \left( -\frac{1}{2} \right)\left( -\frac{3}{2} \right)\dots\left( -\frac{n-3}{2} \right)}^{\frac{(-1)^{n+1}(2n-3)!!}{2^{n}}}}{n!}(-x^{2})^{n} = \\
= 1 + \sum_{n=1}^{\infty} \frac{(-1)^{n}(-1)^{n+1}(2n-3)!!}{2^{n}n!}x^{2n} = \\
= 1-\sum_{n=1}^{\infty} \frac{(2n-3)!!}{2^{n}n!}x^{2n} \\
|-x^{2}| < 1 \implies x^{2} < 1 \implies -1 < x < 1 \implies x \in (-1; 1)
\end{gather}$$

### 10

$$\begin{gather}
f(x) = \frac{5x-4}{x+2} = \frac{5x + 10 - 14}{x+2} = 5-\frac{14}{x+2} = \\
= 5-7\left( \frac{x}{2} + 1 \right)^{-1} = \begin{bmatrix}
\frac{x}{2}= u
\end{bmatrix} = 5-7(u+1)^{-1} = \\
= 5 - 7\sum_{n=0}^{\infty} \frac{(-1)(-2)\dots(-n)}{n!}u^{n} = \\
-2 - 7\sum_{n=1}^{\infty} \frac{(-1)^{n}n!}{n!}\left( \frac{x}{2} \right)^{n} = \\
= -2-7\sum_{n=1}^{\infty} \frac{(-1)^{n}}{2^{n}}x^{n} = \\
= -2+\sum_{n=1}^{\infty} \frac{7(-1)^{n+1}}{2^{n}}x^{n}, \ \left|\frac{x}{2}\right| < 1 \implies x \in (-2; 2)
\end{gather}$$

### 11

$$\begin{gather}
f(x) = \frac{1}{x^{2}-2x-3} = \frac{1}{(x+1)(x-3)} = \frac{}{x+1} + \frac{}{x-3}
\end{gather}$$

### 16
### 17
### 18