---
tags:
  - homework
  - 2nd-semester
  - 2024-11-14
---

### 2

$$\begin{gather}
\sum_{n=0}^{\infty} \frac{(-1)^{n}x^{n}}{2n+1} \\
x-x_{0} = x - 0 \implies x_{0} = 0 \\
c_{n} = \frac{(-1)^{n}}{2n+1}, \ n = 0,1,2,\dots \\
c_{n} - \text{сх-ся абсолютно по пр. Лейбница (очев.)} \\
\lim_{ n \to \infty } \left| \frac{a_{n+1}}{a_{n}} \right| = 1 = L \\
R = \frac{1}{L} = 1 - \text{радиус сходимости} \\
(x_{0}-R; x_{0}+R) = (-1;1) - \text{интервал сходимости} \\
x = 1: \ 
\sum_{n=0}^{\infty} \frac{(-1)^{n}}{2n+1} - \text{сх-ся абсолютно по пр. Лейбница (очев.)} \\
x = -1: \ \sum_{n=0}^{\infty} \frac{1}{2n+1} - \text{расх. (гармонический ряд)} \\
\end{gather}$$

![[2024-11-14 Домашнее задание - Ряды 2024-11-14 10.02.48.excalidraw]]

1. $R = 1$
2. $(-1, 1)$
3. $x=-1$ - расх., $x=1$ - сх. абс.
4. $(a, 1] \subset [-1, 1]$ - сходится равномерно

### 5

$$\begin{gather}
\sum_{n=1}^{\infty} \frac{(x+1)^{n}}{\sqrt{ n+1 }} \ln \frac{3n-2}{3n+2} \\
x - x_{0} = x+1 \implies x_{0} = -1 \\
c_{n} = \frac{1}{\sqrt{ n+1 }}\ln \frac{3n-2}{3n+2}, n = 1,2,\dots \\
\lim_{ n \to \infty } \frac{a_{n+1}}{a_{n}} = \lim_{ n \to \infty } \frac{\sqrt{ n+1 }\ln \frac{3n+1}{3n+5}}{\sqrt{ n+2 }\ln \frac{3n-2}{3n+2}} = \lim_{ n \to \infty } \frac{\ln \left( 1 + \frac{-4}{3n+5} \right) }{\ln \left( 1 + \frac{-4}{3n+2} \right) } = \\
= \lim_{ n \to \infty } \frac{3n+2}{3n+5} = 1 = L \\ 
R = \frac{1}{L} = 1 \\
(x_{0} - R; x_{0}+R) = (-1 - 1; -1 + 1) = (-2; 0) \\
x = -2: \ \sum_{n=1}^{\infty} \frac{(-1)^{n}}{\sqrt{ n+1 }} \ln\frac{3n-2}{3n+2} \\

\end{gather}$$