---
tags:
  - homework
  - 2nd-semester
  - 2024-11-26
---

### 534

$$\begin{gather}
y'' + y = 4xe^{x} \\
\lambda^{2} + 1 = 0 \\
\lambda_{1, 2} = \pm i \\
\phi_{1} = \cos x, \ \phi_{2} = \sin x \\
y_{оо} = c_{1}\cos x + c_{2}\sin x, c_{1}, c_{2} = \mathrm{const} \\
y_{он} =c_{1}(x)\cos x + c_{2}(x)\sin x \\
\begin{cases}
c_{1}'(x)\cos x + c_{2}'(x) \sin x = 0 \\
-c_{1}'(x)\sin x + c_{2}'(x) \cos x = 4xe^{x} \\
\end{cases} \\
\begin{cases}
c_{1}'(x)\sin x\cos x + c_{2}'(x) \sin^{2} x = 0 \\
-c_{1}'(x)\sin x\cos x + c_{2}'(x) \cos^{2} x = 4xe^{x}\cos x \\
\end{cases} \\
\end{gather}$$

$$\begin{gather}
\begin{cases}
c_{1}'(x)\sin x\cos x + c_{2}'(x) \sin^{2} x = 0 \\
-c_{1}'(x)\sin x\cos x + c_{2}'(x) \cos^{2} x = 4xe^{x}\cos x \\
\end{cases} \\
c_{2}'(x) = 4xe^{x}\cos x \\
c_{1}'(x) = -4xe^{x}\sin x \\
\end{gather}$$

$$\begin{gather}
c_{1}(x) = -2e^{x}(x(\sin x-\cos x)+\cos x) + \tilde{c}_{1} \\
c_{2}(x) = 2e^{x}((x-1)\sin x +x\cos x) + \tilde{c}_{2} \\
y_{он} = 2e^{x}(x\sin x\cos x + x\cos ^{2} x - \sin x\cos x + x\sin ^{2} x - x\sin x\cos x + \cos x\sin x) = \\
= 2e^{x}x + 2e^{x} + \tilde{c}_{1}\cos x + \tilde{c}_{2}\sin x 
\end{gather}$$

### 538

$$\begin{gather}
y'' + y = 4\sin x \\
\lambda^{2} + 1 = 0 \\
\lambda_{1,2} = \pm i \\
\phi_{1} = \cos x, \ \phi_{2} = \sin x \\
y_{оо} = c_{1}\cos x + c_{2}\sin x, c_{1}, c_{2} = \mathrm{const} \\
y_{он} = c_{1}(x)\cos x + c_{2}(x)\sin x \\
\begin{cases}
c_{1}'(x)\cos x + c_{2}'(x)\sin x = 0 \\
-c_{1}'(x)\sin x + c_{2}'(x)\cos x = 4\sin x \\
\end{cases} \\
\end{gather}$$

$$\begin{gather}
\begin{cases}
c_{1}'(x)\sin x\cos x + c_{2}'(x)\sin ^{2} x = 0 \\
-c_{1}'(x)\sin x\cos x + c_{2}'(x)\cos ^{2} x = 4\sin x\cos x \\
\end{cases} \\
\end{gather}$$