---
tags:
  - homework
  - 2nd-semester
  - 2024-10-22
---

## 1

$$\begin{gather}
[a_{j}^{i}] = \begin{bmatrix}
\frac{1}{2} & 0 & \frac{1}{2} \\
0 & 1 & 0 \\
\frac{1}{2} & 0 & \frac{1}{2}
\end{bmatrix}, \ g_{ij} = \delta_{ij} \\
\begin{vmatrix}
\frac{1}{2} - \lambda & 0 & \frac{1}{2} \\
0 & 1 - \lambda & 0 \\
\frac{1}{2} & 0 & \frac{1}{2} - \lambda 
\end{vmatrix} = 0 \\
\begin{vmatrix}
- \lambda & 0 & \lambda \\
0 & 1 - \lambda & 0 \\
\frac{1}{2} & 0 & \frac{1}{2} - \lambda 
\end{vmatrix} = 0 \\
\frac{1}{2}\begin{vmatrix}
- \lambda & 0 & \lambda \\
0 & 1 - \lambda & 0 \\
1 & 0 & 1 - 2\lambda 
\end{vmatrix} = 0 \\
\begin{vmatrix}
0 & \lambda \\
1-\lambda & 0
\end{vmatrix} + (1-2\lambda)\begin{vmatrix}
-\lambda & 0 \\
0 & 1-\lambda
\end{vmatrix} = 0 \\
-\lambda(1-\lambda) - \lambda(1-2\lambda)(1-\lambda) = 0 \\
\lambda(1-\lambda)(1 - \lambda) = 0 \\
\lambda(1-\lambda)^{2} = 0 \\
\lambda_{1} = 0, \ \lambda_{2,3} = 1 \\
\end{gather}$$

$$\begin{gather}
\begin{pmatrix}
\frac{1}{2} & 0 & \frac{1}{2} \\
0 & 1 & 0 \\
\frac{1}{2} & 0 & \frac{1}{2}
\end{pmatrix}\begin{pmatrix}
1 \\
0 \\
-1
\end{pmatrix} = \vec{0} \implies \vec{x}_{1} = \begin{pmatrix}
1 \\
0 \\
-1
\end{pmatrix} \\
\begin{pmatrix}
-\frac{1}{2} & 0 & \frac{1}{2} \\
0 & 0 & 0 \\
\frac{1}{2} & 0 & -\frac{1}{2}
\end{pmatrix}\begin{pmatrix}
1 \\
0 \\
1
\end{pmatrix} = \vec{0} \implies \vec{x}_{2} = \begin{pmatrix}
1 \\
0 \\
1
\end{pmatrix} \\
\begin{pmatrix}
-\frac{1}{2} & 0 & \frac{1}{2} \\
0 & 0 & 0 \\
\frac{1}{2} & 0 & -\frac{1}{2}
\end{pmatrix}\begin{pmatrix}
1 \\
1 \\
1
\end{pmatrix} = \vec{0} \implies \vec{x}_{3} = \begin{pmatrix}
1 \\
1 \\
1
\end{pmatrix}
\end{gather}$$

$$\begin{gather}
a_{i}^{i} = 1 + \frac{1}{2} + \frac{1}{2} = 2, \ a_{i}^{i} = \sum_{i=1}^{n} \lambda_{i} = 0+1+1 = 2 \\
a_{j}^{i}a_{i}^{j} = \sum_{i,j=1}^{n} a_{ij}a_{ji} = 2\cdot \frac{1}{4} + 1 + 2 \cdot \frac{1}{4} = 2, \ a_{j}^{i}a_{i}^{j} = \sum_{i=1}^{n} \lambda^{2}_{i} = 2\cdot 1^{2} = 2 \\
\end{gather}$$

$$\begin{gather}
\omega(2,2,1), [J^{ij}] = \begin{bmatrix}
2 & 0 & 1 \\
0 & 1 & 0 \\
1 & 0 & 3
\end{bmatrix}, g_{ij} = \delta_{ij} \\
E = \frac{1}{2}J^{ij}\omega_{i}\omega_{j} = \frac{1}{2}\omega J\omega^{T} \\
L^{i} = J^{ij}\omega_{j} = J\omega^{T} \\
E = \frac{1}{2}\begin{pmatrix}
2 & 2 & 1
\end{pmatrix}\begin{pmatrix}
2 & 0 & 1 \\
0 & 1 & 0 \\
1 & 0 & 3
\end{pmatrix}\begin{pmatrix}
2 \\
2 \\
1
\end{pmatrix} = \begin{pmatrix}
5 & 2 & 5
\end{pmatrix}\begin{pmatrix}
2 \\
2 \\
1
\end{pmatrix} = 19 \\
L^{i} = 
\begin{pmatrix}
2 & 0 & 1 \\
0 & 1 & 0 \\
1 & 0 & 3
\end{pmatrix}\begin{pmatrix}
2 \\
2 \\
1
\end{pmatrix} = 
\end{gather}$$