---
tags:
  - homework
  - 2nd-semester
  - 2024-11-15
---

576 578 593
### 576

$$\begin{gather}
y'' + 3y' + 2y = \frac{1}{e^{x}+1} \\
\alpha^{2} + 3\alpha + 2 = 0 \\
\alpha_{1} = -1, \ \alpha_{2} = -2 \\
\phi_{1} = e^{-x}, \ \phi_{2} = e^{-2x} \\
y_{оо} = c_{1}e^{-x} + c_{2}e^{-2x}, \ c_{1},c_{2} = const \\
y_{он} = c_{1}(x)e^{-x} + c_{2}(x)e^{-2x} \\
\begin{cases}
c'_{1}(x)e^{-x} + c'_{2}(x)e^{-2x} = 0 \\
-c'_{1}(x)e^{-x} + -2c'_{2}(x)e^{-2x} = \frac{1}{e^{x}+1} \\
\end{cases} \\
c'_{2}(x) = \frac{e^{2x}}{e^{x}+1} \\
c'_{1}(x) = -\frac{e^{x}}{e^{x}+1} \\
\end{gather}$$

$$\begin{gather}
c_{2}(x) = \int \frac{e^{x}}{e^{x}+1} \, de^{x} \\
c_{2}(x) = \int de^{x} - \int \frac{d(e^{x}+1)}{e^{x}+1} \\
c_{2}(x) = e^{x} +
\end{gather}$$

