---
tags:
  - homework
  - 2nd-semester
  - 2024-12-05
---

### 5

$$\begin{gather}
y'' = -2xy, \ y(0) = 1, \ y'(0) = 1 \\
y(x) = \sum_{n=0}^{\infty} a_{n}x^{n}, \ y'(x) = \sum_{n=0}^{\infty} a_{n}nx^{n-1}, \ y''(x)=  \sum_{n=0}^{\infty} a_{n}n(n-1)x^{n-2} \\
\left[ y(0) = 1 \implies a_{0} = \frac{y(0)}{0!} = 1, \ y'(0) = 1 \implies a_{1} = \frac{y'(0)}{1!} = 1 \right] \\
2\sum_{n=0}^{\infty} a_{n}x^{n+1} + \sum_{n=0}^{\infty}a_{n}n(n-1)x^{n-2} = 0 \\
2\sum_{k=1}^{\infty} a_{k-1}x^{k} + \sum_{k=0}^{\infty}a_{k+2}(k+2)(k+1)x^{k} = 0 \\
\sum_{k=0}^{\infty} [2a_{k-1} + a_{k+2}(k+2)(k+1)]x^{k} = 0
\end{gather}$$

$$\begin{gather}
\begin{array}{c|c}
x^{0} & a_{2}\cdot 2\cdot 1 = 0 \implies a_{2} = 0 \\
\hline x^{1} & 2a_{0} + a_{3}\cdot 3 \cdot 2 = 0 \implies a_{3} = -\frac{1}{3} \\
\hline x^{2} & 2a_{1} + a_{4} \\ 
\hline x^{3} & \\
\hline x^{k} & 2a_{k-1} + a_{k+2}(k+2)(k+1) = 0 \implies\\
\end{array} \\
\implies a_{k+2} = -\frac{2a_{k-1}}{(k+1)(k+2)}
\end{gather}$$