---
tags:
  - homework
  - 2nd-semester
  - 2024-11-13
---

### 511

$$\begin{gather}
y'' + y' - 2y = 0 \\
\lambda^{2} + \lambda - 2 = 0 \\
(\lambda - 1)(\lambda + 2) = 0 \\
\lambda_{1} = 1, \ \lambda_{2} = -2 \\
y = C_{1}e^{x} + C_{2}e^{-2x}
\end{gather}$$

### 515

$$\begin{gather}
y'' - 4y' + 5y = 0 \\
\lambda^{2} - 4\lambda + 5 = 0 \\
D = -4, \ \sqrt{ D } = 2i \\
\lambda_{1} = \frac{4 - 2i}{2} = 2-i \\
\lambda_{2} = \frac{4+2i}{2} = 2+i \\
y = C_{1}e^{2x}\cos x + C_{2} e^{2x} \sin x = \\
= e^{2x} (C_{1} \cos x + C_{2} \sin x)
\end{gather}$$

### 518

$$\begin{gather}
y''' - 8y = 0 \\
\lambda^{3} - 8 = 0 \\
(\lambda-2)(\lambda^{2} + 2\lambda + 4) = 0 \\
(\lambda - 2)(\lambda - (-1 - i\sqrt{ 3 }))(\lambda - (-1 + i\sqrt{ 3 })) = 0 \\
\lambda_{1} = 2, \ \lambda_{2,3} = -1 \pm i\sqrt{ 3 } \\
y = C_{1}e^{2x} + e^{-x}(C_{2}\cos (x\sqrt{ 3 }) + C_{3}\cos (x\sqrt{ 3 }))
\end{gather}$$

### 524

$$\begin{gather}
y^{V} -6y^{IV} + 9y''' = 0 \\
\lambda^{3}(\lambda^{2} - 6\lambda + 9) = 0 \\
\lambda^{3}(\lambda - 3)^{2} = 0 \\
\lambda_{1,2,3} = 0, \ \lambda_{4,5} = 3 \\
y = C_{1} + C_{2}x + C_{3}x^{2} + e^{3x}(C_{4} + C_{5}x)
\end{gather}$$

### 613

$$\begin{gather}
y_{1} = x^{2}e^{x} \\
(\lambda - 1)^{3} = 0 \\
\lambda^{3} - 3\lambda^{2} + 3\lambda - 1 = 0 \\
y''' - 3y'' + 3y' - y = 0 \\
y = e^{x}(C_{1} + C_{2}x + C_{3}x^{2}) \\
C_{1} = C_{2} = 0, C_{3} = 1: \ y = x^{2}e^{x} \\
\end{gather}$$

### 691

$$\begin{gather}
xy'' - (x+1)y' - 2(x-1)y = 0 \\
y_{1} = x^{n} + a_{1}x^{n-1} + \dots + a_{n} \\
y_{1}' = nx^{n-1} + a_{1}(n-1)x^{n-2} + \dots + a_{n-1} \\
y''_{1} = n(n-1)x^{n-2} + a_{1}(n-1)(n-2)x^{n-3} + \dots + 2a_{n-2} \\
2x^{n+1} = 0 \implies x^{n+1} = 0 \\
(-n - 2a_{1})x^{n} = 0 \implies n = -2a_{1} \\
\left( n(n-1) - a_{1}(n-1) -2a_{2} \right)x^{n-1} = 0 \implies \\
\implies -2a_{1}(-2a_{1}-1) - a_{1}(-2a_{1} - 1) - 2a_{2}  = 0\\
(a_{1}(n-1)(n-2) - a_{2}(n-2)(n-3) - 2a_{3})x^{n-2} = 0 \\
n = 2 \implies a_{1} = -1 \implies a_{2} = -\frac{3}{2} \\
y_{1} = x^{2} -x + a_{2} \\
2x - (x+1)(2x-1) - 2(x-1)(x^{2} - 2 + a_{2}) = 0 \\
2x - (2x^{2} + x - 1)
\end{gather}$$

### 525

$$\begin{gather}
y^{V} - 10y''' + 9y' = 0 \\
\lambda^{5} - 10\lambda^{3} + 9\lambda = 0 \\
\lambda(\lambda^{4} - 10\lambda^{2} + 9) = 0 \\
\lambda(\lambda^{2} - 1)(\lambda^{2} - 9) = 0 \\
\lambda_{1} = 0, \ \lambda_{2,3} = \pm 1, \ \lambda_{4,5} = \pm 3 \\
y = C_{1} + e^{x}C_{2} + e^{-x}C_{3} + e^{3x}C_{4} + e^{-3x}C_{5}
\end{gather}$$

### 528

$$\begin{gather}
y''' - y'' -y' + y = 0 \\ 
\lambda^{3} - \lambda^{2} - \lambda + 1 = 0 \\
(\lambda-1)(\lambda^{2} -1) = 0 \\
(\lambda-1)^{2}(\lambda+1) = 0 \\
\lambda_{1,2} = 1, \ \lambda_{3} = -1 \\
y = e^{x}(C_{1} + C_{2}x) + e^{-x}C_{3} \\
\end{gather}$$

### 530

$$\begin{gather}
y^{V} + 8y''' + 16y' = 0 \\
\lambda^{5} +8\lambda^{3} + 16\lambda = 0 \\
\lambda(\lambda^{4} + 8\lambda^{2} + 16 ) = 0 \\
\lambda(\lambda^{2} + 4)^{2} = 0 \\
\lambda(\lambda - 2i)^{2}(\lambda + 2i)^{2} = 0 \\
\lambda_{1} = 0, \ \lambda_{2,3} = 2i, \ \lambda_{4,5} = -2i \\
y = C_{1} + (C_{1} + C_{2}x)\cos 2x + (C_{3} + C_{4}x)\sin 2x
\end{gather}$$