---
tags:
  - homework
  - 2nd-semester
  - 2025-02-27
---

### 1145

$$\begin{gather}
\begin{cases}
2zy' = y^{2}-z^{2}+1 \\
z'=z+y
\end{cases} \\
\end{gather}$$

$$\begin{gather}
\begin{cases}
2z(z'' - z') = (z'-z)^{2}-z^{2}+1 \ (*) \\
y = z' - z \\
\end{cases} \\
(*) \ 2zz''-2zz' = z'^{2} - 2zz' + z^{2} - z^{2} + 1 \\
2zz'' = z'^{2} + 1 \\
\begin{bmatrix}
z'_{x} = u'_{y} = u' \\
z''_{x} = u'_{y}z'_{x} = u'u
\end{bmatrix}
\end{gather}$$

$$\begin{gather}
2zu'u = u^{2} + 1 \\
\frac{2u'u}{u^{2}+1} = \frac{1}{z} \\
\int \frac{2udu}{u^{2}+1} = \int \frac{dy}{z} \\
\int \frac{d(u^{2}+1)}{u^{2}+1}  = \int \frac{dz}{z}
\end{gather}$$

$$\begin{gather}
\ln |u^{2}+1| = \ln |z| + \ln C_{1} \\
u^{2} + 1 = C_{1}z \\
(z')^{2} = C_{1}z-1 \\
z' = \pm \sqrt{ C_{1}z-1 } \\
\end{gather}$$

$$\begin{gather}
\int \frac{z'dx}{\sqrt{ C_{1}z-1 }} = \int dx \\
\frac{2}{C_{1}}\int \frac{d(C_{1}z-1)}{2\sqrt{ C_{1}z-1 }} = x + C_{2} \\
\frac{2\sqrt{ C_{1}z - 1 }}{C_{1}} = x + C_{2} \\
\sqrt{ C_{1}z-1 } = \frac{C_{1}}{2}(x+C_{2}) \\
\end{gather}$$

$$\begin{gather}
C_{1}z-1 = \frac{C_{1}^{2}}{4}(x + C_{2})^{2} \\
z = \frac{C_{1}}{4}(x+C_{2})^{2} + \frac{1}{C_{1}} \\
z' = \frac{C_{1}}{2}(x + C_{2})
\end{gather}$$

$$\begin{gather}
\begin{cases}
z = \frac{C_{1}}{4}(x+C_{2})^{2} + \frac{1}{C_{1}} \\
y = \frac{C_{1}}{2}(x+C_{2}) -\frac{C_{1}}{4}(x+C_{2})^{2} - \frac{1}{C_{1}}
\end{cases}
\end{gather}$$

### 1154

$$\begin{gather}
\frac{dx}{x} = \frac{dy}{y} = \frac{dz}{xy+z} \\
\frac{dx}{x} = \frac{dy}{y} \\
\ln x = \ln y + C_{1} \\
y = C_{1}x \\
\end{gather}$$

$$\begin{gather}
\frac{dx}{x} = \frac{dz}{xy+z} \\
\frac{dx}{x} = \frac{dz}{x\cdot C_{1}x+z} \\
\frac{dx}{x} = \frac{dz}{C_{1}x^{2}+z} \\
z'_{x} = \frac{C_{1}x^{2}+z}{x} \\
\end{gather}$$

$$\begin{gather}
z' - C_{1}x - \frac{z}{x} = 0 \\
\begin{bmatrix}
z = uv \\
z' = u'v+uv'
\end{bmatrix} \\
u'v+uv'-\frac{uv}{x}-C_{1}x = 0 \\
v' = \frac{v}{x} \\
\frac{v'}{v} = \frac{1}{x} \\
v = x
\end{gather}$$

$$\begin{gather}

\end{gather}$$