---
tags:
  - homework
  - 2nd-semester
  - 2025-02-24
---

### 3, 6, 7, 11, 14

### 3

$$\begin{gather}
f(x,y) = \frac{x^{3}}{y^{2}}e^{-x^{2}/y}, \ [a; b] = [0; 1], \ y_{0} = 0 \\
\lim_{ y \to 0 } f(x,y) = \frac{x^{3}}{0^{2}} e^{-x^{2}/0} = \begin{bmatrix}
\text{полопиталим}\dots
\end{bmatrix} = 0 \\
\int_{a}^{b} 0 \, dx  = 0 \\
\int_{a}^{b} f(x,y) \, dx = \int_{a}^{b} \frac{x^{3}}{y^{2}}e^{-x^{2}/y} \, dx = \\
= \begin{bmatrix}
t = -\frac{x^{2}}{y} \\
dt = -\frac{2x}{y}dx \\
a \to -\frac{a^{2}}{y} \\
b \to -\frac{b^{2}}{y}
\end{bmatrix} = \\
= -\frac{1}{2}\int_{-a^{2}/y}^{-b^{2}/y} te^{t} \, dt = \\
\end{gather}$$

$$\begin{gather}
= -\frac{1}{2} \left.te^{t}\right|_{-a^{2}/y}^{-b^{2}/y} + \frac{1}{2}\int_{-a^{2}/y}^{-b^{2}/y} e^{t} \, dt = \\
= -\frac{1}{2} \left.\left[ (t-1)e^{t} \right]\right|_{-a^{2}/y}^{-b^{2}/y} = \\
= -\frac{1}{2}\left[ \left( \frac{b^{2}}{y} + 1 \right)e^{-b^{2}/y} - \left( \frac{a^{2}}{y} + 1 \right)e^{-a^{2}/y} \right] = g(y) \\
\lim_{ y \to 0 } g(y) = \begin{bmatrix}
\text{полопиталим}\dots
\end{bmatrix} = 0
\end{gather}$$

$$\begin{gather}
\lim_{ y \to 0 } \int_{a}^{b} f(x,y) \, dx  = \int_{a}^{b} \lim_{ y \to 0 } f(x,y) \, dx - \text{верно}, \text{при} \ y \to +0
\end{gather}$$

### 6

$$\begin{gather}
\lim_{ y \to +\infty } \int_{1}^{2} \frac{\ln(x+y)}{\ln(x^{2}+y^{2})} \, dx = \int_{1}^{2}\lim_{ y \to +\infty }  \frac{\ln(x+y)}{\ln(x^{2}+y^{2})} \, dx = \\
= \int_{1}^{2} \frac{1}{2} \, dx = \left. \frac{1}{2}x \right|_{1}^{2} = \frac{2}{2} - \frac{1}{2} = \frac{1}{2}
\end{gather}$$

### 7

$$\begin{gather}
\lim_{ n \to +\infty } \int_{0}^{1} \frac{dx}{1+\left( 1+\frac{x}{n} \right)^{n}} = \int_{0}^{1} \lim_{ n \to +\infty } \frac{dx}{1+\left( 1+\frac{x}{n} \right)^{n}} = \\
= \int_{0}^{1} \frac{dx}{1+e^{x}} = \begin{bmatrix}
e^{x} = t \\
dt = de^{x} = e^{x}dx \\
0 \mapsto 1 \\
1 \mapsto e
\end{bmatrix} = \int_{1}^{e} \frac{dt}{t(1+t)} = \int_{1}^{e} \left[ \frac{1}{t} - \frac{1}{t+1} \right] \, dt = \\
\end{gather}$$

$$\begin{gather}
= \left[\left. \ln t - \ln (t+1)\right] \right|_{1}^{e} = \ln e - \ln(e+1) -\ln 1 + \ln 2 = \\
= 1 + \ln 2 - \ln(e+1) = \ln \frac{2e}{e+1}
\end{gather}$$

### 11

$$\begin{gather}
F(y) = \int_{-1}^{1} \mathrm{sgn}(x^{2}-y) \  \, dx = \\
= \int_{-1}^{1} f(x,y) \, dx , \\
f(x,y) = \begin{cases}
1, \ x^{2} > y \\
0, \ x^{2} = y \\
-1, \ x^{2} < y \\
\end{cases}
\end{gather}$$

![[2025-02-24 Домашнее задание - НИСФ 2025-02-24 17.11.13.excalidraw]]

### 14

$$\begin{gather}
F(\alpha) = \int_{\alpha}^{2\alpha} \frac{\sin\alpha x}{x} \, dx = \dots \\
\frac{\partial f(x,\alpha)}{\partial \alpha} = \cos\alpha x \\
f(\psi(\alpha), \alpha)\psi'(\alpha) = \frac{2\sin2\alpha^{2}}{\alpha} \\
f(\phi(\alpha), \alpha)\phi'(\alpha) = \frac{\sin\alpha^{2}}{\alpha} \\
\end{gather}$$

$$\begin{gather}
F'(\alpha) = \frac{2\sin2\alpha^{2}}{\alpha} - \frac{\sin\alpha^{2}}{\alpha} + \int_{\alpha}^{2\alpha} \cos \alpha x \, dx 
\end{gather}$$