---
tags:
  - homework
  - 2nd-semester
  - 2025-03-27
---

### 804

$$\begin{gather}
\begin{cases}
\dot{x} = 4x - y - z \\
\dot{y} = x + 2y - z \\
\dot{z} = x - y + 2z
\end{cases} \\
A = \begin{pmatrix}
4 & -1 & -1 \\
1 & 2 & -1 \\
1 & -1 & 2
\end{pmatrix} \\
\lambda_{1} = 2, \ \lambda_{2,3} = 3
\end{gather}$$

$$\begin{gather}
A_{\lambda,\lambda=2} = \begin{pmatrix}
2 & -1 & -1 \\
1 & 0 & -1 \\
1 & -1 & 0
\end{pmatrix} \begin{pmatrix}
1 \\
1 \\
1
\end{pmatrix} = \vec{0} \\
A_{\lambda,\lambda=3} = \begin{pmatrix}
1 & -1 & -1 \\
1 & -1 & -1 \\
1 & -1 & -1
\end{pmatrix} \begin{pmatrix}
1 \\
0 \\
1
\end{pmatrix} = \vec{0} \\
A_{\lambda,\lambda=3} = \begin{pmatrix}
1 & -1 & -1 \\
1 & -1 & -1 \\
1 & -1 & -1
\end{pmatrix} \begin{pmatrix}
1 \\
1 \\
0
\end{pmatrix} = \vec{0}
\end{gather}$$

$$\begin{gather}
J = \begin{pmatrix}
1 & 0 & 0 \\
0 & 1 & 0 \\
0 & 0 & 1
\end{pmatrix}
\end{gather}$$

$$\begin{gather}
\begin{pmatrix}
x \\
y \\
z
\end{pmatrix} = C_{1}e^{2t}\begin{pmatrix}
1 \\
1 \\
1
\end{pmatrix} + e^{3t}\left( C_{2}\begin{pmatrix}
1 \\
1 \\
0
\end{pmatrix} + C_{3}\begin{pmatrix}
1 \\
0 \\
1
\end{pmatrix} \right) 
\end{gather}$$

### 811

$$\begin{gather}
\begin{cases}
\dot{x} = 2x-y-z \\
\dot{y} =2x-y-2z \\
\dot{z} = -x+y+2z
\end{cases} \\
\lambda_{1} = \lambda_{2} = \lambda_{3} = 1 \\
A = \begin{pmatrix}
2 & -1 & -1 \\
2 & -1 & -2 \\
-1 & 1 & 2
\end{pmatrix}
\end{gather}$$

$$\begin{gather}
A_{\lambda,\lambda=1} = \begin{pmatrix}
1 & -1 & -1 \\
2 & -2 & -2 \\
-1 & 1 & 1
\end{pmatrix} \begin{pmatrix}
1 \\
0 \\
1
\end{pmatrix} = \vec{0} \\
A_{\lambda,\lambda=1} = \begin{pmatrix}
1 & -1 & -1 \\
2 & -2 & -2 \\
-1 & 1 & 1
\end{pmatrix} \begin{pmatrix}
1 \\
1 \\
1
\end{pmatrix} = \begin{pmatrix}
-1 \\
-2 \\
1
\end{pmatrix} \\
A_{\lambda,\lambda=1} = \begin{pmatrix}
1 & -1 & -1 \\
2 & -2 & -2 \\
-1 & 1 & 1
\end{pmatrix} \begin{pmatrix}
-1 \\
-2 \\
1
\end{pmatrix} = \begin{pmatrix}
0 \\
0 \\
0
\end{pmatrix} \\

\end{gather}$$