---
tags:
  - homework
  - 2nd-semester
  - 2025-03-04
---

### 2

$$\begin{gather}
F(y) = \int_{0}^{1} f(x,y) \, dx \\
f(x,y) = \begin{cases}
xe^{-x^{2}/y}, \ 0 \leq x \leq 1, \ 0 < y \leq 1 \\
0, \ 0\leq x\leq 1, y = 0
\end{cases} \\
F(y)|_{y=0} = \int_{0}^{1} 0 \, dx = 0 \\
\end{gather}$$

$$\begin{gather}
F(y)|_{0<y\leq 1} = \int_{0}^{1} xe^{-x^{2}/y} \, dx = \\
= -\frac{y}{2}\int_{0}^{1} e^{-x^{2}/y} \, d\left( -\frac{x^{2}}{y} \right) = -\left.\frac{y}{2}e^{-x^{2}/y}\right|_{0}^{1} = -\frac{y}{2}\left( \frac{1}{e^{1/y}} - 1 \right) = \frac{y}{2} - \frac{y}{2e^{1/y}} \\
\end{gather}$$

$$\begin{gather}
F'(y) = \frac{1}{2}\left( 1 - \frac{e^{1/y} + \frac{ye^{1/y}}{y^{2}}}{e^{2/y}} \right) = \frac{1}{2} \left( 1- \frac{1+\frac{1}{y}}{e^{1/y}} \right) \\
F'(0) = \frac{1}{2}\left( 1- \frac{1 + 1}{e^{1/0}} \right)  = \frac{1 - 0}{2}
\end{gather}$$

$$\begin{gather}
F'(0) = \lim_{ y \to +0 } \frac{f(x,y) - f(x,0)}{y} = \lim_{ y \to +0 } \frac{xe^{-x^{2}/y} - 0}{y} = \\
= x\lim_{ y \to +0 }  \frac{e^{-x^{2}/y}}{y} = \left[ \frac{0}{0} \right] = \\
= x^{3}\lim_{ y \to +0 } \frac{e^{-x^{2}/y}\cdot \frac{1}{y^{2}}}{1} = \dots = -\infty \\
\end{gather}$$

$$\begin{gather}
\frac{1}{2} \neq -\infty \implies \text{нет, нельзя}
\end{gather}$$

### 6

$$\begin{gather}
F(a) = \int_{0}^{\pi/2} \frac{\arctan (a\sin x)}{\sin x} \, dx \\
f(x,a) = \frac{\arctan (a\sin x)}{\sin x} \\
\frac{\partial f}{\partial a} = \frac{1}{\sin x}\left( \frac{1}{1+a^{2}\sin ^{2} x} \right) = \frac{1}{\sin x+a^{2}\sin ^{3}x} \\
I'(a) = \int_{0}^{\pi/2} \frac{\sin x}{1 + a^{2}\sin ^{2}x} \, dx  = \\
= \begin{bmatrix}
\sin x = \frac{2t}{1+t^{2}} \\
dx = \frac{2dt}{1+t^{2}} \\
dt = \frac{dx(1+t^{2})}{2} \\
x \in \left[ 0; \frac{\pi}{2} \right] \implies \sin x \in [0; 1] \implies \\
\implies \frac{2t}{1+t^{2}} \in [0; 1] \implies \\
0 \to 0 \\
\frac{\pi}{2} \to 1 \to 1
\end{bmatrix} = \\
\end{gather}$$

$$\begin{gather}
= \int_{0}^{1} \frac{\frac{2t}{1+t^{2}}\cdot \frac{2}{1+t^{2}} \, dt}{1+\frac{a^{2}4t^{2}}{(1+t^{2})^{2}}} = \int_{0}^{1} \frac{4t \, dt}{(1+t^{2})^{2} + a^{2}4t^{2}} = \begin{bmatrix}
t^{2} = u \\
\end{bmatrix} = \\
= 2\int_{0}^{1} \frac{du}{(1+u)^{2} + a^{2}4u } = 2\int_{0}^{1} \frac{du}{u^{2} + 2u + 1 + 4a^{2}u} = \\
= 2\int_{0}^{1} \frac{du}{u^{2} + 2(1+2a^{2})u + 1} = \\
\frac{1}{2\sqrt{ 1+a^{2} }}\int  \, dx 
\end{gather}$$

У меня skissue(

### 9

$$\begin{gather}
I(a) = \int_{0}^{\pi} \frac{\ln(1+a\sin x)}{\sin x} \, dx , \ 0 < a < 1 \\
\frac{\partial f}{\partial a} = \frac{\sin x}{\sin x(1+a\sin x)}  = \frac{1}{1+a\sin x}\\
I'(a) = \int_{0}^{\pi} \frac{1}{1+a\sin x} \, dx  =   \\
I(a) = \int \frac{\pi}{1+a} \, da = \pi\ln(1+a) + C \\
I(0) = 0 \implies C = 0 \\
I(a) = \pi \ln(1+a)
\end{gather}$$

### 15

$$\begin{gather}
\frac{\arctan x}{x} = \int_{0}^{1} \frac{dy}{1+y^{2}x^{2}}, \\
\int_{0}^{1} \frac{\arctan x}{x\sqrt{ 1-x^{2} }} = \int_{0}^{1} \frac{1}{\sqrt{ 1-x^{2} }}dx\int_{0}^{1} \frac{dy}{1+x^{2}y^{2}} = \\
= \int_{0}^{1}\int_{0}^{1} \frac{1}{\sqrt{ 1-x^{2} }(1+x^{2}y^{2})} \, dxdy = \begin{bmatrix}
x = \sin u \\
dx = \cos u du \\

\end{bmatrix} = \\
= \int_{0}^{1}\int_{0}^{\pi/2} \frac{1}{\cos x} \, d(\sin x) \, dy
\end{gather}$$