---
tags:
  - homework
  - 2nd-semester
  - 2025-03-05
---

### 790

$$\begin{gather}
\begin{cases}
\dot{x} = x-3y \\
\dot{y} = 3x + y
\end{cases} \\
A = \begin{pmatrix}
1 & -3 \\
3 & 1
\end{pmatrix} \\
\det (A - \lambda E) = \begin{vmatrix}
1-\lambda & -3 \\
3 & 1-\lambda
\end{vmatrix} = 0 \\
\mathcal{X}_{A}(\lambda) = (1-\lambda)^{2} + 9 = 0 \\
1-\lambda = \pm 3i \\
\lambda_{1,2} = 1\pm 3i
\end{gather}$$

$$\begin{gather}
\begin{pmatrix}
-3i & -3 \\
3 & -3i
\end{pmatrix}\begin{pmatrix}
i \\
1
\end{pmatrix} = \vec{0} \\
\begin{pmatrix}
3i & -3 \\
3 & 3i
\end{pmatrix}\begin{pmatrix}
1 \\
i
\end{pmatrix} = \vec{0} \\
\end{gather}$$

$$\begin{gather}
\begin{cases}
x = C_{1}ie^{1+3i} + C_{2}e^{1-3i} \\
y = C_{1}e^{1+3i} + C_{2}ie^{1-3i} \\
\end{cases} \\
\begin{pmatrix}
x \\
y
\end{pmatrix} = C_{1}\begin{pmatrix}
i \\
1
\end{pmatrix}e^{(1+3i)t} + C_{2}\begin{pmatrix}
1 \\
i
\end{pmatrix}e^{(1-3i)t} \\
\begin{pmatrix}
x \\
y
\end{pmatrix} = C_{1}\begin{pmatrix}
e^{i\pi/2}e^{(1+3i)t} \\
e^{(1+3i)t}
\end{pmatrix} + C_{2}\begin{pmatrix}
e^{(1-3i)t} \\
e^{i\pi/2}e^{(1-3i)t} \\
\end{pmatrix} \\
\begin{pmatrix}
x \\
y
\end{pmatrix} = C_{1}\begin{pmatrix}
e^{t}e^{i(\pi/2 + 3t)} \\
e^{t}e^{3it}
\end{pmatrix} + C_{2}\begin{pmatrix}
e^{t}e^{-3it} \\
e^{t}e^{i(\pi/2-3t)}
\end{pmatrix}
\end{gather}$$

$$\begin{gather}
\begin{pmatrix}
x \\
y
\end{pmatrix} = C_{1}e^{t}\begin{pmatrix}
\cos \left( \frac{\pi}{2} + 3t \right) + i\sin \left( \frac{\pi}{2} + 3t \right) \\
\cos 3t + i \sin 3t
\end{pmatrix} + C_{2}e^{t}\begin{pmatrix}
\cos 3t - i \sin 3t \\
\cos \left( \frac{\pi}{2} - 3t \right) + i\sin \left( \frac{\pi}{2} - 3t \right) \\
\end{pmatrix} \\
\begin{cases}
x = e^{t}(C_{1}\sin 3t - C_{2}\cos 3t) \\
y = e^{t}(C_{1}\cos 3t + C_{2}\sin 3t)
\end{cases}
\end{gather}$$

### 797

$$\begin{gather}
A = \begin{pmatrix}
1 & -2 & -1 \\
-1 & 1 & 1 \\
1 & 0 & -1
\end{pmatrix} \\
\lambda_{1} = 0, \ \lambda_{2} = 2, \ \lambda_{3} = -1 \\
\begin{pmatrix}
1 & -2 & -1 \\
-1 & 1 & 1 \\
1 & 0 & -1
\end{pmatrix} \begin{pmatrix}
1 \\
0 \\
1
\end{pmatrix} = \vec{0} \\
\begin{pmatrix}
-1 & -2 & -1 \\
-1 & -1 & 1 \\
1 & 0 & -3
\end{pmatrix} \begin{pmatrix}
3 \\
-2 \\
1
\end{pmatrix} = \vec{0} \\
\begin{pmatrix}
2 & -2 & -1 \\
-1 & 2 & 1 \\
1 & 0 & 0
\end{pmatrix} \begin{pmatrix}
0 \\
1 \\
-2
\end{pmatrix} = \vec{0} \\
\end{gather}$$

$$\begin{gather}
\begin{pmatrix}
x \\
y \\
z
\end{pmatrix} = C_{1}\begin{pmatrix}
1 \\
0 \\
1
\end{pmatrix} + C_{2}e^{2t} \begin{pmatrix}
3 \\
-2 \\
1
\end{pmatrix} + C_{3}e^{-1} \begin{pmatrix}
0 \\
1 \\
-2
\end{pmatrix}
\end{gather}$$

### 804

$$\begin{gather}
A = \begin{pmatrix}
4 & -1 & -1 \\
1 & 2 & -1 \\
1 & -1 & 2
\end{pmatrix} \\
\lambda_{1} = 2, \ \lambda_{2,3} = 3 \\ 
\begin{pmatrix}
2 & -1 & -1 \\
1 & 0 & -1 \\
1 & -1 & 0
\end{pmatrix}\begin{pmatrix}
1 \\
1 \\
1
\end{pmatrix} = \vec{0} \\
\begin{pmatrix}
1 & -1 & -1 \\
1 & -1 & -1 \\
1 & -1 & -1
\end{pmatrix}\begin{pmatrix}
1 \\
0 \\
1
\end{pmatrix} = \vec{0} \\
\begin{pmatrix}
1 & -1 & -1 \\
1 & -1 & -1 \\
1 & -1 & -1
\end{pmatrix}\begin{pmatrix}
1 \\
1 \\
0
\end{pmatrix} = \vec{0} \\
\end{gather}$$

$$\begin{gather}
\begin{pmatrix}
x \\
y \\
z
\end{pmatrix} = C_{1}e^{2t}\begin{pmatrix}
1 \\
1 \\
1
\end{pmatrix} + e^{3t}\left( C_{2}\begin{pmatrix}
1 \\
0 \\
1
\end{pmatrix} + C_{3}\begin{pmatrix}
1 \\
1 \\
0
\end{pmatrix} \right)
\end{gather}$$

