---
tags:
  - homework
  - 2nd-semester
  - 2025-03-02
---

### 13.110

$$\begin{gather}
w = |z-1|^{2} \\
w = (x-1)^{2} + y^{2} \\
u(x,y) = (x-1)^{2} + y^{2} \\
v(x,y) = 0 \\
\end{gather}$$

$$\begin{gather}
\frac{\partial u}{\partial x} = 2x-2 \\
\frac{\partial u}{\partial y} = 2y \\
\frac{\partial v}{\partial x} = \frac{\partial v}{\partial x} = 0 \\
\begin{cases}
x-1 = 0 \\
y=0
\end{cases} \implies z = 1
\end{gather}$$

### 13.112

$$\begin{gather}
f(z) = e^{3z} = e^{3x+3iy} = e^{3x}e^{3iy} = \\
= e^{3x}(\cos 3y + i\sin 3y) \\
u(x,y) = e^{3x}\cos 3y \\
v(x,y) = e^{3x}\sin 3y \\
\end{gather}$$

$$\begin{gather}
\frac{\partial u}{\partial x} = 3e^{3x}\cos 3y \\
\frac{\partial u}{\partial y} = -3e^{3x}\sin 3y \\
\frac{\partial v}{\partial x} = 3e^{3x}\sin 3y \\
\frac{\partial v}{\partial y} = 3e^{3x}\cos 3y \\
\end{gather}$$

$$\begin{gather}
\begin{cases}
\frac{\partial u}{\partial x} = \frac{\partial v}{\partial y} \\
\frac{\partial u}{\partial y} = -\frac{\partial v}{\partial x} \\
\end{cases} - \text{верно} \\
\end{gather}$$

$$\begin{gather}
f'(z) = \frac{\partial u}{\partial x} + i\frac{\partial v}{\partial x} = 3e^{3x}\left( \cos 3y + i\sin 3x \right)  = \\
= 3e^{3x}e^{3iy} = 3e^{3z}
\end{gather}$$

### 13.116

$$\begin{gather}
f(z) = \mathrm{Ln} \ (z^{2}) = 2\mathrm{Ln} \ z = 2 \left( \ln |z| + i(\mathrm{arg} \ z + 2\pi k) \right) = \dots \\
\end{gather}$$

### 13.133

$$\begin{gather}
u(x,y) = 2xy + 3, \ 0 \le |z| < +\infty \\
\frac{\partial u}{\partial x} = 2y \\
\frac{\partial^{2} u}{\partial x^{2}} = 0 \\
\frac{\partial u}{\partial y} = 2x \\
\frac{\partial^{2} u}{\partial y^{2}} = 0 \\
\end{gather}$$

$$\begin{gather}
\frac{\partial^{2}u}{\partial x^{2}} - \frac{\partial^{2}u}{\partial x^{2}} = 0 - \text{верно} \\
dv = \frac{\partial v}{\partial x}dx + \frac{\partial v}{\partial y}dy = -\frac{\partial u}{\partial y}dx + \frac{\partial u}{\partial x}dy = \\
= -(2x)dx + (2y)dy = \\
= \frac{\partial }{\partial x}(-x^{2})dx + \frac{\partial }{\partial y}(y^{2})dy = \\
= \frac{\partial }{\partial x}(y^{2}-x^{2})dx + \frac{\partial }{\partial y}(y^{2}-x^{2})dy = \\
= d(y^{2}-x^{2})
\end{gather}$$

$$\begin{gather}
v(x,y) = \int d(y^{2}-x^{2}) = y^{2}-x^{2}+C \\
f(z) = 2xy+3 + i(y^{2}-x^{2}) + iC = \\
= i(y^{2} -2xy - x^{2}) + 3 + iC = \\
= -iz^{2} + 3+iC
\end{gather}$$