---
tags:
  - homework
  - 2nd-semester
  - 2024-10-05
---

## 27

$$\begin{gather}
\ln y = ax + by \\
\frac{y'}{y} = a +by' \\
\frac{y''y - (y')^{2}}{y^{2}} = by'' \\
b = \frac{y''y - (y')^{2}}{y''y^{2}} \\
a = \frac{y'}{y} - y'\left( \frac{y''y - (y')^{2}}{y''y^{2}} \right) \\
\ln y = \left( \frac{y'}{y} - y'\left( \frac{y''y - (y')^{2}}{y''y^{2}} \right) \right) x + y\left( \frac{y''y - (y')^{2}}{y''y^{2}} \right) 
\end{gather}$$

## 29

$$\begin{gather}
x = ay^{2}+by+c \\ 
\text{продифференциируем 3 раза по} \ y \\
x' = 2ay + b \\
x'' = 2a \\
x''' = 0 - \text{в x-ах} \\
x_{yyy}''' = x'_{y}(x'_{y}(x_{y}')_{y}')_{y}' = \frac{1}{y'_{x}}\left(\frac{1}{y'_{x}}\left(\frac{1}{y'_{x}}\right)_{x}'\right)_{x}' = \dots = \\
= -\frac{y'_{x}y'''_{xxx} - 3(y''_{xx})^{2}}{(y'_{x})^{5}} \\
y'_{x}y'''_{xxx} - 3(y''_{xx})^{2} = 0 - \text{в y-ах}
\end{gather}$$

## 39

$$\begin{gather}
x^{2} = y + Cx, \ \phi = 90^{\circ} \\
2x = y' + C \implies C = 2x-y' \\
x^{2}= y+x(2x-y') \\
x^{2} = y + 2x^{2} - xy' \\
xy' = y+x^{2} \\
y' = \frac{y}{x} + x \\
-\frac{1}{z'} = \frac{z}{x} + x \\
-x =zz' + x^{2}z' \\
-x = z'(z+x^{2})
\end{gather}$$ 

