---
tags:
  - homework
  - 2nd-semester
  - 2024-09-21
---

## 138

$$\begin{gather}
y' + y\tan x - \sec x = 0 \\
\begin{bmatrix}
y = uv \\
y' = uv' + u'v \\
\end{bmatrix} \\
uv' + u'v + uv\tan x - \sec x = 0 \\
uv' + v(u' + u\tan x) - \sec x = 0 \\
(*) \ u' + u\tan x = 0 \\
\frac{u'}{u} = -\tan x \\
\ln |u| = - \int \frac{\sin x}{\cos x} \, dx \\
\ln |u| = \int \frac{d\cos x}{\cos x} \\
\ln |u| = \ln |\cos x| \\
u = \cos x \\
v'\cos x - \sec x = 0 \\
v' = \sec ^{2}x \\
v = \tan x + C \\
y = uv = \cos x(\tan x + C) \\
y = uv = \sin x + C\cos x \\ 
\end{gather}$$

## 146

$$\begin{gather}
(2e^{y}-x)y' = 1 \\
\begin{bmatrix}
x = uv \\
x' = u'v + uv' \\
\frac{x'_{y}}{y'_{x}} = 1 \implies y' = \frac{1}{x'}
\end{bmatrix} \\
\frac{(2e^{y}-x)}{x'} = 1 \\
2e^{y}-x = x' \\
2e^{y}-uv = uv' + u'v \\
2e^{y}-uv - uv' - u'v = 0 \\
2e^{y}- u(v + v') - u'v = 0 \\
(*) \ v + v' = 0 \\
v' = -v \\
\frac{v'}{v} = -1 \\
\ln |v| = -y \\
v = e^{-y} \\
2e^{y} -u'e^{-y} = 0 \\
u' = \frac{2e^{y}}{e^{-y}} \\
u' = 2e^{2y} \\
u = e^{2y} + C \\
x = uv = e^{-y}(e^{2y} + C) \\
x = e^{y} + Ce^{-y}
\end{gather}$$

## 154

$$\begin{gather}
xy^{2}y' = x^{2} + y^{3} \\
\begin{bmatrix}
y^{3} = t \\
y = t^{1/3} \\
y' = \frac{1}{3}t^{-2/3}t'
\end{bmatrix} \\
xt^{2/3}\cdot \frac{1}{3}t^{-2/3}t' = x^{2} + t \\
\frac{1}{3}xt' = x^{2} + t \\
t' - 3x - \frac{3t}{x} = 0 \\
\begin{bmatrix}
t = uv \\
t' = uv' + u'v
\end{bmatrix} \\
u'v + uv' - 3x - \frac{3}{x} \cdot uv = 0 \\
u'v  - 3x +u\left( v' - \frac{3v}{x} \right) = 0 \\
(*) \ v' - \frac{v}{x} = 0 \\
\frac{v'}{v} = \frac{3}{x} \\
\ln |v| = 3\ln |x| \\
v = x^{3} \\
u'x^{3} - 3x = 0 \\
u' = \frac{3}{x^{2}} \\
u = -\frac{3}{x} + C \\
t = uv = x^{3}\left( -\frac{3}{x}+C \right) \\
y^{3} = Cx^{3} + -3x^{2}
\end{gather}$$

## 155

$$\begin{gather}
xydy = (y^{2} + x)dx \\
xyy' = x + y^{2} \\

\end{gather}$$

## 156

$$\begin{gather}
xy' - 2x^{2}\sqrt{ y } = 4y \\
\begin{bmatrix}
\sqrt{ y } = t \\
y = t^{2} \\
y' = 2t\cdot t'
\end{bmatrix} \\
2xt \cdot t' - 2x^{2} t = t^{2} \ (!), \ y = 0
\end{gather}$$