---
tags:
  - homework
  - 2nd-semester
  - 2024-09-13
---
### 56

$$\begin{gather}
xy'+y=y^{2}; \ y(1) = 0.5 \\
xy'=y^{2} - y \\
\frac{y'}{y^{2}-y} = \frac{1}{x} \\
\int \frac{dy}{\left( y^{2}-y + \frac{1}{4} \right) - \frac{1}{4}} = \int \frac{dx}{x} \\
\int \frac{d\left( y-\frac{1}{2} \right)}{\left( y-\frac{1}{2} \right)^{2} - \frac{1}{4}} = \ln |x| + C \\
\ln \left| \frac{y-\frac{1}{2} - \frac{1}{2}}{y-\frac{1}{2}+\frac{1}{2}}\right| = \ln |x| + C \\
\ln \left| \frac{y-1}{y}\right| = \ln |x| + C \\
\frac{y-1}{y} = Cx \\
1-\frac{1}{y} = Cx \\
\frac{1}{y} = 1 - Cx \\
y = \frac{1}{1 - Cx}, \ y = 0 \\
y(1) = 0.5 \implies \frac{1}{2} = \frac{1}{1-C} \implies \\
\implies C = -1 \implies y = \frac{1}{1+x}
\end{gather}$$

### 59

$$\begin{gather}
e^{-s}\left( 1 + \frac{ds}{dt} \right) = 1 \\
s' = e^{s} - 1 \\
\frac{s'}{e^{s}-1} = 1 \\
\int \frac{ds}{e^{s}-1} = \int dt \\
\int \frac{de^{s}}{e^{2s}-e^{s} + \frac{1}{4} - \frac{1}{4}} = \int dt \\
\int \frac{de^{s}}{\left( e^{s}-\frac{1}{2} \right)^{2} - \frac{1}{4}} = \int dt \\
\ln \left| \frac{e^{s}-1}{e^{s}} \right| = t+C \\
\left| \frac{e^{s}-1}{e^{s}} \right| = e^{t+C} \\
\frac{e^{s}-1}{e^{s}}  = Ce^{t} \\
1-\frac{1}{e^{s}}  = Ce^{t} \\
\frac{1}{e^{s}}  = 1 - Ce^{t} \\
e^{s}  = \frac{1}{1 - Ce^{t}} \\
s  = \ln \left( \frac{1}{1 - Ce^{t}} \right)  \\
s  = -\ln ( 1 - Ce^{t} )  \\
\end{gather}$$

### 109

$$\begin{gather}
xy' - y = (x+y)\ln \frac{x+y}{x} \\
y' = \frac{y}{x} + \frac{x+y}{x}\ln \frac{x+y}{x} \\
y' = \frac{x+y}{x} + \frac{x+y}{x}\ln \frac{x+y}{x} - 1 \\
\begin{bmatrix}
\frac{x+y}{x} = t \\
y = xt-x \\
y' = t + xt' - 1
\end{bmatrix} \\
t + xt' - 1 = t + t\ln t - 1 \\
xt'= t\ln t \\
\frac{t'}{t\ln t} = \frac{1}{x} \ (!) \\
\int \frac{dt}{t\ln t} = \int \frac{dx}{x} \\
\int \frac{d \ln t}{\ln t} = \ln |x| + C \\
\ln |\ln t| = \ln |x| + C \\
\end{gather}$$

$$\begin{gather}
\ln t = Cx \\
t = e^{Ce^{x}} \\
\frac{x+y}{x} = e^{Ce^{x}} \\
1 + \frac{y}{x} = e^{Ce^{x}} \\
y = x(e^{Ce^{x}} - 1), \ y = 0 \\
\end{gather}$$

### 113

$$\begin{gather}
(2x-4y+6)dx + (x+y-3)dy = 0 \\
\begin{cases}
x-2y+3=0 \\
x+y-3=0
\end{cases} \\
\begin{cases}
y = 2 \\
x = 1
\end{cases} \implies \begin{cases}
x = \dot{x} + 1 \\
y = \dot{y} + 2
\end{cases} \\
(2\dot{x}+2-4\dot{y}-8+6)d\dot{x} + (\dot{x}+1+\dot{y}+2-3)d\dot{y} = 0 \\
(2\dot{x}-4\dot{y})d\dot{x} + (\dot{x}+\dot{y})d\dot{y} = 0 \\
\begin{bmatrix}
\dot{y} = t\dot{x} \\
d\dot{y} = \dot{x}dt + td \dot{x}
\end{bmatrix} \\
(2 \dot{x} - 4t \dot{x})d \dot{x} + (\dot{x}+t \dot{x})(\dot{x}dt + td \dot{x}) = 0 \\
\begin{bmatrix}
\dot{x} = 0 \ (x = -1) - \text{не реш.} \\
\end{bmatrix} \\
(2 - 4t)d \dot{x} + (1+t)(\dot{x}dt + td \dot{x}) = 0 \\
(2 - 3t + t^{2})d \dot{x} + (1+t)\dot{x}dt = 0 \\
(t-1)(t-2)d \dot{x} + (1+t)\dot{x}dt = 0 \\ 
-\frac{d\dot{x}}{\dot{x}} = \frac{(t+1)dt}{(t-1)(t-2)} \ (!) \\
\end{gather}$$

$$\begin{gather}
-\frac{1}{\dot{x}} = \frac{(t+1)t'}{(t-1)(t-2)} \\
-\int  \frac{d \dot{x}}{\dot{x}} = \int \frac{(t+1)dt}{(t-1)(t-2)} \\
-\ln |\dot{x}| + C = \int \left(\frac{3}{t-2} - \frac{2}{t-1}\right)dt \\
\ln |\dot{x}| + C = 3\ln |t-2| - 2\ln |t-1| \\
\ln |\dot{x}| + C = \ln \left| \frac{(t-2)^{3}}{(t-1)^{2}} \right| \\
\frac{1}{\dot{x}} = C\frac{(t-2)^{3}}{(t-1)^{2}} \\
1 = C \frac{(\dot{y} - 2 \dot{x})^{3}}{(\dot{y} - \dot{x})^{2}} \\
(y-2x)^{3} = C (y-x-1)^{2}, \ y = x+1, \ y = 2x
\end{gather}$$