---
tags:
  - homework
  - 2nd-semester
  - 2024-11-13
---

### 511

$$\begin{gather}
y'' + y' - 2y = 0 \\
\lambda^{2} + \lambda - 2 = 0 \\
(\lambda - 1)(\lambda + 2) = 0 \\
\lambda_{1} = 1, \ \lambda_{2} = -2 \\
y = C_{1}e^{x} + C_{2}e^{-2x}
\end{gather}$$

### 515

$$\begin{gather}
y'' - 4y' + 5y = 0 \\
\lambda^{2} - 4\lambda + 5 = 0 \\
D = -4, \ \sqrt{ D } = 2i \\
\lambda_{1} = \frac{4 - 2i}{2} = 2-i \\
\lambda_{2} = \frac{4+2i}{2} = 2+i \\
y = C_{1}e^{2x}\cos x + C_{2} e^{2x} \sin x = \\
= e^{2x} (C_{1} \cos x + C_{2} \sin x)
\end{gather}$$

### 518

$$\begin{gather}
y''' - 8y = 0 \\
\lambda^{3} - 8 = 0 \\
(\lambda-2)(\lambda^{2} + 2\lambda + 4) = 0 \\
(\lambda - 2)(\lambda - (-1 - i\sqrt{ 3 }))(\lambda - (-1 + i\sqrt{ 3 })) = 0 \\
\lambda_{1} = 2, \ \lambda_{2,3} = -1 \pm i\sqrt{ 3 } \\
y = C_{1}e^{2x} + e^{-x}(C_{2}\cos (x\sqrt{ 3 }) + C_{3}\sin (x\sqrt{ 3 }))
\end{gather}$$

### 524

$$\begin{gather}
y^{V} -6y^{IV} + 9y''' = 0 \\
\lambda^{3}(\lambda^{2} - 6\lambda + 9) = 0 \\
\lambda^{3}(\lambda - 3)^{2} = 0 \\
\lambda_{1,2,3} = 0, \ \lambda_{4,5} = 3 \\
y = C_{1} + C_{2}x + C_{3}x^{2} + e^{3x}(C_{4} + C_{5}x)
\end{gather}$$

### 613

$$\begin{gather}
y_{1} = x^{2}e^{x} \\
(\lambda - 1)^{3} = 0 \\
\lambda^{3} - 3\lambda^{2} + 3\lambda - 1 = 0 \\
y''' - 3y'' + 3y' - y = 0 \\
y = e^{x}(C_{1} + C_{2}x + C_{3}x^{2}) \\
C_{1} = C_{2} = 0, C_{3} = 1: \ y = x^{2}e^{x} \\
\end{gather}$$

### 691

$$\begin{gather}
xy'' - (x+1)y' -2(x-1)y = 0 \\
y_{1} = e^{ax} \\
y'_{1} = ae^{ax} \\
y''_{1} = a^{2}e^{ax} \\
x(a^{2}e^{ax}) - (x+1)(ae^{ax}) - 2(x-1)e^{ax} = 0 \\
e^{ax}(a^{2}x - a(x+1) - 2(x-1)) = 0 \\
a^{2}x - ax - a - 2x + 2 = 0 \\
x(a^{2} - a - 2) - a + 2 = 0 \\
x(a-2)(a+1) + (a-2) = 0 \\
(a-2)(x(a+1) + 1) = 0 \implies a = 2 \\
\end{gather}$$

$$\begin{gather}
y_{1} = e^{2x} \\
\begin{bmatrix}
y = e^{2x}z \\
y' = e^{2x}(2z + z') \\
y'' = 2e^{2x}(2z + z') + e^{2x}(2z' + z'') =  \\
= e^{2x}(4z + 4z' + z'') 
\end{bmatrix}
\end{gather}$$

$$\begin{gather}
xe^{2x}(4z + 4z' + z'') - (x+1)e^{2x}(2z+z') -2(x-1)e^{2x} = 0 \\
x(4z + 4z' + z'') - (x+1)(2z+z') -2(x-1)z = 0 \\
\underbrace{4xz - (x+1)2z -2(x-1)z}_{0} + 4xz' + xz'' - xz' - z' = 0 \\
-\frac{z''}{z'} = \frac{4x - x - 1}{x} \\
\frac{z''}{z'} = \frac{-3x + 1}{x} \\
\frac{z''}{z'} = -3 + \frac{1}{x} \\
\end{gather}$$

$$\begin{gather}
\begin{bmatrix}
z' = u \\
z'' = u'
\end{bmatrix} \\
\frac{u'}{u} = -3 + \frac{1}{x} \\
\ln |u| = -3x + \ln |x| + \ln |C_{1}| \\
u = e^{-3x + \ln |x| + \ln |C_{1}|} \\
z' = C_{1}xe^{-3x} \\
z = C_{1}\int xe^{-3x} \, dx \\
z = -\frac{C_{1}}{9}(e^{-3x}(3x+1) + C_{2}) \\
z = C_{1}e^{-3x}(3x+1) + C_{2} \\
y = C_{1}e^{-x}(3x+1) + C_{2}e^{2x}
\end{gather}$$

### 525

$$\begin{gather}
y^{V} - 10y''' + 9y' = 0 \\
\lambda^{5} - 10\lambda^{3} + 9\lambda = 0 \\
\lambda(\lambda^{4} - 10\lambda^{2} + 9) = 0 \\
\lambda(\lambda^{2} - 1)(\lambda^{2} - 9) = 0 \\
\lambda_{1} = 0, \ \lambda_{2,3} = \pm 1, \ \lambda_{4,5} = \pm 3 \\
y = C_{1} + e^{x}C_{2} + e^{-x}C_{3} + e^{3x}C_{4} + e^{-3x}C_{5}
\end{gather}$$

### 528

$$\begin{gather}
y''' - y'' -y' + y = 0 \\ 
\lambda^{3} - \lambda^{2} - \lambda + 1 = 0 \\
(\lambda-1)(\lambda^{2} -1) = 0 \\
(\lambda-1)^{2}(\lambda+1) = 0 \\
\lambda_{1,2} = 1, \ \lambda_{3} = -1 \\
y = e^{x}(C_{1} + C_{2}x) + e^{-x}C_{3} \\
\end{gather}$$

### 530

$$\begin{gather}
y^{V} + 8y''' + 16y' = 0 \\
\lambda^{5} +8\lambda^{3} + 16\lambda = 0 \\
\lambda(\lambda^{4} + 8\lambda^{2} + 16 ) = 0 \\
\lambda(\lambda^{2} + 4)^{2} = 0 \\
\lambda(\lambda - 2i)^{2}(\lambda + 2i)^{2} = 0 \\
\lambda_{1} = 0, \ \lambda_{2,3} = 2i, \ \lambda_{4,5} = -2i \\
y = C_{1} + (C_{1} + C_{2}x)\cos 2x + (C_{3} + C_{4}x)\sin 2x
\end{gather}$$