---
tags:
  - seminar
  - 2nd-semester
  - 2025-02-14
---

## Решение систем дифф. уравнений

$$\begin{gather}
\begin{cases}
\dot{x} = 3x+y \\
\dot{y} = -x+y
\end{cases} \\
\begin{cases}
y = \dot{x} - 3x \\
\dot{y} = \dot{x} - 4x
\end{cases} \\
\begin{cases}
\dot{y} = \ddot{x} - 3\dot{x} \\
\dot{y} = \dot{x} - 4x
\end{cases} \\
\ddot{x} - 3\dot{x} = \dot{x} - 4x
\end{gather}$$

$$\begin{gather}
\ddot{x} - 4\dot{x} + 4x = 0 \\
A = \begin{pmatrix}
3 & 1 \\
-1 & 1
\end{pmatrix}, \ \mathrm{Tr} \ A = 4, \ \mathrm{dct} \ A = 4 \\
\ddot{x} - \mathrm{Tr} \ A \cdot \dot{x} + \mathrm{dct} \ A \cdot x = 0 \\
\end{gather}$$

$$\begin{gather}
\lambda^{2} - 4\lambda + 4 = 0 \\
(\lambda - 2)^{2} = 0 \\
x = e^{2t}(C_{1}t + C_{2}) \\
y = 2C_{1}e^{2t} - 3e^{2t}(C_{1}t+C_{2}) \\
y = \dots
\end{gather}$$

### Решение уравнений в симметричной форме записи

$$\begin{gather}
\frac{a_{1}}{b_{1}} = \frac{a_{2}}{b_{2}} = \dots = \frac{a_{n}}{b_{n}} = L \\
\frac{a_{1}k_{1} + a_{2}k_{2} +\dots+ a_{n}k_{n}}{b_{1}k_{1}+b_{2}k_{2}+\dots+b_{n}k_{n}} = L \\
a_{i} = Lb_{i} \\
\frac{b_{1}k_{1}L + b_{2}k_{2}L + \dots + b_{n}k_{n}L}{a_{1}k_{1}+a_{2}k_{2}+\dots+a_{n}k_{n}} = 1
\end{gather}$$

$$\begin{gather}
\frac{dx}{y-u} = \frac{dy}{z-x} = \frac{dz}{u-y} = \frac{du}{x-z} \\
\frac{dx+dy+dz+du}{y-u+z-x+u-y+x-z} = L \\
\frac{d(x+y+z+u)}{0} = L \\
d(x+y+z+u) = 0 \\
\end{gather}$$

$$\begin{gather}
x+y+z+u = C_{1} \\
\frac{dx+dz}{y-u+u-y} = 0 \\
d(x+z) = 0 \\
x+z = C_{1} \\
\frac{dy+du}{x-z+z-x} = 0 \\
d(y+u) = 0 \\
y+u = C_{2} \\
\end{gather}$$

$$\begin{gather}
xdx = \frac{1}{2}d(x^{2}) \\
\frac{xdx+ydy+zdz+udu}{x(y-u)+y(z-x)+z(u-y)+u(x-z)} = L \\
\frac{1}{2}\cdot \frac{d(x^{2}) + d(y^{2}) + d(z^{2}) + d(u^{2})}{0} = L \\
d(x^{2}+y^{2}+z^{2}+u^{2}) = 0 \\
x^{2}+y^{2}+z^{2}+u^{2} = C_{3}
\end{gather}$$

$$\begin{gather}
\begin{cases}
x+z = C_{1} \\
y+u = C_{2} \\
x^{2}+y^{2}+z^{2}+u^{2} = C_{3}
\end{cases}
\end{gather}$$

### Сюжет какой-то

$$\begin{gather}
\begin{cases}
\frac{dx}{dt} = y^{2} + \sin t \\
\frac{dy}{dt} = \frac{x}{2y} \\
\end{cases} \\
\begin{cases}
x = 2y\dot{y} = \frac{d}{dt}y^{2} \\
\dot{x} = y^{2} + \sin t \\
\end{cases} \\
\dot{x} = \frac{d^{2}}{dt^{2}}y^{2} = y^{2} + \sin t \\
\ddot{(y^{2})} - y^{2} - \sin t = 0 \\
y^{2} = u \\
\ddot{u} - u = \sin t \\
\lambda^{2} - 1 = 0 \\
(\lambda-1)(\lambda+1)=  0 \\
u_{оо} = C_{1}e^{t} + C_{2}e^{-t} \\
u_{он} = C_{1}e^{t} + C_{2}e^{-t} -\frac{1}{2}\sin t \\
\end{gather}$$