---
tags:
  - seminar
  - 2nd-semester
  - 2025-05-02
---


### 961

$$\begin{gather}
y' = \frac{2x+y}{3x+4y} \\
\frac{\dot{y}}{\dot{x}} = \frac{2x+y}{3x+4y} \\
\begin{cases}
\dot{x} = 3x+4y \\
\dot{y} = 2x+y \\
\end{cases} \\
\lambda_{1} = 5, \ \lambda_{2} = -1 \\
\vec{x}_{1} = \begin{pmatrix}
-1 \\
1
\end{pmatrix}, \ \vec{x}_{2} = \begin{pmatrix}
2 \\
1
\end{pmatrix} \\
\end{gather}$$

![[2025-05-02 Семинар - СГВМ 2025-05-02 09.56.50.excalidraw]]

### 962

$$\begin{gather}
\begin{cases}
\dot{y} = x-4y \\
\dot{x} = 2y-3x \\
\end{cases} \\
A = \begin{pmatrix}
-3 & 2 \\
1 & -4 \\
\end{pmatrix} \\
\lambda^{2} + 7\lambda + 10 = 0 \\
\lambda_{1} = -2, \ \lambda_{2} = -5 \\
\vec{x}_{1} = \begin{pmatrix}
2 \\
1
\end{pmatrix}, \ \vec{x}_{2} = \begin{pmatrix}
1 \\
-1
\end{pmatrix}
\end{gather}$$

![[2025-05-02 Семинар - СГВМ 2025-05-02 10.13.31.excalidraw]]

### 963

$$\begin{gather}
y' =  \frac{y-2x}{y}
\begin{cases}
\dot{x} = y \\
\dot{y} = y-2x
\end{cases} \\
A = \begin{pmatrix}
0 & 1 \\
-2 & 1
\end{pmatrix} \\
\det (A - \lambda E) = \left( \lambda-\frac{1}{2} \right)^{2} + \frac{7}{2} = 0 \\
\lambda_{1,2} = \frac{1}{2} \pm \frac{i\sqrt{ 7 }}{2} \\
\end{gather}$$

![[2025-05-02 Семинар - СГВМ 2025-05-02 10.19.34.excalidraw]]