---
tags:
  - seminar
  - 2nd-semester
  - 2025-04-18
---
## Фазовые траектории

$$\begin{gather}
\begin{cases}
\dot{x} = f_{1}(x,y) \\
\dot{y} = f_{2}(x,y)
\end{cases}
\end{gather}$$

$$\begin{gather}
\frac{dy}{dx} = \frac{f_{2}(x,y)}{f_{1}(x,y)} \\
\ddot{x} = f(x, \dot{x}) \\
\begin{cases}
\dot{x} = y \\
\dot{y} = \ddot{x} = f(x, y)
\end{cases}
\end{gather}$$

### 1005

$$\begin{gather}
\ddot{x} = -2x^{3} \\
\begin{cases}
\dot{x} = y \\
\dot{y} = -2x^{3}
\end{cases}
\end{gather}$$ 

$$\begin{gather}
\frac{dy}{dx} = -\frac{2x^{3}}{y} \\
\frac{ydy}{dx} = -2x^{3} \\
\frac{y^{2}}{2} = -\frac{x^{4}}{2} + C \\
y^{2} = -x^{4} + C \\
x^{4} + y^{2} = C
\end{gather}$$

![[2025-04-18 Семинар - СГВМ 2025-04-18 09.07.09.excalidraw]]

### 1013

$$\begin{gather}
\ddot{x} - \dot{x} - 2x = 0 \\
\ddot{x} = \dot{x} + 2x \\
\begin{cases}
\dot{x} = y \\
\dot{y} = y + 2x
\end{cases}
\end{gather}$$

$$\begin{gather}
\frac{dy}{dx} = \frac{y + 2x}{y} \\
y' = 1 + \frac{2x}{y} \\
\begin{bmatrix}
y = xz \\
z = \frac{y}{z} \\
y' = xz' + z
\end{bmatrix} \\
\frac{zdz}{z^{2} -z - 2} = -\frac{dx}{x} \\
\frac{z}{z^{2} - z - 2} = \frac{z}{(z-2)(z+1)} = \frac{\frac{1}{3}}{z+1} + \frac{\frac{2}{3}}{z-2}
\end{gather}$$

$$\begin{gather}
\frac{1}{3}\left( \int  \frac{dz}{z+1} + 2\int \frac{2dz}{z-2} \right)  = -\int \frac{dx}{x}  \\
\ln |z+1| + 2\ln |z-2| = -3\ln |x| - \ln C \\
\ln (z+1)(z-2)^{2} = \ln \frac{1}{Cx^{3}} \\
(z+1)(z-2)^{2} = Cx^{-3} \\
x^{3}(yx-2)^{2}(yx+1) = C \\
(y-2x)^{2}(y+x) = C \\
\xi_{1}^{2}\xi_{2} = C \\
\xi_{2} = \frac{C}{\xi_{1}^{2}}
\end{gather}$$

![[2025-04-18 Семинар - СГВМ 2025-04-18 09.53.50.excalidraw]]

### 1006

$$\begin{gather}
\ddot{x} + 2x^{3} - 2x = 0 \\
\begin{cases}
\dot{x} = y \\
\dot{y} = 2x-2x^{3}
\end{cases} \\
\frac{dy}{dx} = \frac{2x-2x^{3}}{y} \\
y'y = 2x-2x^{3} \\
\frac{y^{2}}{2} = x^{2} - \frac{x^{4}}{2} + C \\
y^{2} = 2x^{2} - x^{4} + C \\
x^{4} - 2x^{2} + y^{2} = C \\
(x^{2} - 1)^{2} + y^{2} = C + 1 \\
(x^{2} - 1)^{2} + y^{2} = \tilde{C} \\
\end{gather}$$

![[Pasted image 20250418102611.png]]