---
tags:
  - seminar
  - 2nd-semester
  - 2025-03-14
---

### 1

$$\begin{gather}
\begin{cases}
\dot{x} = 12x-6y-2z \\
\dot{y} = 18x - 9y - 3z \\
\dot{z} = 18x-9y-3z
\end{cases}
\end{gather}$$

$$\begin{gather}
\begin{cases}
\dot{x} = x-3y+3z \\
\dot{y} = -2x - 6y +13z \\
\dot{z} = -x-4y+8z
\end{cases} \\
A = \begin{pmatrix}
1 & -3 & 3 \\
-2 & -6 & 13 \\
-1 & -4 & 8
\end{pmatrix} \\
-\lambda^{3} + \lambda^{2}\mathrm{Tr} \ A - \lambda\sum_{i} M_{ii} + \det A = \\
= -\lambda^{3} + 3\lambda^{2} - 3\lambda + 1 \\
\end{gather}$$

$$\begin{gather}
\lambda^{3} - 3\lambda^{2} + 3\lambda - 1 = 0 \\
(\lambda-1)^{3} = 0 \\
\end{gather}$$

$$\begin{gather}
A_{\lambda, \lambda=1}: \  \begin{pmatrix}
0 & -3 & 3 \\
-2 & -7 & 13 \\
-1 & -4 & 7
\end{pmatrix}\begin{pmatrix}
3 \\
1 \\
1
\end{pmatrix} = \vec{0} \\
A_{\lambda, \lambda=1}: \  \begin{pmatrix}
0 & -3 & 3 \\
-2 & -7 & 13 \\
-1 & -4 & 7
\end{pmatrix}\begin{pmatrix}
1 \\
1 \\
1
\end{pmatrix} =  \\
\begin{pmatrix}
1 & 1 & 0 \\
0 & 1 & 1 \\
0 & 0 & 1
\end{pmatrix}
\end{gather}$$

$$\begin{gather}
\begin{pmatrix}
1 \\
1 \\
1
\end{pmatrix}, \ \begin{pmatrix}
0 \\
2 \\
1
\end{pmatrix}, \ \begin{pmatrix}
3 \\
1 \\
1
\end{pmatrix}
\end{gather}$$

$$\begin{gather}
P = \begin{pmatrix}
-6 & 0 & 1 \\
-2 & 4 & 1 \\
-2 & 2 & 1
\end{pmatrix}\\
J = \begin{pmatrix}
1 & 1 & 0 \\
0 & 1 & 1 \\
0 & 0 & 1
\end{pmatrix}
\end{gather}$$

$$\begin{gather}
C_{1}e^{t}\begin{pmatrix}
3 \\
1 \\
1
\end{pmatrix} + C_{2}e^{t}\begin{pmatrix}
3t \\
t-2 \\
t-1
\end{pmatrix} + C_{3}e^{t}\begin{pmatrix}
\frac{3}{2}t^{2} + 1 \\
\frac{t^{2}}{2}-2t \\
\frac{t^{2}}{2} - t
\end{pmatrix}
\end{gather}$$

### 2

$$\begin{gather}
A = \begin{pmatrix}
12 & -6 & -2 \\
18 & -9 & -3 \\
18 & -9 & -3
\end{pmatrix} \\
\begin{pmatrix}
1 \\
2 \\
0
\end{pmatrix}, \ \begin{pmatrix}
0 \\
1 \\
-3
\end{pmatrix}, \ \begin{pmatrix}
0 \\
0 \\
-1
\end{pmatrix}
\end{gather}$$

$$\begin{gather}
h_{0},h_{1},\dots,h_{k} \sim \lambda \\
\vec{\phi_{1}} = e^{\lambda t}\vec{h}_{0} \\
\vec{\phi_{2}}= e^{\lambda t}(\vec{h}_{0}t + \vec{h}_{1}) \\
\vec{\phi_{3}}= e^{\lambda t}\left( \frac{\vec{h}_{0}t^{2}}{2} + \vec{h}_{1}t + \vec{h}_{2} \right)
\end{gather}$$

$$\begin{gather}
\Phi(t) = C_{1} = \begin{pmatrix}
0 \\
1 \\
-3
\end{pmatrix} + C_{2} \begin{pmatrix}
2 \\
3 \\
3
\end{pmatrix} + C_{3}\begin{pmatrix}
2t \\
3t \\
3t-1
\end{pmatrix}
\end{gather}$$

