---
tags:
  - типовой-расчет
  - 2nd-semester
  - 06-04-2024
---

# ТР 2

### Ершов Алексей Геннадьевич КМБО-03-23

### Вариант 4

#### 4.2(а)

$$\begin{gather}
\int _{0}^{2}(2+x^{2})\sqrt{ 4x-x^{2} } \, dx = \int _{0}^{2}(2+((x-2)+2)^{2}) \sqrt{ 2^{2}-(x-2)^{2} }d(x-2) = \\
= \begin{bmatrix}
x-2 = 2\sin t \\
t = \arcsin \frac{x-2}{2} \\
d(x - 2) = 2\cos t \, dt
\end{bmatrix} = \int_{-\frac{\pi}{2}}^{0} (2 + (2\sin t + 2)^{2})\sqrt{ 2^{2} - 2^{2}\sin ^{2}t } \cdot 2\cos t\,dt = \\
= 4\int _{-\frac{\pi}{2}}^{0} (4\sin ^{2}t + 8\sin t + 6)\cos ^{2} t\, dt = \\
= 4 \int _{-\frac{\pi}{2}}^{0} [\sin ^{2} 2t + 8 \sin t \cos ^{2} t + 6 \cos ^{2}t]\, dt = \\
= 2\int _{-\frac{\pi}{2}}^{0} [1 - \cos 4t + 8 \sin t(1 + \cos 2t) + 6(1+\cos 2t)] \, dt = \\ 
= 2\int _{-\frac{\pi}{2}}^{0} [1 - \cos 4t + 8 \sin t + 8\sin t\cos 2t + 6 + 6\cos 2t] \, dt = \\ 
= 2\int _{-\frac{\pi}{2}}^{0} [1 - \cos 4t + 8 \sin t + 4\sin 3t - 4\sin t + 6 + 6\cos 2t] \, dt = \\ 
= 2\int _{-\frac{\pi}{2}}^{0} [7 +4\sin t + 4\sin 3t + 6\cos 2t - \cos 4t] \, dt = \\ 
= 2\left[ 7t -4\cos t -\frac{4}{3}\cos 3t + 3\sin 2t -\frac{1}{4}\sin 4t \right] \Big|_{-\frac{\pi}{2}}^{0} = \\
= 2\left( -4-\frac{4}{3} \right) - 2\left( -\frac{7\pi}{2} \right) = 7\pi - \frac{32}{3}
\end{gather}$$

#### 4.2(б)

$$\begin{multline}
\int_{1}^{1.5} \frac{(x+2)^{3}}{\sqrt{ (2x-x^{2})^{5} }} \, dx = \int_{1}^{1.5} \frac{((x-1)+3)^{3}}{\sqrt{ (1-(x-1)^{2})^{5} }} \, d(x-1) = \\
= \begin{bmatrix}
x-1 = \sin t \\
t = \arcsin(x-1) \\
d(x-1) = \cos t\,dt
\end{bmatrix} = \int_{0}^{\pi/6} \frac{(\sin t+3)^{3}}{\sqrt{ (1-\sin^{2}t)^{5} }} \cos t \, dt = \\
= \int_{0}^{\pi/6} \frac{(\sin t+3)^{3}}{\cos ^{4}t} \, dt = \int_{0}^{\pi/6} \frac{\sin ^{3}t + 9\sin ^{2} t + 27\sin t + 27}{\cos ^{4}t} \, dt = \\
= \underbrace{\int_{0}^{\pi/6} \frac{\sin ^{3}t}{\cos^{4} t} \, dt}_{I_{1}} + 9\underbrace{\int_{0}^{\pi/6} \frac{\sin ^{2}t}{\cos^{4} t} \, dt}_{I_{2}} + 27\underbrace{\int_{0}^{\pi/6} \frac{\sin t}{\cos^{4} t} \, dt}_{I_{3}} + 27\underbrace{\int_{0}^{\pi/6} \frac{1}{\cos^{4} t} \, dt}_{I_{4}} = \\
= \frac{88\sqrt{ 3 }-54}{27} + 9\cdot \frac{\sqrt{ 3 }}{9} + 27 \cdot \frac{160\sqrt{ 3 }-135}{27} + 27 \cdot \frac{10\sqrt{ 3 }}{27} = \\
= \frac{88\sqrt{ 3 }}{27} - 2 + \sqrt{ 3 } + 160\sqrt{ 3 } - 135 + 10\sqrt{ 3 } = \\
= \frac{(88+171\cdot 27) \sqrt{ 3 } - 137 \cdot 27}{27} = \\
= \frac{4705\sqrt{ 3 } - 3699}{27}
\end{multline}$$

$$\begin{multline}
I_{1} = \int_{0}^{\pi/6} \frac{\sin ^{3}t}{\cos^{4} t} \, dt = -\int_{0}^{\pi/6} \frac{\sin ^{2}t \, d\cos t}{\cos^{4} t} = \\
= -\int_{0}^{\pi/6} \left[ \frac{d\cos t}{\cos^{4} t} - \frac{\cos ^{2}t \, d\cos t}{\cos^{4} t} \right] = \int_{0}^{\pi/6} \frac{d\cos t}{\cos ^{2}t} - \int_{0}^{\pi/6} \frac{d\cos t}{\cos ^{4}t} = \\
= \left[ \frac{5}{\cos ^{5}t} - \frac{3}{\cos ^{3}t } \right] \Big|_{0}^{\pi/6} = \left( \frac{5}{\frac{9\sqrt{ 3 }}{32}} - \frac{3}{\frac{3\sqrt{ 3 }}{8}} \right) - (5-3) = \\
= \frac{160 - 72}{9\sqrt{ 3 }} - 2 = \frac{88\sqrt{ 3 }}{27} - 2 = \\
= \frac{88\sqrt{ 3 } - 54}{27}
\end{multline}$$

$$\begin{multline}
I_{2} = \int_{0}^{\pi/6} \frac{\sin^{2} t}{\cos^{4} t} \, dt = \int_{0}^{\pi/6} \tan^{2}t \, d\tan t = \frac{\tan^{3}t}{3} \Big|_{0}^{\pi/6} = \left( \frac{3\sqrt{ 3 }}{27} \right) - 0 = \\
= \frac{\sqrt{ 3 }}{9}
\end{multline}$$

$$\begin{multline}
I_{3} = \int_{0}^{\pi/6} \frac{\sin t}{\cos^{4} t} \, dt = -\int_{0}^{\pi/6} \frac{d\cos t}{\cos^{4} t} = \frac{5}{\cos ^{5}t} \Big|_{0}^{\pi/6} = \\
= \frac{5}{\frac{9\sqrt{ 3 }}{32}} - 5 = \frac{160}{9\sqrt{ 3 }} - 5 = \frac{160\sqrt{ 3 }}{27} - 5 = \\
= \frac{160\sqrt{ 3 } - 135}{27}
\end{multline}$$

$$\begin{multline}
I_{4} = \int_{0}^{\pi/6} \frac{1}{\cos^{4} t} \, dt = \begin{bmatrix}
u = \frac{1}{\cos ^{2}t} \\
dv = \frac{1}{\cos ^{2}t}dt \\
du = \frac{2\sin t}{\cos ^{3}t} \\
v = \tan t
\end{bmatrix} = \frac{\tan t}{\cos ^{2}t} \Big|_{0}^{\pi/6} - 2\int \frac{\tan^{2}t}{\cos^{2}t} \, dt  = \\
= \frac{\tan t}{\cos ^{2}t} \Big|_{0}^{\pi/6} - 2\int \tan^{2}t \, d\tan t = \left[\frac{\tan t}{\cos ^{2}t}  - \frac{2\tan^{3}t}{3}\right]\Big|_{0}^{\pi/6} = \\
= \left( \frac{\frac{\sqrt{ 3 }}{3}}{\frac{3}{4}} - \frac{\frac{6\sqrt{ 3 }}{27}}{3} \right) - 0 = \frac{4\sqrt{ 3 }}{9} - \frac{2\sqrt{ 3 }}{27} = \\
= \frac{10\sqrt{ 3 }}{27}
\end{multline}$$
