---
tags:
  - типовой-рассчет
  - 2nd-semester
  - 18-03-2024
  - матан
---

# ТР 1

## Ершов Алексей Геннадьевич КМБО-03-23

### Вариант 4

## 1.4.a)

$$\int x^{2}\ln(x^{2}+2x+5) \, dx$$

$$\begin{gather}
\int x^{2}\ln(x^{2}+2x+5) \, dx = \frac{x^{3}}{3}\ln(x^{2}+2x+5) - \int \frac{x^{3}}{3} \cdot \frac{2x+2}{x^{2}+2x+5} \, dx = \\
= \frac{x^{3}\ln(x^{2}+2x+5)}{3} - \frac{2}{3} \underbrace{\int \frac{x^{4}+x^{3}}{x^{2}+2x+5} \, dx}_{(1)} = \dots = \\
= \frac{x^{3}\ln(x^{2}+2x+5)}{3} + \frac{x^{3}}{3}-\frac{x^{2}}{2}-3x+\frac{11}{2}\ln |x^{2}+2x+5| + \\
+ 2\arctan \frac{x+1}{2} + C
\end{gather}$$

$$\begin{gather}
(1): \int \frac{x^{4}+x^{3}}{x^{2}+2x+5} \, dx = \int \left[ (x^{2}-x-3) + \frac{11x+15}{x^{2}+2x+5} \right] \, dx = \\
= \frac{x^{3}}{3} - \frac{x^{2}}{2} - 3x + \underbrace{\int \frac{5.5(2x+2) + 4}{x^{2}+2x+5} \, dx}_{(2)} = \dots = \\
= \frac{x^{3}}{3}-\frac{x^{2}}{2}-3x+\frac{11}{2}\ln |x^{2}+2x+5| + 2\arctan \frac{x+1}{2} + C
\end{gather}$$

$$\begin{gather}
(2): \frac{11}{2}\int \frac{2x+2}{x^{2}+2x+5} \, dx + 4\int \frac{dx}{x^{2}+2x+5} = \frac{11}{2}\int \frac{d(x^{2}+2x+5)}{x^{2}+2x+5} + \\
+ 4\int \frac{dx}{(x+1)^{2} + 2^{2}} = \frac{11}{2}\ln |x^{2}+2x+5| + 2\arctan \frac{x+1}{2} + C
\end{gather}$$

## 1.4.б)

$$\int \frac{-x^{4}+5x^{3}-7x^{2}+11x-16}{(x-1)(x+1)^{2}(x^{2}-4x+5)} \, dx$$

$$\begin{gather}
\int \frac{-x^{4}+5x^{3}-7x^{2}+11x-16}{(x-1)(x+1)^{2}(x^{2}-4x+5)} \, dx = \\
= \int \underbrace{\left[\frac{A}{x-1} + \frac{B}{x+1} + \frac{C}{(x+1)^{2}} + \frac{Dx + E}{x^{2}-4x+5}\right]}_{(1)} \, dx = \\
\end{gather}$$

$$\begin{gather}
= -\int \frac{1}{x-1} \, dx + 2\int \frac{1}{(x+1)^{2}} \, dx + \int \frac{1}{x^{2}-4x+5} \, dx = \\
=-\ln |x-1| - \frac{2}{x+1} + C + \int \frac{1}{(x-2)^{2}+1^{2}} \, dx = \\
= -\ln |x-1| - \frac{2}{x+1} + \arctan(x-2) + C
\end{gather}$$

$$\begin{gather}
(1): \ \frac{-x^4+5 x^3-7 x^2+11 x-16}{(x-1) (x+1)^2 \left(x^2-4 x+5\right)}= \\
= \frac{A}{x-1}+\frac{B}{x+1}+\frac{C}{(x+1)^{2}}+\frac{Dx + E}{x^{2}-4x+5}
\end{gather}$$

$$\begin{gather}
-x^{4}+5x^{3}-7x^{2}+11x-16 = \\
= A(x+1)^{2}(x^{2}-4x+5) + B(x-1)(x+1)(x^{2}-4x+5) + \\
+ C(x-1)(x^{2}+4x-5) + (Dx+E)(x-1)(x+1)^{2}
\end{gather}$$  

$$\begin{gather}
-x^4+5 x^3-7 x^2+11 x-16=5 A-5 B-5 C-E+ \\
+\left(A+B+D\right) x^4+\left(-2 A-4 B+C+D+E\right) x^3+ \\
\left(-2 A+4 B-5 C-D+E\right) x^2+\left(6 A+4 B+9 C-D-E\right) x
\end{gather}$$

$$\begin{array}{c}
-16=5 A-5 B-5 C-E \\
11=6 A+4 B+9 C-D-E \\
-7=-2 A+4 B-5 C-D+E \\
5=-2 A-4 B+C+D+E \\
-1=A+B+D
\end{array}$$

$$\begin{gather}
\left(
\begin{array}{ccccc}
 5 & -5 & -5 & 0 & -1 \\
 6 & 4 & 9 & -1 & -1 \\
 -2 & 4 & -5 & -1 & 1 \\
 -2 & -4 & 1 & 1 & 1 \\
 1 & 1 & 0 & 1 & 0
\end{array}
\right)\left(
\begin{array}{c}
 A \\
 B \\
 C \\
 D \\
 E
\end{array}
\right) =\left(
\begin{array}{c}
 -16 \\
 11 \\
 -7 \\
 5 \\
 -1
\end{array}
\right)
\end{gather}$$

$$\begin{gather}
\left(\begin{array}{ccccc|c}
 5 & -5 & -5 & 0 & -1 & -16 \\
 6 & 4 & 9 & -1 & -1 & 11 \\
 -2 & 4 & -5 & -1 & 1 & -7 \\
 -2 & -4 & 1 & 1 & 1 & 5 \\
 1 & 1 & 0 & 1 & 0 & -1
\end{array}\right)
\end{gather}$$

После преобразований приходим к данной системе:

$$\left(
\begin{array}{ccccc|c}
 1 & 0 & 0 & 0 & 0 & -1 \\
 0 & 1 & 0 & 0 & 0 & 0 \\
 0 & 0 & 1 & 0 & 0 & 2 \\
 0 & 0 & 0 & 1 & 0 & 0 \\
 0 & 0 & 0 & 0 & 1 & 1
\end{array}
\right) \implies \begin{cases}
A = -1 \\
B = 0 \\
C = 2 \\
D = 0 \\
E = 1
\end{cases}$$

Откуда следует, что

$$\begin{gather}
\frac{-x^4+5 x^3-7 x^2+11 x-16}{(x-1) (x+1)^2 \left(x^2-4 x+5\right)}= \\
= -\frac{1}{x-1}+\frac{2}{(x+1)^{2}}+\frac{1}{x^{2}-4x+5}
\end{gather}$$
