---
tags:
  - типовой-расчет
  - 2nd-semester
  - 16-05-2024
---

## Ершов Алексей Геннадьевич КМБО-03-23

### Вариант 4

## 9.4

$$\begin{gather}
a = \{ (1-y)x; yz; z \} \\
\sigma : (2-z)^{2} = x^{2} + y^{2}, \ z = 0
\end{gather}$$

![[scan_2024-05-23_11-53-42.jpg|50%]]

## а)

$$\begin{gather}
\sigma : x^{2} + y^{2} - (z-2)^{2} = 0, \ z = 0 \\
\iint_{\sigma} = \iint_{\sigma_{1}} + \iint_{\sigma_{2}} \\
\sigma_{1} : z = 0, x^{2} + y^{2} = 4 \\
\iint_{\sigma_{1}} (1-y)x \, dydz + yz \, dxdz + z \, dxdy = \begin{bmatrix}
\vec{N}_{\sigma_{1}} = \{ 0, 0, -1 \}
\end{bmatrix} = \\
= -\left.\iint_{D_{xy}} z\,dxdy\right|_{z = 0} = -0\iint_{D_{xy}}dxdy = 0 \\
\end{gather}$$

$$\begin{gather}
\iint_{\sigma_{2}} (1-y)x \, dydz + yz \, dxdz + z \, dxdy = \\
= \begin{bmatrix}
F : z = \sqrt{ x^{2}+y^{2} } + 2 \\
\vec{N}_{\sigma_{2}} = \frac{1}{\sqrt{ (F'_{x})^{2} + (F'_{y})^{2} + 1 }}\{ -z'_{x}; -z'_{y}; 1 \} = \\
= \frac{1}{\sqrt{ \frac{x^{2}}{x^{2}+y^{2}} + \frac{y^{2}}{x^{2}+y^{2}} + 1 }}\left\{ -\frac{x}{\sqrt{ x^{2}+y^{2} }}; -\frac{y}{\sqrt{ x^{2}+y^{2} }}; 1 \right\} = \\
= \frac{\sqrt{ 2 }}{2}\left\{ -\frac{x}{\sqrt{ x^{2}+y^{2} }}; -\frac{y}{\sqrt{ x^{2}+y^{2} }}; 1 \right\}
\end{bmatrix} = \\
= \frac{\sqrt{ 2 }}{2} \left.\iint_{D_{xy}} \left[ \frac{x^{2}(1-y)}{\sqrt{ x^{2}+y^{2} }} + \frac{y^{2}z}{\sqrt{ x^{2}+y^{2} }} + z \right] \, dxdy\right|_{z = \sqrt{ x^{2} + y^{2} } + 2} = \\
= \frac{\sqrt{ 2 }}{2} \iint_{D_{xy}} \left[ \frac{x^{2}(1-y)}{\sqrt{ x^{2}+y^{2} }} + \frac{y^{2}(\sqrt{ x^{2} + y^{2} } + 2)}{\sqrt{ x^{2}+y^{2} }} + \sqrt{ x^{2} + y^{2} } + 2 \right] \, dxdy = \\
= \frac{\sqrt{ 2 }}{2} \iint_{D_{xy}} \left[ \frac{2x^{2}-x^{2}y+3y^{2}}{\sqrt{ x^{2}+y^{2} }} + y^{2} + 2 \right] \, dxdy = \\
= \begin{bmatrix}
x = \rho \cos \phi \\
y = \rho \sin \phi \\
\rho = \sqrt{ x^{2}+y^{2} } \\
|J| = \rho
\end{bmatrix} =
\end{gather}$$

$$\begin{gather}
= \frac{\sqrt{ 2 }}{2} \int_{0}^{2\pi} \, d\phi \int_{0}^{2} \rho \left[ \frac{2\rho^{2}\cos^{2} \phi - \rho^{3}\cos^{2} \phi \sin \phi  + 3\rho^{2}\sin^{2} \phi}{\rho} + \rho^{2} \sin^{2} \phi + 2 \right]  \, d\rho = \\
= \frac{\sqrt{ 2 }}{2} \int_{0}^{2\pi} \, d\phi \int_{0}^{2} \left[ 2\rho^{2}\cos^{2} \phi - \rho^{3}\cos^{2} \phi \sin \phi  + 3\rho^{2}\sin^{2} \phi + \rho^{3} \sin^{2} \phi + 2\rho \right]  \, d\rho = \\
= \frac{\sqrt{ 2 }}{2} \int_{0}^{2\pi} \, d\phi \int_{0}^{2} \left[ \rho^{3}(\cos^{2} \phi \sin \phi + \sin^{2} \phi) + \rho^{2}(\underbrace{2\cos^{2} \phi + 3\sin^{2} \phi}_{\sin^{2} \phi + 2}) + 2\rho \right]  \, d\rho = \\
= \frac{\sqrt{ 2 }}{2} \int_{0}^{2\pi} \left[ \frac{2^{4}}{4}(\cos^{2} \phi \sin \phi + \sin^{2} \phi) + \frac{2^{3}}{3}(\sin^{2} \phi + 2) + 2^{2} \right]  \, d\phi = 
\end{gather}$$

$$\begin{gather}
= \frac{2\sqrt{ 2 }}{3} \int_{0}^{2\pi} \left[ 3(\cos^{2} \phi \sin \phi + \sin^{2} \phi) + 2(\sin^{2} \phi + 2) + 3 \right]  \, d\phi = \\
= \frac{2\sqrt{ 2 }}{3} \int_{0}^{2\pi} \left[ 3\cos^{2} \phi \sin \phi + 5\sin^{2} \phi + 7 \right]  \, d\phi = \\
= \frac{\sqrt{ 2 }}{3} \int_{0}^{2\pi} \left[ 3(\cos 2\phi + 1)\sin \phi + 5(1 - \cos 2\phi) + 14 \right]  \, d\phi = \\
= \frac{\sqrt{ 2 }}{3} \int_{0}^{2\pi} \left[ 3\cos 2\phi \sin \phi + 3\sin \phi - 5\cos 2\phi + 19\right]  \, d\phi =
\end{gather}$$

$$\begin{gather}
= \frac{\sqrt{ 2 }}{3} \int_{0}^{2\pi} \left[ \frac{3}{2}\sin 3\phi - \frac{3}{2}\sin \phi + 3\sin \phi - 5\cos 2\phi + 19\right]  \, d\phi = \\
= \frac{\sqrt{ 2 }}{6} \int_{0}^{2\pi} \left[ 3\sin 3\phi - 10\cos 2\phi  + 3\sin \phi + 38\right]  \, d\phi = \\
= \frac{\sqrt{ 2 }}{6} \left.\left[ -\cos 3\phi - 5\sin 2\phi - 3\cos \phi + 38\phi \right]\right|_{0}^{2\pi} = \\
= \frac{76\sqrt{ 2 }}{6} = \frac{38\sqrt{ 2 }}{3}
\end{gather}$$

$$\begin{gather}
\iint_{\sigma} = \iint_{\sigma_{1}} + \iint_{\sigma_{2}} = 0 + \frac{264\pi}{5} = \frac{264\pi}{5}
\end{gather}$$

## б) (по т. Гаусса-Остроградского)

$$\iint_{\sigma} P\,dydz + Q\,dxdz + R\,dxdy = \iiint_{V}(\underbrace{P_{x}' + Q_{y}' + R_{z}'}_{\mathrm{div} \ \vec{a}})\,dxdydz$$

$$\begin{gather}
\iint_{\sigma} (1-y)x \, dydz + yz \, dxdz + z \, dxdy = \iiint_{V} \left( 1-y + z + 1 \right) \, dxdydz = \\
= \iiint_{V} (2-y+z)\, dxdydz = \int_{-2}^{2}  \, dx \int_{-\sqrt{ 4-x^{2} }}^{\sqrt{ 4-x^{2} }}  \, dy \int_{0}^{\sqrt{ x^{2}+y^{2} }+2} (2-y+z) \, dz = \\
= \int_{-2}^{2}  \, dx \int_{-\sqrt{ 4-x^{2} }}^{\sqrt{ 4-x^{2} }} \left( (2-y)(\sqrt{ x^{2}+y^{2} }+2)+\frac{(\sqrt{ x^{2}+y^{2} }+2)^{2}}{2} \right) \, dy = \\
= \int_{0}^{2\pi} \, d\phi \int_{0}^{2} \rho\left( (2-\rho\sin \phi)(\rho+2)  + \frac{\rho^{2} + 4\rho + 4}{2} \right)  \, d\rho = \\
= \int_{0}^{2\pi} \, d\phi \int_{0}^{2} \frac{1}{2}\left( (1-2\sin \phi)\rho^{3} + (8-4\sin \phi)\rho^{2} + 12\rho \right) \, d\rho = \\
= \frac{1}{2}\int_{0}^{2\pi} \left.\left( (1-2\sin \phi) \frac{\rho^{4}}{4} + (8-4\sin \phi) \frac{\rho^{3}}{3} + 12 \frac{\rho^{2}}{2} \right)\right|_{0}^{2} \, d\phi = \\
= \frac{1}{2}\int_{0}^{2\pi} \left( 4(1-2\sin \phi)  + \frac{8}{3}(8-4\sin \phi) + 24 \right) \, d\phi = \\
= \int_{0}^{2\pi} \left( 2(1-2\sin \phi)  + \frac{4}{3}(8-4\sin \phi) + 12 \right) \, d\phi = \\
= \frac{1}{3}\int_{0}^{2\pi} \left( 74 - 28\sin \phi \right) \, d\phi = \frac{1}{3} \left. \left( 74\phi + 28\cos \phi \right) \right|_{0}^{2\pi} = \\
= \frac{148\pi}{3}
\end{gather}$$
