## 10.4

$$
\vec{a} = \{ y;xy;-z \}, \ 
\Gamma = x+y+z=2, \left[\begin{align}
&x=0 \\
&z=0 \\
&y=0
\end{align}\right.
$$

![[scan_2024-05-23_12-49-56.jpg]]

## 10.4(а)

$$\begin{gather}
\oint_{\Gamma} y\,dx + xy\,dy -z\,dz \\
\oint_{\Gamma} = \oint_{\Gamma_{1}} + \oint_{\Gamma_{2}} + \oint_{\Gamma_{3}}
\end{gather}$$

$$\begin{gather}
\oint_{\Gamma_{1}} = \begin{bmatrix}
F : y = 2-x \implies x = 2-y \\
y = t, \ 
x = 2-t, \ 
z = 0 \\
t \in [0;2] \\
dx = -dt \\
dy = dt \\
dz = 0
\end{bmatrix} = \int_{0}^{2} \left(-t + t(2-t) \right)\,dt = \\
= \int_{0}^{2} \left( -t^{2} + t \right) \, dt = -\frac{8}{3} + 2 = -\frac{2}{3}
\end{gather}$$

$$\begin{gather}
\oint_{\Gamma_{2}} = \begin{bmatrix}
F : z = 2-x \\
x = t, \
z = 2-t, \
y = 0 \\
t \in [0;2] \\
dx = dt \\
dy = 0 \\
dz = -dt
\end{bmatrix} = \int_{0}^{2} \left( 2-t \right)  \, dt = 4 - 2 = 2
\end{gather}$$

$$\begin{gather}
\oint_{\Gamma_{3}} = \begin{bmatrix}
F : z = 2-y \\
y = t, \
z = 2-t, \
x = 0 \\
t \in [0; 2] \\
dx = 0 \\
dy = dt \\
dz = -dt
\end{bmatrix} = \int_{0}^{2} (t-2) \, dt = \\
= -\int_{0}^{2} (2-t) \, dt = -\oint_{\Gamma_{2}} = -2
\end{gather}$$

$$\begin{gather}
\oint_{\Gamma} = -\frac{2}{3} + 2 - 2 = -\frac{2}{3}
\end{gather}$$

## 10.4(б) (по т. Стокса)

$$\begin{gather}
\oint_{\Gamma} (\vec{a}, d\vec{r}) = \iint_{\sigma} (\mathrm{rot} \ \vec{a}, \vec{n}) \,d\sigma \\
\mathrm{rot} \ \vec{a} = \begin{vmatrix}
\vec{i} & \vec{j} & \vec{k} \\
\frac{ \partial  }{ \partial x } & \frac{ \partial  }{ \partial y } & \frac{ \partial  }{ \partial z } \\
y & xy & -z
\end{vmatrix} = \vec{i} \cdot 0 - \vec{j} \cdot 0 + \vec{k} \cdot (y-1) = \{ 0; 0; y-1 \} \\
\vec{n} = \{ 1; 1; 1 \} \ (\text{смотрит на нас}) \\
\iint_{\sigma} (\mathrm{rot} \ \vec{a}, \vec{n}) \, d\sigma = \iint_{\sigma} (y-1) \, d\sigma = \\
= \int_{0}^{2} \, dx \int_{0}^{2-x} (y-1) \, dy = \frac{1}{2}\int_{0}^{2} (-2x+x^{2}) \, dx = -\frac{2}{3}
\end{gather}$$
