---
tags:
  - seminar
  - 2nd-semester
  - 2024-09-18
---

## 136

$$\begin{gather}
xy' - 2y = 2x^{4} \\
y' - \frac{2y}{x} = 2x^{3} \\
\begin{bmatrix}
y = uv \\
y' = u'v + uv'
\end{bmatrix} \\
u'v + uv' - \frac{2uv}{x} = 2x^{3} \\
u'v + u\left(  v' - \frac{2v}{x} \right) = 2x^{3} \\
v' - \frac{2v}{x} = 0 \\
\frac{v'}{v} = \frac{2}{x} \\
\ln |v| = 2\ln |x| + \ln |C| \\
v = Cx^{2} \\
C'x^{2} = 2x^{3} \\
C' = 2x \\
C = x^{2} + \tilde{C} \\
y = x^{4} + \tilde{C}x^{2}
\end{gather}$$

## 147

$$\begin{gather}
(\sin ^{2}y + x\cot y)y' = 1 \\
\sin ^{2}y + x\cot y = \frac{1}{y'} \\
\sin ^{2}y + x\cot y = x' \\
x = uv \\
x = u'v+uv' \\
\sin ^{2}y + \cot y = x' \\
\end{gather}$$