---
tags:
  - seminar
  - 2nd-semester
  - 2024-11-13
---
$$a_{0}(x)y^{(n)} + a_{1}(x)y^{(n-1)} + \dots + a_{n}(x)y = f(x)$$

$y_{он} = y_{оо} + y_{чн}$
фср: $\phi_{1}, \dots, \phi_{n}$ 
$y_{оо} = c_{1}\phi_{1} + \dots + c_{n}\phi_{n}, \ c_{i} = const$
$y_{он} = c_{1}(x)\phi_{1} + \dots + c_{n}(x)\phi_{n}$

$$\begin{cases}
c_{1}'\phi_{1} + \dots + c_{n}'(x)\phi_{n} = 0 \\
c_{1}'\phi_{1}' + \dots + c_{n}'(x)\phi_{n}' = 0 \\
\dots \\
c_{1}'(x) \phi^{(n-1)}_{1} + \dots + c_{n}'(x)\phi^{(n-1)}_{n} = \frac{f(x)}{a_{0}(x)}
\end{cases}$$

$y_{он} = c_{1}(x)\phi_{1} + \dots + c_{n}(x)\phi_{n}$
$y_{он}' = c_{1}\phi_{1}' + \dots + c_{n}(x)\phi'_{n} + \underbrace{c_{1}'(x)\phi_{1} + \dots + c_{n}'(x)\phi_{n}}_{0}$
$y_{он}'' = c_{1}(x)\phi''_{1} + \dots + c_{n}(x)\phi_{n}'' + \underbrace{c_{1}(x)'\phi_{1}' + \dots + c_{n}'(x)\phi_{n}'}_{0}$
...
$y_{он}^{(n)} = c_{1}(x)\phi_{1}^{(n)} + \dots + c_{n}\phi^{(n)}_{n} + c_{1}'\phi_{1}^{(n-1)} + \dots + c_{n}'\phi_{n}^{(n-1)}$
$a_{0}(x)(c_{1}'\phi_{1}^{(n-1)} + \dots + c_{n}\phi_{n}^{(n-1)}) = f(x)$

### 575

$$\begin{gather}
y''-2y'+y = \frac{e^{x}}{x} \\
y'' - 2y'  + y = 0 \\
\lambda^{2} - 2\lambda + 1 = 0 \\
(\lambda - 1)^{2} = 0 \\
\phi_{1}(x) = e^{x}, \ \phi_{2}(x) = xe^{x} \\
y_{оо} = C_{1}e^{x} + C_{2}xe^{x}, \ C_{1},C_{2} = const \\
y_{он} = C_{1}(x)e^{x} + C_{2}(x)xe^{x} \\
\end{gather}$$

$$\begin{gather}
\begin{cases}
C_{1}'(x) e^{x} + C_{2}'(x)xe^{x} = 0 \\
C_{1}'(x) e^{x} + C_{2}'(x)(e^{x} + xe^{x}) = 0
\end{cases}
\end{gather}$$