---
tags:
  - seminar
  - 2nd-semester
  - 2024-12-04
---

$$F(p) = \frac{3}{p^{2}}\cdot \frac{1+e^{-4p}}{1-e^{-4p}} - \frac{3}{2p^{3}}$$

$$\begin{gather}
f(t) = -\frac{3}{4}(t^{2}-4t)\theta(t) + \frac{3}{4}(t^{2}-4t)\theta(t-4) \\
t^{n}\theta(t) \fallingdotseq \frac{n!}{p^{n+1}} \\
f(t) = F(p) \\
f(t-\tau) \fallingdotseq e^{-p\tau}F(p)
\end{gather}$$

$$\begin{gather}
-\frac{3}{4}t^{2}\theta(t)+3t\theta(t) + \frac{3}{4}(t-4+4)(t-4)\theta(t-4) = \\ 
= -\frac{3}{4}t^{2}\theta(t)+3t\theta(t) + \frac{3}{4}(t-4)^{2}\theta(t-4)+3(t-4)\theta(t-4) \fallingdotseq \\ 
\fallingdotseq -\frac{3}{2p} 
\end{gather}$$