---
tags:
  - seminar
  - 2nd-semester
  - 2024-09-11
---
### 53

$$\begin{gather}
(x^{2}-1)y' + 2xy^{2}=0, \ y(0) = 1 \\
\frac{y'}{y^{2}} = -\frac{2x}{x^{2}-1} \\
\int \frac{dy}{y^{2}} = -\int \frac{dx^{2}}{x^{2}-1} \\
\frac{1}{y} = \ln |x^{2}-1| + C \\
y = \frac{1}{\ln |x^{2}-1| + C}, \ C = 1 \\
y = \frac{1}{\ln |x^{2}-1| + 1}
\end{gather}$$

### 51

$$\begin{gather}
xydx+(x+1)dy = 0 \\
xy+(x+1)y' = 0 \\
\frac{dy}{dx} = -\frac{xy}{x+1} \\
\frac{dx}{dy} = -\frac{x+1}{xy} \\
\frac{y'}{y} = -\frac{x}{x+1} \\
\int \frac{dy}{y} = -\int \frac{xdx}{x+1} \\
\ln |y| = -\int \frac{(x + 1 - 1)dx}{x+1} \\
\ln |y| = -x \int \frac{(x + 1 - 1)dx}{x+1} \\
\end{gather}$$