---
tags:
  - seminar
  - 2nd-semester
  - 2024-11-20
---


## Уранение эйлера
### 589

$$\begin{gather}
x^{2}y'' - 4xy' + 6y = 0 \\
\begin{bmatrix}
x = e^{t} \\
y(t(x)) \\
1 = e^{t}t'_{x} \implies t'_{x} = e^{-t} \\
y'_{x} = y'_{t}t'_{x} = y'_{t}e^{-t} \\
y''_{x} = (y''_{x}e^{-t})'_{t}t'_{x} = (y''_{t}e^{-t} - y'_{t}e^{-t})e^{-t} = e^{-2t}(y''_{t} - y'_{t}) \\
\end{bmatrix} \\
e^{2t} e^{-2t}(y''_{t}-y'_{t})-4e^{t}y'_{t}e^{-t} + 6y = 0 \\
y''_{t} - y'_{t} - 4y'_{t} + 6y = 0 \\
y''_{t} - 5y'_{t} + 6y = 0 \\
\alpha^{2} - 5\alpha + 6 = 0 \\
(\alpha - 2)(\alpha - 3) = 0 \\
\alpha_{1} = 2, \ \alpha_{2} = 3 \\
\phi_{1} = e^{2t}, \ \phi_{2} = e^{3t} \\
y_{оо} = c_{1}e^{2t} + c_{2}e^{3t} \\
y_{оо} = c_{1}x^{2} + c_{2}x^{3} \\
\end{gather}$$

$$\begin{gather}
a_{0}x^{n}y^{(n)}+a_{1}x^{n-1}y^{(n-1)}+\dots+a_{n}y = 0 \\
a_{i} = const \\
\end{gather}$$

