---
tags:
  - seminar
  - 2nd-semester
  - 2025-02-18
---

### Основные элементарные функции комплексной переменной



$$\begin{gather}
e^{z} = e^{x+iy} = e^{x}(\cos y + i \sin y) \\
\cos z = \frac{e^{iz}+e^{-iz}}{2} \\
\sin z = \frac{e^{iz} - e^{-iz}}{2i} \\
\cosh z = \frac{e^{z} + e^{-z}}{2} \\
\sinh z = \frac{e^{z} - e^{-z}}{2} \\
\mathrm{Ln} z  = \ln |z| + i (\mathrm{arg} \ z + 2\pi k), k \in \mathbb{Z} \\
a^{z} = e^{z\mathrm{Ln} \ a} \\
z^{a} = e^{a\mathrm{Ln} \ z} \\
\frac{1}{i} = -i
\end{gather}$$

### 1. Доказать, что 

1. $\sin iz = i\sinh z$
2. $\cos iz = \cosh z$
3. $\tan iz = i\tanh z$
4. $\cot iz = -i\coth z$

$$\begin{gather}
\sin iz = \frac{e^{-z}- e^{z}}{i2} = -\frac{1}{i}\frac{e^{z} - e^{-z}}{2} = -\frac{1}{i} \sinh z = i\sinh z \\
\cos iz = \frac{e^{-z} + e^{z}}{2} = \cosh z \\
\tan iz = \frac{e^{-z}-e^{z}}{e^{-z}+e^{z}} = \frac{\sin iz}{\cos iz} = \frac{i\sinh z}{\cosh z} = i\tanh z \\
\coth iz = \frac{\cos iz}{\sin iz} = \frac{\cosh z}{i\sinh z} = -i\coth z
\end{gather}$$

### 2. Выделить $\mathrm{Re} \ w, \ \mathrm{Im} \ w$

$$\begin{gather}
w = e^{1-z} = e^{1 - \mathrm{Re}\ z - i\mathrm{Im} \ z} = e^{1-\mathrm{Re} \ z}(\cos (-\mathrm{Im} \ z) + i \sin (-\mathrm{Im} \ z)) = \\
= e^{1-\mathrm{Re} \ z}(\cos \mathrm{Im} \ z - i \sin \mathrm{Im} \ z) \\
\mathrm{Re} \ w = e^{1-\mathrm{Re}\ z}\cos \mathrm{Im} \ z \\
\mathrm{Im} \ w = -e^{1-\mathrm{Re}\ z}\sin \mathrm{Im} \ z
\end{gather}$$

$$\begin{gather}
\mathrm{Re} \ z = x, \ \mathrm{Im} \ z = y \\
w = \sin z = \frac{e^{iz} + e^{-iz}}{2i} = \frac{e^{i(x+iy)}+e^{-i(x+iy)}}{2i} = \frac{e^{ix-y} + e^{y - ix}}{2i} = \\
= \frac{1}{2i}\left( e^{-y}e^{ix} + e^{y}e^{-ix} \right) = \\
= \frac{1}{2i}\left( \frac{1}{e^{y}}\left( \cos x + i \sin x \right) + e^{y}\left( \cos x-i\sin x \right) \right) = \\
= \frac{1}{2i}\left[ \left( e^{-y} + e^{y} \right)\cos x + i(e^{-y} - e^{y}) \sin x \right] = \\
=\frac{1}{2}(e^{-y} - e^{y}) \sin x +\frac{i}{2}\left( e^{-y} + e^{y} \right)\cos x =
\end{gather}$$

$$\begin{gather}
= \cosh y\sin x + i\sinh y\cos x
\end{gather}$$

$$\begin{gather}
\sin z = \sin(x+iy) = \sin x \cosh y + i\cos x\sinh y
\end{gather}$$

> [!important] Важный результат
> $$\sin z = \sin(x+iy) = \sin x \cosh y + i\cos x\sinh y$$

$$\begin{gather}
w = \tan z = \frac{\sin z}{\cos z} = \frac{e^{i(x+iy)} - e^{-i(x+iy)}}{2i}\cdot \frac{2}{e^{i(x+iy)} + e^{-i(x+iy)}} = \\
= -i\cdot \frac{e^{-y}e^{ix} - e^{y}e^{-ix}}{e^{-y}e^{ix} + e^{y}e^{-ix}} = -i\cdot \frac{e^{2i(x+iy)} - 1}{e^{2i(x+iy)} + 1} = \\
= -i\cdot \frac{(e^{2ix-2y} - 1)(e^{-2ix-2y} + 1)}{(e^{2ix-2y} + 1)(e^{-2ix-2y} + 1)} = \\
= -i\cdot \frac{e^{-4y}+e^{2ix-2y}-e^{-2ix+2y}-1}{e^{-4y}+e^{2ix-2y} + e^{-2ix-2y}+1} = \\
\end{gather}$$

$$\begin{gather}
= -i\cdot \frac{e^{-2y} + 2i\sin 2x -e^{2y}}{e^{-2y} + 2\cos 2x + e^{2y}} = \\
= -i\cdot \frac{-2\sinh 2y + 2i\sin 2x}{2\cosh 2y + 2\cos 2x} = \\
= \frac{i\sinh 2y + \sin 2x}{\cosh 2y+ \cos 2x} \\
u(x,y) = \frac{\sin 2x}{\cosh 2y+ \cos 2x} \\
v(x,y) = \frac{\sinh 2y}{\cosh 2y+ \cos 2x}
\end{gather}$$

### 3. Вычислить

$$\begin{gather}
\cot\left(  \frac{\pi}{4} - i \ln 2 \right) = \frac{\cos \left( \frac{\pi}{4} - i \ln 2 \right)}{\sin \left( \frac{\pi}{4} - i \ln 2 \right)} = \\
= i\cdot \frac{e^{i(\pi/4-i\ln 2)} + e^{-i(\pi/4 - i\ln 2)}}{e^{i(\pi/4-i\ln 2)} - e^{-i(\pi/4 - i\ln 2)}} = \\
= i\cdot \frac{e^{2i(\pi/4-i\ln 2)} + 1}{e^{2i(\pi/4-i\ln 2)} - 1} = \dots \\

\end{gather}$$

$$\begin{gather}
e^{2i(\pi/4-i\ln 2)} = e^{i\pi/2 + \ln 4} = e^{i\pi/2}e^{\ln 4} = \\
= 4i \\
\dots = i \frac{4i + 1}{4i - 1} = \frac{4-i}{1-4i} = \frac{(4-i)(1+4i)}{17} = \frac{8 + 15i}{17}
\end{gather}$$

### 4. Найти все значения степени

$$\begin{gather}
(1+i)^{i} = e^{i\mathrm{Ln} \ (1+i)} = e^{i}e^{\mathrm{Ln} \ (i+1)} = \\
= e^{i\ln (\sqrt{ 2 } + i (\pi/4 + 2\pi k))} = e^{i\ln \sqrt{ 2 }}e^{-(\pi/4+2\pi k)} = \\
= e^{-\pi/4+2\pi k}(\cos\ln \sqrt{ 2 } + i \sin \ln \sqrt{ 2 })
\end{gather}$$

$$\begin{gather}
\arcsin z = ? \\
z = \sin w \iff z = \frac{e^{iw}-e^{-iw}}{2i} \\
2ize^{iw} = e^{2iw} - 1 \\
t = e^{iw} \\
2izt = t^{2} - 1 \\
t^{2} - 2izt - 1 = 0 \\
D = 4i^{2}z^{2} + 4 = 4-4z^{2} \implies \sqrt{ D } = 2iz \\
t_{1,2} = \frac{2iz \pm 2iz}{2} \implies \begin{cases}
t_{1} = 0 \\
t_{2} = 2iz
\end{cases} \\
\end{gather}$$

$$\begin{gather}
e^{iw} = 2iz \implies 
\end{gather}$$