---
tags:
  - seminar
  - 2nd-semester
  - 2025-04-15
---

### Дз: 270

$$\begin{gather}
\oint_{|z| = \frac{1}{2}} \frac{1}{z^{3}} \cos \frac{\pi}{z+1} \\
f' = \frac{\pi}{(z+1)^{2}} \sin \frac{\pi}{z+1} \\
f'' = \pi \cdot \frac{-\pi \cos \frac{\pi}{z + 1} - 2(z+1)\sin \frac{\pi}{z+1}}{(z+1)^{4}} \\
f''(0) = \pi (-\pi(-1) - 0) = \pi^{2} \implies I = \pi i\pi^{2} = \pi^{3}i
\end{gather}$$

## Ряд Лорана

### Найти все разложения $f(z)$ в ряд Лорана по степеням $(z-z_{0})$

$$f(z) = \frac{1}{(z-2)(z+3)}, \ z_{0} = 2$$

![[2025-04-15 Семинар - ТФКП 2025-04-15 14.36.00.excalidraw]]

$$\begin{gather}
D_{1}: 0 < |z-2| < 5 \\
D_{2}: |z-2| > 5
\end{gather}$$

$$\begin{gather}
D_{1}: \ f(z) = \frac{1}{5(z-2)} - \frac{1}{5(z+3)} \\
\frac{1}{z+3} = \frac{1}{(z-2) + 5} = \frac{1}{5\left( 1+\frac{z-2}{5} \right)} = \\
= \frac{1}{5}\sum_{n=0}^{\infty} (-1)^{n} \left( \frac{z-2}{5} \right)^{n} = \sum_{n=1}^{\infty} \frac{(-1)^{n}(z-2)^{n}}{5^{n+1}} \\
f(z) = \frac{1}{5(z-2)} + \sum_{n=0}^{\infty} \frac{(-1)^{n}(z-2)^{n}}{5^{n+1}}
\end{gather}$$

$$\begin{gather}
D_{2}: \ \frac{1}{z+3} = \frac{1}{z-2 + 5} = \frac{1}{(z-2)\left( 1 + \frac{5}{z-2} \right)} = \frac{1}{z-2}\sum_{n=0}^{\infty} (-1)^{n} \left( \frac{5}{z-2} \right)^{n} = \\
= \sum_{n=0}^{\infty} (-1)^{n}\cdot \frac{5^{n}}{(z-2)^{n+1}} \\
f(z) = \frac{1}{5(z-2)} + \sum_{n=0}^{\infty} \frac{(-1)^{n+1}5^{n-1}}{(z-2)^{n+1}} = \\
= \frac{1}{5(z-2)} - \frac{1}{5(z-2)} + \sum_{n=1}^{\infty} \frac{(-1)^{n+1}5^{n-1}}{(z-2)^{n+1}} = \sum_{n=1}^{\infty} \frac{(-1)^{n+1}5^{n-1}}{(z-2)^{n+1}} = \\
= \begin{bmatrix}
n+1 = k
\end{bmatrix} = \sum_{k=2}^{\infty} \frac{(-1)^{k}5^{n-2}}{(z-2)^{k}}
\end{gather}$$

### 2

$$\begin{gather}
f(z) = \frac{1}{(z-2)(z+3)}, \ z_{0} = 0 \\
\end{gather}$$

![[2025-04-15 Семинар - ТФКП 2025-04-15 14.45.41.excalidraw]]

$$\begin{gather}
D_{1}: |z| < 2 \\
D_{2}: 2 < |z| < 3 \\
D_{3}: |z| > 3 \\
\end{gather}$$

$$\begin{gather}
D_{1}: \ f(z) = \frac{1}{5(z-2)} - \frac{1}{5(z+3)} = \frac{1}{10}\cdot \frac{1}{-\frac{z}{2} + 1} - \frac{1}{15} \cdot \frac{1}{\frac{z}{3} + 1} = \dots \\
(I) = -\frac{1}{10}\sum_{n=0}^{\infty} \left( \frac{z}{2} \right)^{n} \\
(II) = \frac{1}{15}\sum_{n=0}^{\infty} (-1)^{n}\left( \frac{z}{3} \right)^{n} \\
\end{gather}$$

$$\begin{gather}
f(z) = \sum_{n=1}^{\infty} \left( \frac{1}{15}\left( \frac{-1}{3} \right)^{n} - \frac{1}{10}\left( \frac{1}{2} \right)^{n} \right)z^{n}
\end{gather}$$

$$\begin{gather}
D_{2}: \ f(z) = \dots = \sum_{n=0}^{\infty} \frac{2^{n}}{5z^{n+1}} + \sum_{n=0}^{\infty} \frac{(-1)^{n+1}}{15\cdot 3^{n}}z^{n}
\end{gather}$$

$$\begin{gather}
D_{3}: f(z) = \dots = \sum_{n=0}^{\infty} \left( \frac{2^{n}}{5} + \frac{(-1)^{n+1}3^{n}}{5} \right) \frac{1}{z^{n+1}}
\end{gather}$$

### 4

$$\begin{gather}
f(z) = \frac{1}{(z-3)^{2}}, \ z_{0} = 1 \\
D_{1}: |z-1| < 2  \\
D_{2}: |z-1| > 2 \\
\end{gather}$$

$$\begin{gather}
D_{1} = f(z) = \frac{1}{(z-3)^{2}} = \left( -\frac{1}{z-3} \right)' = \left( -\frac{1}{(z-1)-2} \right)' = \left( \frac{1}{2\left( 1-\frac{z-1}{2} \right)} \right)' = \\
= \left( \frac{1}{2}\sum_{n=0}^{\infty} \frac{(z-1)^{n-1}}{2^{n}} \right)' = \\
= \sum_{n=}^{\infty} \frac{n(z-1)^{n-1}}{2^{n+1}} = \begin{bmatrix}
k = n-1
\end{bmatrix} = \\
= \sum_{k=0}^{\infty} \frac{(k+1)(z-1)^{k}}{2^{k+2}}
\end{gather}$$

$$\begin{gather}
D_{2}: \ f(z) = \left( -\frac{1}{(z-1)\left( 1- \frac{2}{z-1} \right)} \right)' = \left( -\frac{1}{z-1}\sum_{n=0}^{\infty} \frac{2^{n}}{(z-1)^{n}}  \right)' = \\
= -\sum_{n=0}^{\infty} \frac{2^{n}(-n-1)}{(z-1)^{n+2}} = \sum_{n=0}^{\infty} \frac{2^{n}(n+1)}{(z-1)^{n+2}}
\end{gather}$$

### 6

$$\begin{gather}
f(z) = ze^{1/(z-2)}, \ z_{0} = 2 \\
e^{u} = \sum_{n=0}^{\infty} \frac{u^{n}}{n!}, \ |u| < \infty  \\
f(z) = ((z-2)+2)e^{1/(z-2)} = (z-2)e^{1/(z-2)} + 2e^{1/(z-2)} = \\
\sum_{n=0}^{\infty} \frac{1}{(z-2)^{n-1}n!} + \sum_{n=0}^{\infty} \frac{2}{(z-2)^{n} n!} = \\
= (z-2) + \sum_{k=0}^{\infty} \frac{2k+3}{(z-2)^{k}(k+1)!}
\end{gather}$$

### 10

$$\begin{gather}
f(z) = e^{\frac{4z-2z^{2}}{(z-1)^{2}}}, \ z_{0} = 1
\end{gather}$$

$$\begin{gather}
f(z) = e^{-2}e^{\frac{2}{(z-1)^{2}}} = \\
= e^{-2}\sum_{n=0}^{\infty} \frac{2^{n}}{(z-1)^{2n}n!} = \sum_{n=0}^{\infty} \frac{2^{n}}{e^{2}n!(z-1)^{2n}}
\end{gather}$$