---
tags:
  - seminar
  - 2nd-semester
  - 2025-04-30
---

## Функции Бесселя

> [!definition] Д/у Бесселя
> $$y''(x) + \frac{1}{x}y'(x) + \left( 1-\frac{\nu^{2}}{x^{2}} \right)y(x) = 0, \ \nu > 0 \ (1)$$
> Любое решение уравнения Бесселя является функцией Бесселя.


$$\begin{gather}
J_{\nu}(x) = \sum_{m=0}^{\infty} \frac{(-1)^{m}\left( \frac{x}{2} \right)^{2m+\nu}}{\Gamma(m + \nu + 1)m!} \\
Y_{\nu}(x) = \frac{\cos \pi J_{\nu}(x) - J_{-\nu}(x)}{\sin \pi \nu}, \ \nu \not\in \mathbb{Z} - \text{ф-ция Бесселя второго рода}
\end{gather}$$

Если $\nu \not\in\mathbb{Z}$, то общее решние (1): $y(x)C_{1}J_{\nu}(x) + C_{2}J_{-\nu}(x)$
Если $\nu = n \in\mathbb{Z}$, то общее решние (1): $y(x)C_{1}J_{n}(x) + C_{2}Y_{n}(x)$

$$J_{-n}(x) = (-1)^{n}J_{n}(x), \ n = 1,2,\dots$$

$$\begin{gather}
x^{2}y''(x) + xy'(x) + (\lambda^{2}x^{2} - \nu^{2})y(x) = 0 \ (3)
\end{gather}$$

### 2. Найти общее решние

$$\begin{gather}
x^{2}y''(x) + xy'(x) + \left( 4x^{2} - \frac{9}{25} \right)y(x) = 0 \\
y(x) = C_{1}J_{\frac{3}{5}}(2x) + C_{2}J_{-\frac{3}{5}}(2x)
\end{gather}$$

### 3. Найти общее решние

$$\begin{gather}
x^{2}y''(x) + xy'(x) + (3x^{2} - 4)y(x) = 0 \\
\nu^{2} = 4, \ \lambda^{2} = 3 \\
y(x) = C_{1}J_{2}(\sqrt{ 3 }x) + C_{2}Y_{2}(\sqrt{ 3 }x)
\end{gather}$$

### 4

$$\begin{gather}
x^{2}y''(x) + 2xy'(x) + (x^{2} - 2)y(x) = 0 \\
y(0) = 0, \ y'(0) = \frac{1}{3} \\
y(x) = x^{\alpha}u(x) \\
x^{2}(\alpha x^{\alpha-1}u(x) + x^{\alpha}u'(x))' + 2x(\alpha x^{\alpha-1}u(x) + x^{\alpha}u'(x)) + (x^{2}-2)x^{\alpha}u(x) = 0 \\
x^{2}(\alpha(\alpha-1) x^{\alpha-2}u(x) + \alpha x^{\alpha-1}u'(x) + \alpha x^{\alpha-1}u'(x) + x^{\alpha}u''(x)) + \\
+ 2x(\alpha x^{\alpha-1}u(x) + x^{\alpha}u'(x)) + (x^{2}-2)x^{\alpha}u(x) = 0 \\
\end{gather}$$

$$\begin{gather}
x^{\alpha+2}u''(x) + (2\alpha x^{\alpha+1} + 2x^{\alpha+1})u'(x) + \\
+ (\alpha(\alpha-1) x^{\alpha} + 2\alpha x^{\alpha} + (x^{2}-2)x^{\alpha})u(x) = 0 \\
x^{\alpha+2} u''(x) + 2x^{\alpha+1}(\alpha + 1)u'(x) + x^{\alpha}(\alpha^{2} + \alpha + x^{2} - 2)u(x) = 0
\end{gather}$$

$$\begin{gather}
2(\alpha+1) = 1 \implies \alpha = -\frac{1}{2} \\
x^{3/2}y''
\end{gather}$$