---
tags:
  - seminar
  - 2nd-semester
  - 2025-05-06
---

### Применение вычетов к вычислению контурных интегралов

$$\begin{gather}
\oint_{\gamma} f(z) \, dz = 2\pi i\sum_{k=1}^{n} \mathrm{res}_{z=z_{k}} f(z)
\end{gather}$$
Если $f(z)$ - аналитична в $\mathbb{C}$ за истклюением $z_{1}, z_{2}, \dots, z_{n-1}$, то 



$$\begin{gather}
\sum_{k=1}^{n-1} \mathrm{res}_{z=z_{k}} f(z) + \mathrm{res}_{z=\infty} f(z) = 0
\end{gather}$$

### 1

$$\begin{gather}
\oint_{|z-1| = 1} \frac{dz}{z^{4}+1} = ? \\
z^{4} = -1 \\
z = \sqrt[4]{ -1 } = e^{i\frac{\pi+2\pi k}{4}} \\
\end{gather}$$

![[2025-05-06 Семинар - ТФКП 2025-05-06 14.29.24.excalidraw]]

$$\begin{gather}
z_{1} = e^{i\pi/4} \\
z_{2} = e^{-i\pi/4} \\
z_{1}, z_{2} - П1 \\
\end{gather}$$

$$\begin{gather}
I = 2\pi i[\underset{z=z_{1}}{\mathrm{res}} f(z) + \underset{z=z_{2}}{\mathrm{res}} f(z)] = 2\pi i \left[ \frac{1}{4e^{3i\pi/4}} + \frac{1}{4e^{-3i\pi/4}} \right] = \pi i\cos \frac{3\pi}{4} = -\frac{\pi i}{\sqrt{ 2 }}
\end{gather}$$

### 2

$$\begin{gather}
\oint_{|z| = 5} \frac{e^{1/z}}{z^{8} + 1} \\
z_{0} = 0 \\
z_{k} = \sqrt[8]{ -1 } = e^{i(\pi+2\pi k)/8} \\
\text{все z попали в} \ \gamma \\
f(z)\sim_{z\to \infty} \frac{a}{z^{k}}, \ z = 2,3,4,\dots \\
\underset{z=\infty}{\mathrm{res}} f(z) = 0 \\
\end{gather}$$

$$\begin{gather}
\text{тогда} \\
I = 2\pi i \left[ \sum_{n=1}^{8} \underset{z=z_{k}}{\mathrm{res}} f(z) + \underset{z=0}{\mathrm{res}} f(z)  \right] = 2\pi i \cdot 0 = 0
\end{gather}$$

![[2025-05-06 Семинар - ТФКП 2025-05-06 14.41.27.excalidraw]]

### 3

$$\begin{gather}
\oint_{|z|=1} \frac{e^{z}dz}{z^{2}(z^{2}+9)} \\
z_{0} = 0 - П2 \\
z_{1,2} = \pm 3i \\
\end{gather}$$

$$\begin{gather}
I = 2\pi i\cdot \underset{z=0}{\mathrm{res}} f(z) = 2\pi i\lim_{ z \to 0 } \left( \frac{e^{z}}{z^{2}+9} \right)' = 2\pi i\lim_{ z \to 0 } \left( \frac{e^{z}(z^{2}+9) - 2ze^{z}}{(z^{2}+9)^{2}} \right) = \\
= 2\pi i\cdot e^{0} \cdot \frac{9}{81} = \frac{2\pi i}{9} \\
\end{gather}$$

### 4

$$\begin{gather}
\oint_{|z| = 1} z^{n}e^{2/z} \, dz \\
z = 0 - \text{сущ. особая} \\
f(z) = z^{n}\sum_{k=0}^{\infty} \frac{\left( \frac{2}{z} \right)^{k}}{k!} = \\
= \sum_{k=0}^{\infty} \frac{2^{k}}{k!} \cdot z^{n-k} \\
z^{-1} \implies k = n+1 \implies c_{-1} = \frac{2^{n+1}}{(n+1)!} \\
\end{gather}$$

$$\begin{gather}
I = \frac{2^{n+2}\pi i}{(n+1)!}
\end{gather}$$

### 