---
tags:
  - seminar
  - 2nd-semester
  - 2025-02-21
---

### Нелинейные системы

### 1

$$\begin{gather}
\begin{cases}
\dot{x} = -y^{2} + \sin x \\
\dot{y} = -y\cos x
\end{cases}  - \text{система автономного вида} \\
\frac{\dot{y}}{\dot{x}} = \frac{dy}{dx} = \frac{y\cos x}{y^{2}-\sin x} \\
\end{gather}$$

$$\begin{gather}
y' = \frac{y\cos x}{y^{2}-\sin x} \\
\frac{y'}{y} = \frac{\cos x}{y^{2}-\sin x} \\
(y^{2}-\sin x)dy - (y\cos x)dx = 0 - \text{уравнение в полн. дифф} \\
F(x,y) = -\int y\cos x \, dx + \phi(y) = -y\sin x + \phi(y) \\
\phi'(y) -\sin x = y^{2}-\sin x \\
\phi(y) = \frac{y^{3}}{3} \\
F(x,y) = \frac{y^{3}}{3} - y\sin x = C \\
\end{gather}$$

### 2

$$\begin{gather}
\begin{cases}
\frac{dx}{dt} = \frac{1}{y^{2} - ax} \\
\frac{dy}{dt} = \frac{1}{2xy} \\
\end{cases} \\
y'_{x} = \frac{y^{2} - ax}{2xy} \\
(2xy)dy + (ax-y^{2})dx = 0 \\
x\,dy^{2} + (ax-y^{2})dx = 0 \\
\frac{dy^{2}}{dx} = \frac{y^{2}-ax}{x} \\
\begin{bmatrix}
y^{2} = z
\end{bmatrix} \\
\frac{dz}{dx} = \frac{z-ax}{x} \\
z'x = z-ax \\
z'x - z + ax = 0 \\
z' - \frac{z}{x} + a = 0 \\
\end{gather}$$

$$\begin{gather}
\begin{bmatrix}
z = uv \\
z' = u'v+uv'
\end{bmatrix} \\
uv' + u'v - uv\cdot\frac{1}{x} + a = 0 \\
uv' + v\left( u' - u\cdot\frac{1}{x} \right) + a = 0 \\
u' = \frac{u}{x} \\
\frac{u'}{u} = \frac{1}{x} \\
\ln u = \ln x \\
u = x
\end{gather}$$

$$\begin{gather}
xv' + a = 0 \\
v' = -\frac{a}{x} \\
v = -a\ln x \\
z = uv = -ax(\ln x + C) \\
\end{gather}$$

$$\begin{gather}
y^{2} = -ax(\ln x + C) \\
y^{2} = x(-a\ln x + C) \\
\end{gather}$$

$$\begin{gather}
dt = ((C-a)x - ax\ln x)dx \\
t+C_{1} = \frac{c-a}{2}x^{2} - a\left( \frac{x^{2}}{2}\ln x - \frac{x^{2}}{4} \right) + C \\
\end{gather}$$

### 3

$$\begin{gather}
\begin{cases}
y' = \frac{z}{x} \\
z' = \frac{z(y+2z-1)}{x(y-1)} \\
\end{cases} \\
\frac{z'}{y'} = \frac{xz(y+2z-1)}{xz(y-1)} = \frac{y+2z-1}{y-1} \\
\end{gather}$$

$$\begin{gather}
\frac{z'}{y'} = 1+\frac{2z}{y-1} \\
\frac{dz}{d(y-1)} = 1 + \frac{2z}{u-1} \\
\begin{bmatrix}
y-1 = u
\end{bmatrix} \\
\frac{dz}{du} = 1+ \frac{2z}{u} \\
\end{gather}$$

$$\begin{gather}
\text{Угадали:} \ z = -u \\
z_{оо} = Cu^{2} \\
z = C(y-1)^{2} - y + 1 \\
y' = \frac{C(y-1)-y+1}{x} \\
\int \frac{d(y-1)}{C(y-1)^{2}-(y-1)} = \ln |x| + \ln \tilde{C} \\
\end{gather}$$

$$\begin{gather}
\begin{bmatrix}
y-1 = t
\end{bmatrix} \\
-\int \frac{dt}{t}  + \int \frac{d(Ct-1)}{Ct-1} = \ln(y-1) + \ln(C(y-1)-1)
\end{gather}$$

$$\begin{gather}
\ln(y-1) + \ln(C(y-1)-1) = \ln x + \ln \tilde{C} \\
\frac{C(y-1)-1}{y-1} = \tilde{C} x
\end{gather}$$

### 4

$$\begin{gather}
\begin{cases}
\dot{x} = x - 5y + 2z \\
\dot{y} = -x-3y+2z \\
\dot{z} = x-3y \\
\end{cases} \\
\end{gather}$$

$$\begin{gather}
\begin{cases}
\dot{x} = x - 5y + 2z \\
\dot{y} = -x-3y+2z \\
\dot{z} = x-3y \\
\ddot{z} = \dot{x}-3\dot{y} \\
\dddot{z} = \ddot{x}-3\ddot{y} \\
\ddot{x} = \dot{x} - 5\dot{y} + 2\dot{z} \\
\ddot{y} = -\dot{x} - 3\dot{y} + 2\dot{z}
\end{cases}
\end{gather}$$

$$\begin{gather}
\begin{cases}
\dot{z} = x - 3y \\
\ddot{z} = x-5y+2z - 3(-x+3y+2z) \\
\dddot{z} = (\dot{x}-5\dot{y} + 2\dot{z}) - 3(-\dot{x} -3\dot{y} + 2\dot{z}) \\
\end{cases} \\
\begin{cases}
\dot{z} = x - 3y \\
\ddot{z} = 4x-14y-4z \\
\dddot{z} = (x-5y+2z-5(-x-3y+2z) + 2(x-3y)) - \\ - 3(-(x-5y+2z) -3(-x-3y+2z) + 2(x-3y)) \\
\end{cases}
\end{gather}$$

$$\begin{gather}
\begin{cases}
\dot{z} = x - 3y \\
\ddot{z} = 4(x+y-z) \\
\dddot{z} = -32y+12z \\
\end{cases} \\
\end{gather}$$

$$\begin{gather}
\dddot{z} = 4\dot{z} - 2\ddot{z} + 8z \\
\dddot{z} +2\ddot{z}
\end{gather}$$