---
tags:
  - seminar
  - 2nd-semester
  - 2025-04-09
---

### 9 (Дз)

$$\begin{gather}
f(x) = xe^{-x^{2}} - \text{нечетная} \\
f(x) = \frac{2}{\pi} \int_{0}^{+\infty} \, dz \int_{0}^{+\infty} ue^{-u^{2}}\sin zu\sin zx \, dx  \\
I(z) = \int_{0}^{+\infty} ue^{-u^{2}}\sin zu \, du = -\frac{1}{2}\int_{0}^{+\infty} \sin zu \, d(e^{-u^{2}}) = \\
= -\frac{1}{2} \left.\left[ \sin zu e^{-u^{2}}  \right|_{0}^{+\infty} - \int_{0}^{+\infty} e^{-u^{2}} \cos zu \cdot z \, du\right] = \\
\end{gather}$$

$$\begin{gather}
= \frac{z}{2}\underbrace{\int_{0}^{+\infty} e^{-u^{2}} \cos zu \, du}_{J(z)} = \dots
\end{gather}$$

$$\begin{gather}
J(z) = \int_{0}^{+\infty} e^{-u^{2}}\cos zu \, du \\
J'(z) = -\int_{0}^{+\infty} e^{-u^{2}}\sin zu \, du = \\
= -\frac{z}{2} \int_{0}^{+\infty} e^{-u^{2}} \cos zu \, du  \\
J'(z) = -\frac{z}{2}J(z)
\end{gather}$$

$$\begin{gather}
\frac{dJ}{dz} = -\frac{z}{2} \cdot J(z) \\
\ln |J| = -\frac{z^{2}}{4} + C_{1} \\
J = \pm e^{C_{1}}e^{-z^{2}/4} \\
J = Ce^{-z^{2}/4} \\
J(0) = \frac{\sqrt{ \pi }}{2} \implies C = \frac{\sqrt{ \pi }}{2} \\
J(z) = \frac{\sqrt{ \pi }}{2} e^{-z^{2}/4}
\end{gather}$$

$$\begin{gather}
I(z) = \frac{\frac{z}{2}\sqrt{ \pi }}{2} e^{-z^{2}/4} = \frac{\sqrt{ \pi }}{4}ze^{-z^{2}/4} \\
f(x) = \frac{2}{\pi}\int_{0}^{+\infty} \sin zx \cdot I(z) \, dz \\ 
f(x) = \frac{1}{2\sqrt{ \pi }} \int_{0}^{+\infty} ze^{-z^{2}/4} \sin zx \, dz
\end{gather}$$

## Преобразование Фурье

$$f(x) = \frac{1}{\pi}\int_{0}^{+\infty} dz \int_{-\infty}^{+\infty} f(u) \cos[z(x-u)] \, du$$

$$\begin{gather}
f(x) = \frac{1}{2\pi} \int_{-\infty}^{+\infty} \, dz \int_{-\infty}^{+\infty} f(u) e^{iz(x-u)} \, du \\
\end{gather}$$

$$\begin{cases}
F(z) = \frac{1}{\sqrt{ 2\pi }} \int_{-\infty}^{+\infty} f(u) e^{-izu} \, du - \text{преобразование Фурье ф-ции} \ f(x) \\
f(x) = \frac{1}{\sqrt{ 2\pi }}\int_{-\infty}^{+\infty} F(z)e^{izx} \, dz - \text{формула обращения} \\
\mathcal{F}[f]
\end{cases}$$

Если $f(x)$ - четная, то 

$$\begin{gather}
\begin{cases}
F_{c}(z) = \sqrt{ \frac{2}{\pi} } \int_{0}^{+\infty} f(u)\cos zu \, du \\
f(x) = \sqrt{ \frac{2}{\pi} } \int_{0}^{+\infty} F_{c}\cos zx \, dz \\
\mathcal{F}[f] = \mathcal{F}_{c}[f]
\end{cases}
\end{gather}$$

Если $f(x)$ - нечетная, то 

$$\begin{cases}
F_{s}(z) = \sqrt{ \frac{2}{\pi} } \int_{0}^{+\infty} f(u)\sin zu \, du \\
f(x) = \sqrt{ \frac{2}{\pi} } \int_{0}^{+\infty} F_{s}\sin zx \, dz \\
\mathcal{F}[f] = -i\mathcal{F}_{s}[f]
\end{cases}$$

### Свойства преобразования Фурье

1. $\mathcal{F}[f^{(k)}] = (iz)^{k}\mathcal{F}[f]$
2. $i^{k}\mathcal{F}^{(k)}[f] = \mathcal{F}[x^{k} f]$

### 11. Найти преобразование Фурье функции $f(x)$

$$\begin{gather}
f(x) = \begin{cases}
e^{ix}, |x| \leq \pi \\
0, |x| > \pi
\end{cases}
\end{gather}$$

$$\begin{gather}
\mathcal{F}(z) = \frac{1}{\sqrt{ 2\pi }} \int_{-\infty}^{+\infty} e^{iu}e^{-izu} \, du = \\
= \frac{1}{\sqrt{ 2\pi }}\int_{-\pi }^{\pi} e^{iu(1-z)} \, du = \\
= \frac{1}{\sqrt{ 2\pi }} \left.\frac{e^{iu(1-z)}}{i(1-z)}\right|_{-\pi}^{\pi} = \\
\end{gather}$$

$$\begin{gather}
= \frac{2i\sin \pi(1-z)}{\sqrt{ 2\pi }\cdot i \cdot (1-z)} = \\
= \frac{\sqrt{ 2 } \sin (\pi - \pi z)}{\sqrt{ \pi }(1-z)} = \\
= \frac{\sqrt{ 2 }\sin \pi z}{\sqrt{ \pi }(1-z)}
\end{gather}$$

### 14

$$\begin{gather}
f(x) = \frac{d}{dx} (xe^{-|x|}) \\
\text{Найти} \ \mathcal{F}[f] \\
\end{gather}$$

$$\begin{gather}
f_{0}(x) = e^{-|x|} - \text{четная} \\
\mathcal{F}[f_{0}] = \mathcal{F}_{c}[f_{0}] = \sqrt{ \frac{2}{\pi} } \int_{0}^{+\infty} e^{-|u|}\cos zu \, du = \\
= \sqrt{ \frac{2}{\pi} } \int_{0}^{+\infty} e^{-u}\cos zu \, du = \sqrt{ \frac{2}{\pi} } \cdot \frac{1}{1+z^{2}} \\
\end{gather}$$

$$\begin{gather}
\mathcal{F}[xf_{0}] = i\mathcal{F}'[f_{0}] = i\sqrt{ \frac{2}{\pi} }\left( \frac{1}{1+z^{2}} \right)' = \dots = \frac{2\sqrt{ 2 }iz}{\sqrt{ \pi }(1+z^{2})^{2}}
\end{gather}$$

$$\begin{gather}
\mathcal{F}[f] = \frac{2\sqrt{ 2 }iz}{\sqrt{ \pi }(1+z^{2})^{2}}
\end{gather}$$

### Эйлеров интеграл

$$\begin{gather}
\Gamma(p) = \int_{0}^{+\infty} x^{p-1}e^{-x} \, dx \ (p>0) \\
\mathrm{B}(p,q) = \int_{0}^{1} x^{p-1}(1-x)^{q-1} \, dx, \ (p,q > 0) \\
\end{gather}$$

1. $\Gamma(1) = 1, \ \Gamma\left( \frac{1}{2} \right) = \sqrt{ \pi }$
2. $\Gamma(p+1) = p\Gamma(p), p > 0$ (формула понижения)
3. $\Gamma(n+1)= n!, \ \Gamma\left( n + \frac{1}{2} \right) = \frac{(2n-1)!!}{2^{n}}\sqrt{ \pi }, \ n \in \mathbb{N}$
4. $\Gamma(p)\Gamma(1-p) = \frac{\pi}{\sin \pi p}, \ 0 < \pi < 1$ (формула дополнения)
5. $\mathrm{B}(p,q) = \mathrm{B}(q,p)$ (свойство симметрии)
6. $\mathrm{B}(p,q) = \frac{\Gamma(p)\Gamma(q)}{\Gamma(p+q)}$
7. $\mathrm{B}(p,1-p) = \frac{\pi}{\sin \pi p}, \ 0 < p < 1$

### 1a

$$\begin{gather}
\Gamma\left( \frac{1}{6} \right)\Gamma\left( \frac{23}{6} \right) = ? \\
\Gamma\left( \frac{23}{6} \right) = \Gamma\left( 1 + \frac{17}{6} \right) = \frac{17}{6}\Gamma\left( 1 + \frac{11}{6} \right) = \frac{17\cdot 11}{36}\Gamma\left( 1 + \frac{5}{6} \right) = \\
= \frac{17\cdot 11\cdot 5}{216}\Gamma\left( \frac{5}{6} \right) \\
\frac{17\cdot 11\cdot 5}{216}\Gamma\left( \frac{1}{6} \right)\Gamma\left( \frac{5}{6} \right) = \frac{935\pi}{108}
\end{gather}$$

### 2a

$$\begin{gather}
\mathrm{B}\left( \frac{1}{4}, \frac{11}{4} \right) = \frac{\Gamma\left( \frac{1}{4} \right)\Gamma\left( \frac{11}{4} \right)}{\Gamma(3)} = \frac{\frac{7\cdot 3}{16}\Gamma\left( \frac{1}{4} \right)\Gamma\left( \frac{3}{4} \right)}{2} = \\
= \frac{21}{16\cdot 2}\cdot 4\pi \sqrt{ 2 } = \frac{21\pi}{16\sqrt{ 2 }}
\end{gather}$$

### 3

$$\begin{gather}
\int_{0}^{1}\sqrt{ x-x^{2} } \, dx  = \int_{0}^{1} \sqrt{ x }\sqrt{ 1-x } \, dx = \int_{0}^{1} x^{1/2}(1-x)^{1/2} \, dx = \\
= B\left( \frac{3}{2}, \frac{3}{2} \right) = \frac{\Gamma\left( \frac{3}{2} \right) \Gamma\left( \frac{3}{2} \right)}{\Gamma(3)} = \frac{\left( \frac{(2-1)!!}{2}\sqrt{ \pi } \right)^{2}}{2} = \frac{\pi}{8} \\
\end{gather}$$

### 4

$$\begin{gather}
\int_{0}^{a} x^{2} \sqrt{ a^{2}-x^{2} } \, dx = \begin{bmatrix}
t = \frac{x^{2}}{a^{2}} \\
dt = \frac{2x}{a^{2}}dx \\
dx = \frac{a^{2}dt}{2x} = \frac{a\,dt}{2\sqrt{ t }}
\end{bmatrix} = \\
= \frac{a^{4}}{2}\int_{0}^{1} t^{3/2-1}(1-t)^{3/2-1} \, dx =  \\
= \frac{a^{4}}{2}\mathrm{B}\left( \frac{3}{2}, \frac{3}{2} \right) = \frac{a^{3}\pi}{16} \\
\end{gather}$$

### 5

$$\begin{gather}
\int_{0}^{+\infty} \frac{\sqrt[4]{ x }}{(1+x)^{2}} \, dx = \begin{bmatrix}
t = \frac{x}{1+x} \\
x = \frac{t}{1-t} \\
dx = \frac{1}{(1-t)^{2}}dt
\end{bmatrix} = \int_{0}^{1} \frac{\sqrt[4]{ \frac{t}{1-t} }}{\left( 1+\frac{1}{1-t} \right)^{2}}\frac{1}{(1-t)^{2}} \, dt = \\
\end{gather}$$