---
tags:
  - seminar
  - 2nd-semester
  - 2025-02-28
---

### Продолжение 

$$\begin{gather}
\begin{cases}
x = 2C_{1}e^{2t} + e^{-2t}\left( C_{2}-\frac{C_{3}}{2} \right) + C_{3}te^{-2t} \\
y = e^{-2t}\left( C_{2}-\frac{C_{3}}{2} \right) + C_{3}te^{-2t} \\
z = C_{1}e^{2t} + C_{2}e^{-2t} + C_{3}te^{-2t}
\end{cases}
\end{gather}$$

$$\begin{gather}
A = \begin{pmatrix}
1 & -5 & 2 \\
-1 & -3 & 2 \\
1 & -3 & 0
\end{pmatrix} \\
\det \left( A-\lambda E \right)  = -\lambda^{3} + \lambda^{2}\mathrm{Tr} \ A  -\lambda\sum_{i}^{n} M_{ii} + \det A \\
-\lambda^{3} +2\lambda^{2} - \lambda(6 - 3 + 2) + 8 = \\
= -\lambda^{3} - 2\lambda^{2} + 4\lambda + 8
\end{gather}$$

$$\begin{gather}
\dot{y} = -x-3y+2z \\
\ddot{y} = -\dot{x}-3\dot{y}+2\dot{z} \\
\ddot{y} = -(x-5y+2z) - 3\dot{y} + 2x - 6y = x-2z -y-3\dot{y}
\end{gather}$$

$$\begin{gather}
\dot{y} + \ddot{y} = -y-3\dot{y} \\
y = C_{1}e^{-2t}+C_{2}te^{-2t} \\
\dot{x} - \dot{y} = 2x-2y \\
\dot{x} -2x = \dot{y}-2y
\end{gather}$$

$$\begin{gather}
\dot{x} -2x = -2C_{1}e^{-2t} \\
\dot{x} - 2x = 0 \\
x_{оо} = C_{3}e^{2t} \\
x_{он} = C_{1}e^{-2t} + C_{2}te^{-2t} + C_{3}e^{2t}
\end{gather}$$

### 796

$$\begin{gather}
\begin{cases}
\dot{x} = x-y+z \\
\dot{y} = x+y-z \\
\dot{z} = 2x-y
\end{cases} \\
A = \begin{pmatrix}
1 & -1 & 1 \\
1 & 1 & -1 \\
2 & -1 & 0
\end{pmatrix} \\
\det \left( A - \lambda E \right)  = -\lambda^{3} + \lambda^{2}\mathrm{Tr} \ A + \lambda \sum_{i}^{n} M_{ii} + \det A = \\
= -\lambda^{3} +2\lambda^{2} + \left( 1-2+2 \right) \lambda + 2 = \\
= -\lambda^{3} + 2\lambda^{2}+\lambda-2 = 0 \\
\lambda^{3}-2\lambda^{2}-\lambda+2 = 0 \\
(\lambda-1)(\lambda^{2}-\lambda-2) = 0 \\
(\lambda-1)(\lambda-2)(\lambda+1)=0
\end{gather}$$

$$\begin{gather}
\lambda_{1} = 1: \ \begin{pmatrix}
0 & -1 & 1 \\
1 & 0 & -1 \\
2 & -1 & -1
\end{pmatrix} \begin{pmatrix}

\end{pmatrix}
\end{gather}$$