---
tags:
  - seminar
  - 2nd-semester
  - 2025-04-04
---

$$\begin{gather}
\begin{cases}
\dot{x} = 5x - 3y + 2e^{3t} \\
\dot{y} = x + y + 5e^{-t}
\end{cases} \\
\end{gather}$$

### 1. Метод вариации постоянного

$$\begin{gather}
\begin{cases}
\dot{x} = 5x - 3y \\
\dot{y} = x+y
\end{cases} \\
\lambda_{1} = 2, \ \lambda_{2} = 4 \\
\vec{x}_{1} = \begin{pmatrix}
1 \\
1
\end{pmatrix}, \ \vec{x}_{2} = \begin{pmatrix}
3 \\
1
\end{pmatrix} \\
\begin{pmatrix}
x \\
y
\end{pmatrix} = C_{1}e^{2t}\begin{pmatrix}
1 \\
1
\end{pmatrix} + C_{2}e^{4t}\begin{pmatrix}
3 \\
1
\end{pmatrix} \\
\end{gather}$$

$$\begin{gather}
\begin{pmatrix}
e^{2t} & 3e^{4t} \\
e^{2t} & e^{4t}
\end{pmatrix}\begin{pmatrix}
C_{1} \\
C_{2}
\end{pmatrix} = \mathbf{X}(t)\mathbf{C}
\end{gather}$$

$$\begin{gather}
\dot{\mathbf{X}} = A\mathbf{X} + \mathbf{f}(t), \ \text{где} \ \mathbf{f}(t) = \begin{pmatrix}
2e^{3t} \\
5e^{-t}
\end{pmatrix}
\end{gather}$$

$$\begin{gather}
\mathbf{X}_{он} = \mathbf{X}(t)\mathbf{C}(t) \\
\dot{\mathbf{X}} = \dot{\mathbf{X}}\mathbf{C} + \mathbf{X}\dot{\mathbf{C}} \\
A\mathbf{X} + \mathbf{f} = A\mathbf{X}\mathbf{C} + \mathbf{f}
\end{gather}$$

$$\begin{gather}
\dot{\mathbf{X}} = A\mathbf{X} \\
\mathbf{X}\dot{\mathbf{C}} = \mathbf{f} \\
\dot{\mathbf{C}} = \mathbf{X}^{-1}\mathbf{f} \\
\end{gather}$$

$$\begin{gather}
\mathbf{X}^{-1} = -\frac{1}{2e^{6t}}\begin{pmatrix}
e^{4t} & -3e^{4t} \\
-e^{2t} & e^{2t}
\end{pmatrix} = -\frac{1}{2}\begin{pmatrix}
e^{-2t} & -3e^{-2t} \\
-e^{-4t} & e^{-4t}
\end{pmatrix} \\
\dot{\mathbf{C}} = -\frac{1}{2}\begin{pmatrix}
e^{-2t} & -3e^{-2t} \\
-e^{-4t} & e^{-4t}
\end{pmatrix}\begin{pmatrix}
2e^{3t} \\
5e^{-t}
\end{pmatrix} = -\frac{1}{2}\begin{pmatrix}
2e^{t}-15e^{-3t} \\
-2e^{-t}+5e^{-5t}
\end{pmatrix}
\end{gather}$$

$$\begin{gather}
\mathbf{C} = -\frac{1}{2}\begin{pmatrix}
2e^{t}+5e^{-3t} + \tilde{C}_{1} \\
2e^{-t} -e^{-5t} + \tilde{C}_{2}
\end{pmatrix}
\end{gather}$$

$$\begin{gather}
\mathbf{X}_{он} = \begin{pmatrix}
e^{2t} & 3e^{4t} \\
e^{2t} & e^{4t}
\end{pmatrix}\left( -\frac{1}{2} \right)\begin{pmatrix}
2e^{t}+5e^{-3t} + \tilde{C}_{1} \\
2e^{-t} -e^{-5t} + \tilde{C}_{2}
\end{pmatrix} = -\frac{1}{2}\begin{pmatrix}
\dots
\end{pmatrix}
\end{gather}$$

$$\begin{gather}
\mathbf{X} = \begin{pmatrix}
\tilde{C}_{1}e^{2t} +3\tilde{C}_{2}e^{4t}-4e^{3t} - e^{-t} \\
\tilde{C}_{1}e^{} + 
\end{pmatrix}
\end{gather}$$