---
tags:
  - seminar
  - 2nd-semester
  - 2025-09-03
---

### 1.

$$\begin{gather}
u_{x} = 8xy - 4y^{3}, \ u = (x,y) \\
u = 4x^{2}y - 4xy^{3} + C(y)
\end{gather}$$

### 2.

$$\begin{gather}
u_{y} = 8xy - 4y^{3} \\
u = 4xy^{2} - y^{4} + C(x)
\end{gather}$$

### 3. 

$$\begin{gather}
u_{xx} = 80y\sin(4x) \\
u_{x} = -20y\cos(4x) + C_{1}(y) \\
u = -5y\sin(4x) + C_{1}(y)x + C_{2}(y)
\end{gather}$$

### 4.

$$\begin{gather}
u_{xy} = x-y \\
u_{y} = \frac{x^{2}}{2} - xy + C_{1}(y) \\
u = \frac{x^{2}y}{2} -\frac{xy^{2}}{2} + \tilde{C}_{1}(y) + C_{2}(x)
\end{gather}$$

### 5.

$$\begin{gather}
u_{x} = x + yz^{2}, \ u = u(x,y,z) \\
u = \frac{x^{2}}{2} + xyz^{2} + C(y,z)
\end{gather}$$

### 6.

$$\begin{gather}
u_{yy} + u_{y} - 2u = 0, \ u = u(x,y) \\
\lambda^{2} + \lambda - 2 = 0 \\
\begin{cases}
\lambda_{1} = 1 \\
\lambda_{2} = -2
\end{cases} \\
u = C_{1}(x)e^{y} + C_{2}(x)e^{-2y}
\end{gather}$$

### 7.

$$\begin{gather}
u_{xx} -2u_{x} = 0 \\
\lambda^{2} - 2\lambda = 0 \\
\lambda(\lambda-2) = 0 \\
\lambda_{1} = 0, \ \lambda_{2} = 2 \\
u = C_{1}(y)e^{x} + C_{2}(y)e^{2x} \\
\end{gather}$$

### 8.

$$\begin{gather}
x^{2}u_{yy} + 2xu_{y} + u = 0 \\
x^{2}\lambda^{2} + 2x\lambda + 1 = 0 \\
(x\lambda + 1)^{2} = 0 \\
u = C_{1}(x)e^{-y/x} + C_{2}(x)ye^{-y/x}
\end{gather}$$

### 9.

$$\begin{gather}
u_{xx} + u = yxe^{x} \\
\lambda^{2} + 1 = 0 \\
\lambda_{1,2} = \pm i \\
u^{оо} = C_{1}(y)\sin x + C_{2}(y)\cos x \\
\end{gather}$$

$$\begin{gather}
u_{x} = Ae^{x} + (Ax + B)e^{x} \\
u_{xx} = 2Ae^{x} + (Ax + B)e^{x} \\
2Ae^{x} + (Ax+B)e^{x} + (Ax + B)e^{x} = xye^{x} \\
\end{gather}$$

$$\begin{gather}
\begin{cases}
2A + 2B = 0 \\
2A = y
\end{cases} \implies \begin{cases}
A = \frac{y}{2} \\
B = -\frac{y}{2}
\end{cases} \\
u^{чн} = \frac{y}{2}(x-1)e^{x}
\end{gather}$$

$$\begin{gather}
y^{он} = C_{1}(y)\sin x + C_{2}(y)\cos x + \frac{y}{2}(x-1)e^{x}
\end{gather}$$

### 10.

$$\begin{gather}
\begin{cases}
u_{x} = y \\
u_{y} = x
\end{cases} \\
\begin{cases}
u = xy + C_{1}(y) \\
u = xy + C_{2}(x)
\end{cases} \\
u = xy + C
\end{gather}$$

$$\begin{gather}
\begin{cases}
u_{x} = y \\
u_{y} = x
\end{cases} \\
u_{x} = y, \ u = \int y \, dx  = xy + C_{1}(y) \\
u_{y} = x + C_{1}'(y) = x \\
C_{1}'(y) = 0 \implies C_{1}(y) = C = \mathrm{const} \\
y = xy + C
\end{gather}$$

$$\begin{gather}
u(x,y) = C \\
u_{x}dx + u_{y}dy = 0 \\
ydx + xdy = 0 \\
\frac{y}{x} + \frac{dy}{dx} = 0 \\
\dots
\end{gather}$$

### 11.

$$\begin{gather}
\begin{cases}
u_{x} = z \\
u_{y} = 2y \\
u_{z} = x
\end{cases} \\
u = xz + C_{1}(y,z) \\
u_{y} = \frac{\partial C_{1}(y,z)}{\partial  y} = 2y \\
C_{1}(y,z) = y^{2} + C_{2}(x,z) \\
u = xz + y^{2} + C_{2}(z) \\
u_{z} = x + \frac{\partial C_{2}(z)}{\partial z} = x \\
C_{2}(z) = C \\
u = xz + y^{2} + C
\end{gather}$$

### 12.

$$\begin{gather}
\begin{cases}
u_{x} = 0 \\
u_{y} = ze^{yz} \\
u_{z} = ye^{yz}
\end{cases} \\
u = e^{yz} + C_{1}(z) \\
u_{z} = ye^{yz} + \frac{\partial C_{1}(z)}{\partial z} = ye^{yz} \implies C_{1}(z) = C \\
u = e^{yz} + C
\end{gather}$$

### 13.

$$\begin{gather}
\begin{cases}
u_{x} = 2xy \\
u_{y}= x-y
\end{cases}
\end{gather}$$