---
tags:
  - seminar
  - 2nd-semester
  - 2025-05-13
---

## Приложения теории вычетов

$$\begin{gather}
1. \ \int_{0}^{2\pi} R(\cos \phi, \sin \phi) \, d\phi = \oint_{|z| = 1} R_{1}(z) dz = \\
= 2\pi i \sum_{|z_{k}| < 1} \underset{z=z_{k}}{\mathrm{res}} R_{1}(z) \\
z = e^{i\phi} \\
\cos\phi = \frac{1}{2}\left( z + \frac{1}{z} \right) \\
\sin\phi = \frac{1}{2i}\left( z-\frac{1}{z} \right) \\
dz = e^{i\phi}id\phi \implies d\phi = \frac{dz}{iz}
\end{gather}$$

$$\begin{gather}
2. \ \int_{-\infty}^{+\infty} F(x) \, dx = 2\pi i \sum_{\mathrm{Im} z_{k} > 0} \underset{z=z_{k}}{\mathrm{res}} F(z) = -2\pi i \sum_{\mathrm{Im} z_{k} < 0} \underset{z=z_{k}}{\mathrm{res}} F(z) \\
F(x) = \frac{P_{m}(x)}{Q_{n}(x)}, \ n - m \geq 2 \\
F(x) - \text{непр. на} \ \mathbb{R}
\end{gather}$$

$$\begin{gather}
3. \ \int _{-\infty}^{+\infty} F(x)e^{i\alpha x} \, dx  = \begin{cases}
2\pi i \sum_{\mathrm{Im} \ z_{k}>0} \underset{z=z_{k}}{\mathrm{res}} [F(z) e^{i\alpha z}] \ (\alpha>0) \\
-2\pi i \sum_{\mathrm{Im} \ z_{k}<0} \underset{z=z_{k}}{\mathrm{res}} [F(z) e^{i\alpha z}] \ (\alpha < 0) \\
\end{cases} \\
F(x) - \text{правильная рац. дробь}; \ F(x) - \text{непрерывна на} \ \mathbb{R}
\end{gather}$$

### 1

$$\begin{gather}
\int_{0}^{2\pi} \frac{dx}{a+\cos x} = \\
\begin{bmatrix}
z = e^{i\phi} \\
\cos x = \frac{1}{2}\left( z + \frac{1}{z} \right) \\
dx = \frac{dz}{iz}
\end{bmatrix} = \\
= \frac{2}{i}\oint_{|z| = 1} \frac{dz}{2az + z^{2} + 1}
\end{gather}$$

$$\begin{gather}
z = -a \pm \sqrt{ a^{2}-1 } \\
\underset{z=-a+\sqrt{ a^{2}-1 }}{\mathrm{res}} R_{1}(z) = \frac{1}{2\sqrt{ a^{2}-1 }} \\
I = \frac{2\pi}{\sqrt{ a^{2} - 1 }}
\end{gather}$$

### 4

$$\begin{gather}
\int_{-\infty}^{+\infty} \frac{x^{2} + 1}{x^{4} + 1} \, dx \\
z = \sqrt[4]{ -1 } = e^{(\pi/4 + 2\pi k/4)i} \\
I = 2\pi i \left( \underset{z=e^{i\pi/4}}{\mathrm{res}} \frac{z^{2}+1}{z^{4}+1} + \underset{z=e^{3\pi i/4}}{\mathrm{res}}\frac{z^{2}+1}{z^{4}+1}  \right) = \\
= 2\pi i\left( \frac{1}{4}[e^{-i\pi/4} + e^{-3i\pi/4}] + \frac{1}{4}\left[ -\frac{3\pi i}{4} + e^{-9\pi i/4} \right] \right) = \\
= \pi i(e^{i\pi})

\end{gather}$$
