---
tags:
  - seminar
  - 2nd-semester
  - 2025-03-28
---

$$\begin{gather}
A = \begin{pmatrix}
1 & -2 \\
1 & 3
\end{pmatrix} \\ 
e^{At} \risingdotseq (pE - A)^{-1} \\
\end{gather}$$

$$\begin{gather}
\left( \begin{pmatrix}
p & 0 \\
0 & p
\end{pmatrix} - \begin{pmatrix}
1 & -2 \\
1 & 3
\end{pmatrix} \right)^{-1} = \begin{pmatrix}
p-1 & 2 \\
-1 & p-3
\end{pmatrix}^{-1} \\
(p-1)(p-3) +2 \neq 0 \\
p^{2} -4p + 5 \neq 0 \\
(p-2)^{2} \neq -1 \\
p \neq 2\pm i \\
\end{gather}$$

$$\begin{gather}
\begin{pmatrix}
p-1 & 2 \\
-1 & p-3
\end{pmatrix}^{-1} = \frac{1}{p^{2}-4p+5} \begin{pmatrix}
p-3 & -2 \\
1 & p-1
\end{pmatrix} \\
\frac{p-3}{p^{2}-4p+5} \risingdotseq  \\
e^{\alpha t}\cos\beta t \risingdotseq \frac{p-\alpha}{(p-\alpha)^{2} + \beta^{2}} \\
e^{\alpha t}\sin\beta t \risingdotseq \frac{\beta}{(p-\alpha)^{2} + \beta^{2}} \\ 
\end{gather}$$

$$\begin{gather}
\frac{p-3}{(p-2)^{2} + 1} = \frac{p-2}{(p-2)^{2} + 1} - \frac{1}{(p-2)^{2} + 1} \\
\frac{p-3}{(p-2)^{2} + 1} \fallingdotseq e^{2t}\cos t - 2e^{2t}\sin t \\
\text{Остальное - аналогично}
\end{gather}$$

$$\begin{gather}
e^{At} = e^{2t}\begin{pmatrix}
\cos t - 2 \sin t & -2\sin t \\
\sin t & \cos t + \sin t
\end{pmatrix} \\
\end{gather}$$

$$\begin{gather}
X(t) - \text{фундаментальная матрица системы} \\
e^{At} = X(t)(X(0))^{-1} \\
\begin{cases}
\dot{x} = x-2y \\
\dot{y} = x+3y
\end{cases} \\
\lambda_{1,2} = 2\pm i 
\end{gather}$$

$$\begin{gather}
A_{\lambda,\lambda=2+i}: \ \begin{pmatrix}
-1-i & -2 \\
1 & 1-i
\end{pmatrix} \sim \begin{pmatrix}
1 & 1-i
\end{pmatrix}\begin{pmatrix}
-1+i \\
1
\end{pmatrix} = \vec{0} \\
v_{1} = \begin{pmatrix}
-1+i \\
1
\end{pmatrix} \\
e^{(2+i) t}\begin{pmatrix}
-1+i \\
1
\end{pmatrix} = e^{2t}e^{it}\begin{pmatrix}
-1+i \\
1
\end{pmatrix} = e^{2t}e^{it}\begin{pmatrix}
-1+i \\
1
\end{pmatrix} = 
\end{gather}$$