---
tags:
  - типовой-расчет
  - 2nd-semester
  - 2024-11-03
---
## ТР 1 СГВМ

### Ершов Алексей Геннадьевич КМБО-03-23

### Вариант 5

### 1.1

$$\begin{gather}
y' + 3y = x^{2} - 2x, \ y(0) = -2 \\
\begin{bmatrix}
y = uv \\
y' = uv' + u'v
\end{bmatrix} \\
uv' + u'v + 3uv = x^{2} - 2x \\
uv' + v(u' + 3u) = x^{2} - 2x \\
\end{gather}$$

$$\begin{gather}
u' + 3u = 0 \\
\frac{u'}{u} = -3 \\
\ln |u| = -3x \\
u = e^{-3x} \\
\end{gather}$$

$$\begin{gather}
v'e^{-3x} = x^{2} - 2x \\
v' = e^{3x}(x^{2} - 2x) \\
v = \int e^{3x}(x^{2}-2x) \, dx \\
v = \frac{1}{3}e^{3x}(x^{2}-2x) - \frac{1}{3}\int e^{3x}(2x-2) \, dx \\
v = \frac{1}{3}e^{3x}(x^{2}-2x) - \frac{1}{3}\left( \frac{1}{3}e^{3x}(2x-2) - \frac{2}{3}\int e^{3x} \, dx \right) \\
\end{gather}$$

$$\begin{gather}
v = \frac{1}{3}e^{3x}(x^{2}-2x) - \frac{1}{3}\left( \frac{1}{3}e^{3x}(2x-2) - \frac{2}{9} e^{3x} \right) + C \\
v = \frac{1}{3}e^{3x}(x^{2}-2x) - \frac{1}{9}e^{3x}(2x-2) + \frac{2}{27} e^{3x} + C \\
v = e^{3x}\left( \frac{1}{3}x^{2} - \frac{2}{3}x - \frac{2}{9}x + \frac{2}{9} + \frac{2}{27} \right) + C \\
v = e^{3x}\left( \frac{1}{3}x^{2} - \frac{8}{9}x + \frac{8}{27} \right) + C \\
\end{gather}$$

$$\begin{gather}
y = uv = e^{-3x}\cdot e^{3x}\left( \frac{1}{3}x^{2} - \frac{8}{9}x + \frac{8}{27} \right) + Ce^{-3x} \\
y = \frac{1}{3}x^{2} - \frac{8}{9}x + \frac{8}{27} + Ce^{-3x} \\
\end{gather}$$

### 1.2

$$\begin{gather}
y'+3y = x^{2} - 2x \\
\lambda +3 = 0 \\
\lambda = -3 \\
y_{оо} = Ce^{-3x} \\
y_{чн} = a_{0}x^{2} + a_{1}x + a_{2} \\
2a_{0}x + a_{1} + 3a_{0}x^{2} + 3a_{1}x + 3a_{2} = x^{2} - 2x \\
\end{gather}$$

$$\begin{gather}
\begin{cases}
3a_{0} = 1 \\
2a_{0} + 3a_{1} = -2 \\
a_{1} +3a_{2} = 0
\end{cases} \\
\begin{cases}
a_{0} = \frac{1}{3} \\
a_{1} = \frac{-2-\frac{2}{3}}{3} = -\frac{8}{9} \\
a_{2} = \frac{8}{27}
\end{cases} \\
\end{gather}$$

$$\begin{gather}
y_{чн} = \frac{x^{2}}{3} - \frac{8x}{9} + \frac{8}{27} \\
y_{он} = Ce^{-3x} + \frac{x^{2}}{3} - \frac{8x}{9} + \frac{8}{27}
\end{gather}$$

### Поиск частного решения

$$\begin{gather}
y(0) = -2 \implies \frac{8}{27} + C = -2 \\
C = -\frac{62}{27} \\
y_{\mathrm{ч}} = \frac{1}{3} x^{2} - \frac{8}{9}x + \frac{8}{27} - \frac{62}{27}e^{-3x} \\
\end{gather}$$
