---
tags:
  - homework
  - 2nd-semester
  - 2024-09-23
---

## 3

$$\begin{gather}
a_{n} = \frac{\arctan(3 + 2 \cdot (-1)^{n})}{\sqrt{ n }} \tan \frac{1}{\sqrt{ n }} \\
\frac{1}{n}\tan \frac{1}{n} \sim \frac{\arctan 1}{n}\tan \frac{1}{n} \leq \frac{\arctan(1)}{\sqrt{ n }} \tan \frac{1}{\sqrt{ n }} \leq a_{n} \leq \frac{\arctan(5)}{\sqrt{ n }} \tan \frac{1}{\sqrt{ n }} \\
\lim_{ n \to \infty } \frac{\frac{1}{n+1} \tan \frac{1}{n+1}}{\frac{1}{n}\tan \frac{1}{n}} = \lim_{ n \to \infty } \frac{n \tan \frac{1}{n+1}}{(n+1)\tan \frac{1}{n}} = \lim_{ n \to \infty } \left( \frac{n}{n+1} \cdot \frac{\tan\frac{1}{n+1}}{\tan \frac{1}{n}} \right) = \\
= \lim_{ n \to \infty } \frac{\tan\frac{1}{n+1}}{\tan \frac{1}{n}} = \lim_{ n \to \infty } \frac{\cos ^{2} \frac{1}{n} \cdot \frac{1}{(n+1)^{2}}}{\cos ^{2} \frac{1}{n+1} \cdot \frac{1}{n^{2}}} = \lim_{ n \to \infty } \frac{\cos ^{2} \frac{1}{n}}{\cos ^{2} \frac{1}{n+1}} = \\
= \frac{1}{1} = 1 \\
\end{gather}$$

$$\begin{gather}

\end{gather}$$

## 5

$$\begin{gather}
a_{n} = \frac{\sqrt{ n+2 }}{n+3} \ln \frac{3n+1}{3n-1} \\
a_{n} \leq \frac{\sqrt{ n+2 }}{n} \ln \frac{n + 1}{n} = b_{n} \\
\lim_{ n \to \infty }  \frac{\frac{\sqrt{ n+3 }}{n+1}\ln \frac{n+2}{n+1}}{\frac{\sqrt{ n+2 }}{n} \ln \frac{n+1}{n}} = \lim_{ n \to \infty } \frac{n\sqrt{ n+3 }}{(n+1)\sqrt{ n+2 }} \cdot \lim_{ n \to \infty } \frac{\frac{n+1}{n+2}}{\frac{n}{n+1}} = 1 \cdot 1 = 1 \\
\int_{1}^{+\infty} \frac{\sqrt{ x+2 }}{x} \ln \frac{x+1}{x} \, dx
\end{gather}$$

## 6 
- [x] 
$$\begin{gather}
a_{n} = \frac{1}{n^{3}} \left( \frac{3n^{2} + 4}{2n^{2} + 3} \right)^{n} \\
\lim_{ n \to \infty } \sqrt[n]{ a_{n} } = \lim_{ n \to \infty } \frac{1}{n^{3/n}} \cdot \frac{3n^{2}+4}{2n^{2}+3} = \frac{3}{2} \lim_{ n \to \infty } n^{-3/n} = \\
= \frac{3}{2}\lim_{ n \to \infty } e^{-3 \cdot 1/n \cdot \ln n} = \frac{3}{2}e^{-3 \lim_{ n \to \infty } \frac{\ln n}{n}} = \frac{2}{3} e^{-3 \cdot (-\infty)} = \infty \implies a_{n} - \text{расх}
\end{gather}$$

## 8
- [x] 
$$\begin{gather}
a_{n} = \frac{(n+1)!}{7^{n}(n^{2}+4)^{3}} \\
\lim_{ n \to \infty } \sqrt[n]{ a_{n} } = \sqrt[n]{ \frac{\sqrt{ 2\pi(n+1) }\left( \frac{n+1}{e} \right)^{n+1}}{7^{n}(n^{2}+4)^{3}}} = \lim_{ n \to \infty } \frac{ (2\pi(n+1))^{1/2n} \left( \frac{n+1}{e} \right)^{\frac{n+1}{n}}}{7(n^{2}+4)^{3/n}} = \\
= \lim_{ n \to \infty }  \frac{e^{\ln (2\pi(n+1))/2n} e^{\ln ((n+1)/e) \cdot (n+1)/n}}{7e^{\ln (n^{2}+4) \cdot 3/n}} = \\
= \frac{1}{7} e^{\lim_{ n \to \infty } \left(\ln(2\pi(n+1))/2n + \ln((n+1)/e)\cdot(n+1)/n - 3\ln(n^{2}+4)/n\right)} = \\
= \dots = +\infty \implies a_{n} - \text{расх.}
\end{gather}$$

## 10

$$\begin{gather}
a_{n} = \left( \sqrt{ n^{2}+1 } - n + 1 \right)^{-n^{2}} \\
\lim_{ n \to \infty } \sqrt[n]{ a_{n} } = \lim_{ n \to \infty } \left( \sqrt{ n^{2}+1 } - n + 1 \right)^{-n} = 
\end{gather}$$

## 13

$$\begin{gather}
a_{n} = \left( \sqrt{ n }\tan \frac{1}{\sqrt{ n }} \right)^{n\sqrt{ n^{2}+n}}
\end{gather}$$

## 20

$$\begin{gather}
a_{n} = \frac{1}{n(\ln n)^{3/2} (\ln \ln n)^{2}}, \ n > 2
\end{gather}$$