---
tags:
  - homework
  - 2nd-semester
  - 2024-10-05
---

## 2

$$\begin{gather}
\sum_{n=1}^{\infty} \frac{(-1)^{n-1}\sqrt[3]{ n+1 }}{\sqrt{ n }+2} \\
|a_{n}| = \frac{\sqrt[3]{ n+1 }}{\sqrt{ n }+2} < \frac{\sqrt[3]{ n+1 }}{\sqrt{ n }} \sim n^{-1/6} = \frac{1}{n^{1/6}} - \text{расх.}, \ \frac{1}{6} < 1 \implies \\
\implies |a_{n}| - \text{расх.} \implies \text{абс. сх. нет} \\
1) \ \lim_{ n \to \infty } a_{n} = 0 \\
2) \ \frac{\sqrt[3]{ n+1 }}{\sqrt{ n }+2} < \frac{\sqrt[3]{ n+1 }}{\sqrt{ n }}, \ \left( \frac{\sqrt[3]{ x+1 }}{\sqrt{ x }} \right)' = \frac{\frac{\sqrt{ x }}{3\sqrt[3]{ (x+1)^{2} }} + \frac{\sqrt[3]{ x+1 }}{2\sqrt{ x }}}{x} = \frac{5x+3}{x} \\
3) f' = 0 \implies 5x+3 = 0 \implies x = -\frac{3}{5}
\end{gather}$$