---
tags:
  - homework
  - 2nd-semester
  - 2024-09-14
---
## I

### 3

$$\begin{gather}
a_{n} = \frac{\sin ^{2} 3n}{n\sqrt{ n }} \\
0 \leq \frac{\sin ^{2} 3n}{n\sqrt{ n }} \leq \frac{1}{n^{3/2}} - \text{сходится}, \ \frac{3}{2} > 1 \implies \\
\implies a_{n} - \text{сходится}
\end{gather}$$

### 5

$$\begin{gather}
a_{n} = \sin \frac{3+(-1)^{n}}{n^{2}} \\
\sin \frac{2}{n^{2}} \leq \sin \frac{3+(-1)^{n}}{n^{2}} \leq \sin \frac{4}{n^{2}} \sim \frac{4}{n^{2}} = 4\cdot \frac{1}{n^{2}} - \text{сходится}, \ 2 > 1 \implies \\
\implies a_{n} - \text{сходится по пр. ср.}
\end{gather}$$

### 6

$$\begin{gather}
a_{n} = \frac{\arctan(n^{2}+2n)}{n^{2}+3^{n}} \\
\frac{\arctan 3}{n^{2} + 3^{n}} \leq \frac{\arctan(n^{2}+2n)}{n^{2}+3^{n}} < \frac{\frac{\pi}{2}}{n^{2} + 3^{n}} - \text{сходится}, \ 2 > 1, \ \frac{1}{3} < 1 \implies \\
\implies a_{n} - \text{сходится}
\end{gather}$$

## II

### 2

$$\begin{gather}
a_{n} = \ln\left( 1+\frac{1}{n\sqrt[3]{ n }} \right) \\
b_{n} = \frac{1}{n^{4/3}} \\
\lim_{ n \to \infty } \frac{a_{n}}{b_{n}} = \frac{\ln\left( 1+\frac{1}{n\sqrt[3]{ n }} \right)}{\frac{1}{n^{4/3}}} = \lim_{ n \to \infty } \frac{a_{n}}{b_{n}} = \frac{\frac{1}{n\sqrt[3]{ n }}}{\frac{1}{n^{4/3}}} = \lim_{ n \to \infty }  \frac{1}{1} = 1 \neq 0 \implies \\
\implies a_{n}, b_{n} - \text{сх. / расх.}, b_{n} - \text{сх. по пр. ср.} \implies \\
\implies a_{n} - \text{сх.}
\end{gather}$$

### 4

$$\begin{gather}
a_{n} = \frac{n^{3} + 3n^{2} + 5}{n\sqrt[5]{ n^{16} + n^{4} + 1 }} \\
b_{n} = \frac{n^{3}}{n\sqrt[5]{ n^{16} }} \\
\lim_{ n \to \infty } \frac{a_{n}}{b_{n}} \frac{\frac{n^{3} + 3n^{2} + 5}{n\sqrt[5]{ n^{16} + n^{4} + 1 }}}{\frac{n^{3}}{n\sqrt[5]{ n^{16} }}} = \lim_{ n \to \infty } \frac{n^{36/5} \cdot \dots}{n^{36/5} \cdot \dots} = \lim_{ n \to \infty } \frac{1}{1} = 1 \neq 0 \implies a_{n}, b_{n} - \text{сх. / расх.} \\
b_{n} = \frac{1}{n\sqrt[5]{ n }} - \text{расх.}, \ \frac{6}{5} > 1 \implies a_{n} - \text{сх.}
\end{gather}$$

### 6

$$\begin{gather}
a_{n} = \ln \frac{1}{\cos\left( \frac{2\pi}{n} \right)}, \ n = 6,7,\dots \\
a_{n} = -\ln \cos \frac{2\pi}{n} \\
\begin{bmatrix}
1-\frac{x^{2}}{2} \sim \cos x, \ x\to 0 \\
\ln(1+x) \sim x, \ x\to 0
\end{bmatrix} \\
b_{n} = \frac{1}{n^{2}} \\
\lim_{ n \to \infty } \frac{a_{n}}{b_{n}} = \frac{-\ln \cos \frac{2\pi}{n}}{\frac{1}{n^{2}}} = \lim_{ n \to \infty } \frac{-\left( -\frac{4\pi^{2}}{n^{2}} \right)}{\frac{1}{n^{2}}} = \\
= 4\pi^{2}\lim_{ n \to \infty } \frac{1}{1} = 4\pi^{2} \neq 0 \implies a_{n}, b_{n} - \text{сх./расх.} \\
b_{n} - \text{сх.}, \ 2 > 1 \implies a_{n} - \text{сх.}
\end{gather}$$

## III

### 2

$$\begin{gather}
a_{n} = \frac{2\cdot 5\cdot 8\cdot \dots \cdot(3n-1)}{1\cdot 6\cdot 11\cdot \dots \cdot (5n-4)} \\
a_{n+1} = \frac{2\cdot 5\cdot 8\cdot \dots \cdot(3n+2)}{1\cdot 6\cdot 11\cdot \dots \cdot (5n+1)} \\
\lim_{ n \to \infty } \frac{a_{n+1}}{a_{n}} = \lim_{ n \to \infty } \frac{\frac{3n-1}{5n-4} \cdot \frac{3n+2}{5n+1}}{\frac{3n-1}{5n-4}} = \lim_{ n \to \infty } \frac{3n+2}{5n+1} = \frac{3}{5} < 1 \implies a_{n} - \text{сх.}
\end{gather}$$

### 6

$$\begin{gather}
a_{n} = \frac{5^{2n}(n!)^{3}}{(3n)!} \\
a_{n+1} = \frac{5^{2n + 2}(n+1)^{3}(n!)^{3}}{(3n+3)(3n+2)(3n+1)(3n)!} \\
\lim_{ n \to \infty } \frac{a_{n+1}}{a_{n}} = \lim_{ n \to \infty } \frac{\frac{5^{2n + 2}(n+1)^{3}(n!)^{3}}{(3n+3)(3n+2)(3n+1)(3n)!}}{\frac{5^{2n}(n!)^{3}}{(3n)!}} = \\
= \lim_{ n \to \infty } \frac{25(n+1)^{3}}{(3n+3)(3n+2)(3n+1)} = \frac{25}{27} < 1 \implies a_{n} - \text{сх.}
\end{gather}$$

## IV

### 2

$$\begin{gather}
a_{n} = \left( \frac{\sqrt{ n }+2}{\sqrt{ n }+3} \right)^{n\sqrt{ n }} \\
\sqrt[n]{ a_{n} } = \left( \frac{\sqrt{ n }+2}{\sqrt{ n }+3} \right)^{\sqrt{ n }} \\
\lim_{ n \to \infty } \sqrt[n]{ a_{n} } = \left( \frac{\sqrt{ n }+2}{\sqrt{ n }+3} \right)^{\sqrt{ n }} = \lim_{ n \to \infty } \left( \frac{1+\frac{2}{\sqrt{ n }}}{1+\frac{3}{\sqrt{ n }}} \right)^{\sqrt{ n }} =  \\
\end{gather}$$

## V

### 2

$$\begin{gather}

\end{gather}$$