---
tags:
  - seminar
  - 2nd-semester
  - 2024-10-22
---

## Звезда Ходжа

> [!definition] Звезда Ходжа
> $$\begin{gather}
> (*T)_{\underbrace{i\dots l}_{n-q}} = \frac{1}{q!}\epsilon_{\underbrace{i\dots lj\dots k}_{n}}T^{\underbrace{j\dots k}_{q}}, \ (0,n-1) \overset{*}{\leftrightarrow} (q,0), \\
  \text{где} \ *T - \text{тензор, дуальный} \ T
> \end{gather}$$

$$\begin{gather}
C_{n}^{q} = C_{n}^{n-q} = \frac{n!}{q!(n-q)!} \\
**T = (-1)^{q(n-q)}T \\
\end{gather}$$

$$\begin{gather}
\mathbb{R}^{2}: *(dx^{i}\wedge dx^{j}) = \epsilon^{ij} \\
\mathbb{R}^{3}: *(dx^{i}\wedge dx^{j}) = \epsilon^{ijk}\vec{e}_{k} \\
*\vec{e}_{i} = \frac{1}{2}\epsilon_{ijk}dx^{j}\wedge dx^{k}
\end{gather}$$

$$\begin{gather}
*(\tilde{u}\wedge\tilde{v}) = \vec{w} = \vec{u} \times \vec{v} \\
*(\tilde{u}\wedge\tilde{v}\wedge\tilde{w}) = \langle \tilde{u},\tilde{v},\tilde{w} \rangle = V
\end{gather}$$

### Примеры

1. Найти $*((2dx^{1} + 3dx^{2})\wedge(dx^{1} - dx^{2}))$ в $\mathbb{R}^{2}$ и $\mathbb{R}^{3}$

$$\begin{gather}
*(2dx^{1}\wedge dx^{1} - 2dx^{1}\wedge dx^{2} + 3dx^{2}\wedge dx^{1} - 3dx^{2}\wedge dx^{2}) = *(-5dx^{1} \wedge dx^{2}) \\
\mathbb{R}^{2}: \ -5 \\
\mathbb{R}^{3}: \ -5e^{123}\vec{e_{3}} = -5\vec{e_{3}} \\
\end{gather}$$

2. Найти $*((dx^{1}-3dx^{2})\wedge(dx^{1}-dx^{2})\wedge(dx^{1}-4dx^{3}))$ в $\mathbb{R}^{3}, \ \mathbb{R}^{4}$

$$\begin{gather}
*((dx^{1}-3dx^{2})\wedge(dx^{1}-dx^{2})\wedge(dx^{1}-4dx^{3})), \ \mathbb{R}^{3}, \ \mathbb{R}^{4} \\
\mathbb{R}^{3}: \ -8 \\
\mathbb{R}^{4}: \ -9\epsilon^{1234}\vec{e}_{4} = -8\vec{e}_{4}
\end{gather}$$

3. Найти $*((-2dx^{1}+2dx^{2})\wedge(dx^{1}\wedge dx^{2} + 4dx^{1}\wedge dx^{3}))$ в $\mathbb{R}^{3}$ и $\mathbb{R}^{4}$

$$\begin{gather}
*((-2dx^{1}+2dx^{2})\wedge(dx^{1}\wedge dx^{2} + 4dx^{1}\wedge dx^{3})) = *(8dx^{2}\wedge dx^{1}\wedge dx^{3}) = \\
*(-8dx^{1}\wedge dx^{2}\wedge dx^{3}) \\
\mathbb{R}^{3}: \ -8\epsilon^{123} = -8 \\
\mathbb{R}^{4}: \ -8\epsilon^{1234}\vec{e}_{4} = -8\vec{e}_{4} \\
\end{gather}$$

4. Показать, что произведение 1 и 2-форм в $\mathbb{R}^{3}$ $\tilde{\omega}_{a} = a_{i}dx^{i}, \ \tilde{\omega}_{b} = b_{ij}dx^{i}\wedge dx^{j}$ выражается чере