---
aliases: 
tags:
  - homework
  - 2024-02-29
  - 2nd-semester
---

## 23

$$
\begin{gather}
\int \frac{4-3x}{\sqrt{ x^{2}-8x+20 }} \, dx  = \\ 
= \begin{vmatrix}
\sqrt{ x^{2}-8x+20} = \sqrt{ (x-4)^{2}+2^{2} } \\
(\sqrt{ x^{2}+8x+20 })'=\frac{\cancelto{ x-4 }{ 2x-8 }}{2\sqrt{ x^{2}-8x+20 }}
\end{vmatrix} =\int \frac{-\frac{1}{3}(x-4)+\frac{8}{3}}{\sqrt{ x^{2}-8x+20 }} \, dx  = \\ \\
=  -\frac{1}{3}\int  \, d(\sqrt{ x^{2}-8x+20 }) + \frac{8}{3}\int  \frac{d(x-4)}{\sqrt{ (x-4)^{2} +2^{2}}} \,  = \\ 
= \frac{8}{3}\ln |(x+4)+\sqrt{ x^{2}-8x+20 }| -\frac{1}{3}\sqrt{ x^{2}-8x+20 }+C
\end{gather}
$$

## 24

$$
\begin{gather}
\int \frac{2x+11}{3x^{2}+12x+7} \, dx =2\int  \, \frac{xdx}{3x^{2}+12x+7}+11\int  \, \frac{dx}{3x^{2}+12x+7} = \\ 
= 2 \cdot \int \frac{\frac{1}{6} \cdot (6x+12)-2}{3x^{2}+12x+7} \, dx + 11\int \frac{1}{3x^{2}+12x+7} \, dx  = \\ 
= \frac{1}{3}\ln |3x^{2}+12x+7|-9\int \frac{1}{3x^{2}+12x+7} \, dx  = \\ 
=    \frac{1}{3}\ln |3x^{2}+12x+7|-3\int \frac{1}{(x^{2}+4x+4)-\frac{5}{3}} \, dx  = \\ 
=   \frac{1}{3}\ln |3x^{2}+12x+7| + \frac{9}{10}\ln | \frac{x+\frac{1}{3}}{x-\frac{1}{3}}|+C
\end{gather}
$$


## 25

$$
\begin{gather}
\int \frac{(x+6)}{-x^{2}+3x+4} \, dx = \int  \, \frac{xdx}{-x^{2}+3x+4} +6 \int   \, \frac{dx}{-x^{2}+3x+4}  = \\ 
*\  \int  \, \frac{xdx}{-x^{2}+3x+4} = \\ 
= -\frac{1}{2}\int \frac{-2x+3}{-x^{2}+3x+4} \, dx+ \frac{3}{2}\int  \, \frac{dx}{-x^{2}+3x+4}  = \\ 
= -\frac{1}{2}\ln |-x^{2}+3x+4|+ \frac{3}{2} \int  \, \frac{dx}{-x^{2}+3x+4} *\\ \\ 
= -\frac{1}{2}\ln |-x^{2}+3x+4|-\frac{3}{2}\ln | \frac{x+\frac{3}{2}-\frac{5}{2}}{x+\frac{3}{2}+\frac{5}{2}}|+C
\end{gather}
$$

## 7.76

$$
\begin{gather}
\int  \, \frac{dx}{(a-b)x^{2}-(a+b)} =-\int  \, \frac{dx}{\sqrt{ (a+b) }^{2}-(\sqrt{ a-b }x)^{2}} = \\ 
= -\frac{1}{2\sqrt{ a+b }}\ln | \frac{\sqrt{ a+b }+\sqrt{ a-b }x}{\sqrt{ a+b }-\sqrt{ a+b }x}|+C
\end{gather}
$$
## 7.78

$$
\begin{gather}
\int \frac{xdx}{4y^{2} + 7} \, = \frac{1}{8}\int \frac{1}{4x^{2}+7}  \, d(4x^{2}+7)=\frac{1}{8}\ln |4x^{2} + 7|+C   
\end{gather}
$$

## 7.80

$$
\begin{gather}
\int \frac{a^{x}}{\sqrt{ a^{2x}-1 }} \, dx =  \frac{1}{\ln a}\int \frac{1}{\sqrt{ a^{2x}-1 }} \, d(a^{x}) = \\ 
= \frac{1}{\ln a} \cdot \ln |a^{y}+\sqrt{ a^{2x}-1 }|+C 
\end{gather}
$$

## 7.82

$$
\begin{gather}
\int \frac{x^{2}}{3+x^{2}} \, dx =\int \frac{x^{2}+3-3}{x^{2}+3} \, dx =\int  \, dx -3\int  \frac{1}{x^{2}+3} \, dx  = \\ 
= x-3 \cdot \frac{1}{\sqrt{ 3 }}\arctan \frac{x}{\sqrt{ 3 }}+C 
\end{gather}
$$

## 7.84

$$
\begin{gather}
\int \frac{x}{a^{2}x^{4}-b^{2}} \, dx =\frac{1}{2} \int \frac{1}{a^{2}x^{4}-b^{2}} \, dx^{2} = \frac{1}{2}  \cdot  \frac{1}{2b} \ln | \frac{ax^{2}-b}{ax^{2}+b}|+C  
\end{gather}
$$

## 7.86

$$
\begin{gather}
\int \frac{(x^{4}+1)}{x^{5}+5x-8} \, dx = \begin{vmatrix}
d(x^{5}+5x-8)=(5x^{4}+5)dx
\end{vmatrix}  = \\ 
= \frac{1}{5}\int \frac{1}{x^{5}+5x-8} \, d(x^{5}+5x-8)  = \\ 
= \frac{1}{5} \cdot \ln |x^{5}+5x-8|+C
\end{gather}
$$

## 7.88

$$
\begin{gather}
\int \left( 3-\frac{x}{\sqrt{ x^{2}-1 }} \right)  \cdot  \frac{dx}{\sqrt{ x^{2}+1 }} \, = 3 \int   \, \frac{dx}{\sqrt{ x^{2}+1 }}-\int  \, \frac{xdx}{x^{2}+1} = \\ 
= 3 \ln |x+\sqrt{ x^{2}+1 }|-\frac{1}{2}\ln |x^{2}+1|+C 
\end{gather}
$$
## 7.90

$$
\begin{gather}
\int  \frac{a^{2}+\sqrt{ a^{2}+b^{2}x^{2} }}{a^{2}+b^{2}x^{2}} \, dx = a^{2}\int \frac{1}{a^{2}+b^{2}x^{2}} \, dx + \int \frac{1}{\sqrt{ a^{2}+b^{2}x^{2} }} \, dx = \\ 
= \frac{a^{2}}{b} \int  \frac{1}{bx^{2}+a^{2}} \, d(bx) + \frac{1}{b} \int \frac{1}{\sqrt{ b^{2}x^{2}+a^{2} }} \, d(bx) = \\ 
= \frac{a^{2}}{b} \cdot \frac{1}{a}\arctan \frac{bx}{a} + \frac{1}{b} \cdot \ln |bx+\sqrt{ b^{2}x^{2}+a^{2} }|+C   
\end{gather}
$$

## 7.92

$$
\begin{gather}
\int e^{x}\sqrt[3]{ 4+e^{x} } \, dx = \int \sqrt[3]{ 4+e^{x} } \, d(e^{x}+4)  = \\ 
= \int (e^{x}+4)^{\frac{1}{3}} \, d(e^{x}+4)=\frac{3}{4} \cdot (e^{x}+4)^{\frac{4}{3}}+C  
\end{gather}
$$

