---
tags:
  - seminar
  - 2nd-semester
  - 2024-02-28
  - геома
---

#TODO Вынести
## Однородные ф-ции

$$\begin{gather}
f(tp) = t^{m}f(p), \ \forall t \in \mathbb{R}, \ t \neq 0 \\
\phi(tp) = t^{\mu}\phi(p) \\
\end{gather}$$

$$\begin{align}
&1) \ f\pm \phi = \psi \\
&2) \ f\phi = \psi \\
&3) \ \frac{f}{\phi} = \psi
\end{align}$$

#TODO Вынести
## 4) Теорема Эйлера об однородных ф-циях

$$x_{1}f'_{x_{1}}(p) + x_{2}f'_{x_{2}}(p) + \dots + x_{n}f'_{x_{n}}(p) = mf(p)$$

### Примеры

#### 8.75

$$\begin{gather}
z= \frac{y}{x^{3}-y^{3}} \\
z(tx,ty)= \frac{ty}{t^{3}(x^{3}-y^{3})} \\
z(tx, ty)= \frac{y}{t^{2}(x^{3}-y^{3})} \\
t^{-2} \implies m = -2\\
x \cdot \left( \frac{1}{(x^{3}-y^{3})^{2}} \right)\cdot 3x^{2} + \frac{x^{3}-y^{3}+3y^{2}}{(x^{3}-y^{3})^{2}} \cdot y = \\ 
=  \frac{-3x^{3}}{(x^{3}-y^{3})^{2}}+ \frac{-3x^{3}+x^{3}y+y^{4}}{(x^{3}-y^{3})^{2}}  = \\ 
= \frac{-2x^{3}y+2y^{4}}{(x^{3}-y^{3})^{2}}=-2y \cdot \frac{y}{x^{3}-y^{3}}
\end{gather}$$

## Оператор Лапласа

$$\Delta = \frac{\partial^{2}}{\partial x^{2}}\vec{i} + \frac{\partial^{2}}{\partial y^{2}}\vec{j}$$

$$\Delta u = \frac{\partial^{2} u}{\partial x^{2}} + \frac{\partial^{2} u}{\partial y^{2}}$$

### Примеры

#### 8.83

$$\begin{gather}
u = \frac{1}{2a\sqrt{ \pi \ t }}\underbrace{ e^{- \frac{(x-x_{0})^{2}}{4a^{2}t}} }_{ \beta } \\
\text{ удв. } \frac{ \partial u }{ \partial t } =a^{2} \frac{ \partial^{2} u }{ \partial^{2} x } \\
\text{ проверим: } \\ \\
\frac{ \partial u }{ \partial t } = \left( - \frac{1}{(2a\sqrt{ \pi \ t })^{2} } \cdot  \frac{\pi}{2\sqrt{ \pi \ t }} \right) \cdot \beta+\beta  \cdot 4a  \cdot  \frac{(x-x_{0})^{2}}{(4a^{2}t)^{2}} \cdot  \left( \frac{1}{2a\sqrt{ \pi  \cdot t }} \right)  = \\ 
(=) \frac{\beta}{t^{2} \cdot 4a\sqrt{ \pi  \cdot t }}\left( -\frac{1}{\pi}+ \frac{(x-x_{0})^{2}}{2a^{2}} \right)  \\
\end{gather}$$

$$\begin{gather}
\frac{ \partial u }{ \partial x } = \frac{1}{2a \sqrt{ \pi t }}e^{-\frac{(x-x_{0})^{2}}{4a^{2}t}}=2(x-x_{0}) \\
\frac{ \partial^{2} u }{ \partial x^{2} }=\frac{1}{2a \sqrt{ \pi t }}e^{-\frac{(x-x_{0})^{2}}{4a^{2}t}} \cdot (2(x-x_{0}))^{2}+ \frac{1}{2a\sqrt{ \pi  \cdot t }}e^{-\frac{(x-x_{0})^{2}}{4a^{2}t}} \cdot 2 \\
a^{2}\frac{ \partial^{2} u }{ \partial x^{2} } = \frac{1}{a\sqrt{ \pi  \cdot t}}\beta  \cdot 2(x-x_{0})^{2}+ \frac{1}{a\sqrt{ \pi  \cdot t }}\beta \ ????????? \\
\frac{ \partial u }{ \partial x } =\alpha\beta\left( \frac{-2(x-x_{0})}{4a^{2}t} \right) \\
\frac{ \partial^{2} u }{ \partial x^{2} }=\alpha\beta  \cdot \left( \frac{+2 \cdot (x-x_{0})}{4a^{2}t} \right)^{2}+\alpha\beta \frac{-2}{4a^{2}t} \\
\frac{ \partial u }{ \partial t } = \frac{???}{-(2a\sqrt{ \pi  \cdot t })^{2}} \\
\end{gather}$$

$$\begin{gather}
\frac{1}{2a\sqrt{ \pi }}(t)^{\frac{-1}{2}}= \frac{-\frac{1}{2}t^{\frac{-3}{2}}}{2a\sqrt{ \pi }} =\frac{1}{2a}(\pi t)^{\frac{-1}{2}}= \frac{-\pi(\pi t)^{\frac{-3}{2}}}{2 \cdot 2a} = \\ 
= \frac{-\pi}{4a\sqrt{ (\pi t)^{3} }}= \frac{-\pi}{4a\pi t\sqrt{ \pi t }} \\
\frac{ \partial u }{ \partial t } = \frac{-1}{4at\sqrt{ \pi  \cdot t }}e^{-\frac{(x-x_{0})^{2}}{4a^{2}t}}+ \frac{-1}{2at\sqrt{ \pi  \cdot t }} \cdot \beta  \cdot \beta  \cdot  \frac{1}{t^{2}} \cdot \frac{(x-x_{0})^{2}}{4a^{2}} \\
\left( e^{-\frac{(x-x_{0})^{2}}{4a^{2}t}} \right)'=\beta  \cdot \left( + \frac{(x-x_{0})^{2}}{4a^{2}}  \right) \cdot  \frac{+1}{t^{2}}  = \\ 
= \beta  \cdot \left( \frac{-1}{4at\sqrt{ \pi  \cdot t }}- \frac{(x-x_{0})^{2}}{8at\sqrt{ \pi t }  \cdot t^{2} \cdot 4a^{2}}  \right)  = \\ 
= \beta\left(  \right)
\end{gather}$$

$$\begin{gather}
\frac{ \partial^{2} u }{ \partial x^{2} } = - \frac{1}{2a\sqrt{ \pi \ t }} \cdot \beta  \cdot  \left( \frac{+2(x-x_{0})}{4a^{2}t} \right)^{2}+ \frac{1}{2a\sqrt{ \pi t }}\beta  \cdot \frac{-2}{4a^{2}t} \\
a^{2} \frac{ \partial^{2} u }{ \partial x^{2} }=\frac{(x-x_{0})^{2}}{8a^{3}t^{2}\sqrt{ \pi t }}\beta- \frac{1}{4at\sqrt{ \pi t }}=\frac{ \partial u }{ \partial t } \\ 
\end{gather}$$

>[!NOTE]
> Витя наcooking ошибок, я не буду это разбирать ))))))
