---
tags:
  - seminar
  - 2nd-semester
  - 2024-03-27
  - геома
---

## 8.148(2)

$$\begin{gather}
\frac{\partial z}{\partial y} = -\frac{\frac{\partial f}{\partial y}}{\frac{\partial f}{\partial z}} = -\frac{f'_{u}u'_{y}+f'_{v}v'_{y}}{f'_{u}u'_{z}+f'_{v}v'_{z}} = -\frac{f'_{u}\cdot z}{f'_{u}\cdot y + f'_{v} \cdot xe^{xz}}
\end{gather}$$

## 8.150

$$\begin{gather}
dz - ?, \ xz-e^{z/y}+x^{3}+y^{3} = 0 \\
\frac{\partial f}{\partial x}dx + \frac{\partial f}{\partial y}dy + \frac{\partial f}{\partial z}dz = 0 \\
\left( z + x\cdot \frac{\partial z}{\partial x} - \frac{e^{z/y}}{y} \cdot \frac{\partial z}{\partial x} +3x^{2} \right)dx + \\
+ \left( x\cdot \frac{\partial z}{\partial y} - e^{z/y} \cdot \left( \frac{\partial z}{\partial y} \cdot \frac{1}{y} + z \cdot \left( -\frac{1}{y^{2}} \right) \right) + 3y^{2} \right)dy + \\
+ \left( x - \frac{e^{z/y}}{y} \right)dz = 0 \\
\frac{\partial z}{\partial x} \ : \ 
\end{gather}$$

## 3398

$$\begin{gather}
F(xz;yz) = 0, \ \frac{\partial^{2} z}{\partial x^{2}} - ? \\
\frac{\partial z}{\partial x} = -\frac{F'_{u}\cdot u'_{x} + F'_{v}\cdot v'_{x}}{F'_{u}\cdot u'_{z} + F'_{v}\cdot v'_{z}} = -\frac{F'_{u}\cdot z + F'_{v}\cdot 0}{F'_{u}\cdot x + F'_{v}\cdot y} = -\frac{zF'_{u}}{xF'_{u}+yF_{v}'}\\
\frac{\partial^{2}z}{\partial x^{2}} = -\frac{\frac{\partial }{\partial x}\left( -\frac{zF'_{u}}{xF'_{u}+yF'_{v}} \right)}{\frac{\partial }{\partial z}\left( -\frac{zF'_{u}}{xF'_{u}+yF'_{v}} \right)} = \dots
\end{gather}$$

## Система неявно заданных функций

$$\begin{gather}
\begin{cases}
F(x,y,z) = 0 \\
G(x,y,z) = 0
\end{cases}, \ y = y(x), \ z = z(x)
\end{gather}$$

> [!note]
> Существование решения для указанной системы:
> $$\frac{\partial y}{\partial x}, \frac{\partial z}{\partial x} \neq 0$$

## 8.157

$$\begin{gather}
\begin{cases}
7x^{2}+y^{2}-3z^{2}=-1 \\
4x^{2}+2y^{2}-3z^{2}=0
\end{cases} \\
\begin{cases}
14x+2y\cdot y'_{x}-6z\cdot z'_{x}=0 \\
8x+4y\cdot y'_{x}-6z\cdot z'_{x}=0 \\
\end{cases} \\
\left(\begin{array}{cc|c}
2y & -6z & -14x \\
4y & -6z & -8x
\end{array}\right) \sim 
\left(\begin{array}{cc|c}
2y & -6z & -14x \\
0 & 6z & 20x
\end{array}\right) \sim
\left(\begin{array}{cc|c}
2y & 0 & 6x \\
0 & 6z & 20x
\end{array}\right) \implies \\
\implies \frac{\partial y}{\partial x} = \frac{3x}{y}, \ \frac{\partial z}{\partial x} = \frac{10x}{3z}
\end{gather}$$

