---
tags:
  - типовой-расчет
  - 2nd-semester
  - 31-05-2024
---

# Алгебра и геометрия ТР 8

## Ершов Алексей Геннадьевич КМБО-03-23

### Вариант 4

$$\begin{gather}
[-2; -1], \ B = \langle t^{2} ; t; 1 \rangle, \ (p(t),q(t)) = \int_{-2}^{-1} p(t)q(t) \, dt 
\end{gather}$$

## 1. Ортогонализация

$$\begin{gather}
(1,1) = \int_{-2}^{-1} dt = 1 \\
(t, 1) = (1, t) = \int_{-2}^{-1} t \, dt = \frac{1}{2} - 2 = -\frac{3}{2} \\
(1, t^{2}) = (t^{2}, 1) = \int_{-2}^{-1} t^{2} \, dt = -\frac{1}{3} + \frac{8}{3} = \frac{7}{3} \\
\end{gather}$$

$$\begin{gather}
(t, t) = \int_{-2}^{-1} t^{2}  \, dt = (1, t^{2}) = \frac{7}{3} \\
(t, t^{2}) = (t^{2}, t) = \int_{-2}^{-1} t^{3} \, dt = \frac{1}{4} - 4 = -\frac{15}{4} \\
(t^{2}, t^{2}) = \int_{-2}^{-1} t^{4} \, dt = -\frac{1}{5} + \frac{32}{5} = \frac{31}{5}
\end{gather}$$

$$G = \begin{pmatrix}
1 & -\frac{3}{2} & \frac{7}{3} \\
-\frac{3}{2} & \frac{7}{3} & -\frac{15}{4} \\
\frac{7}{3} & -\frac{15}{4} & \frac{31}{5}
\end{pmatrix}$$

$$s_{1} = e_{1} = \begin{pmatrix}
1 \\
0 \\
0
\end{pmatrix} = 1$$

$$\begin{gather}
s_{2} = e_{2} - \mathrm{Proj}_{s_{1}}e_{2} = e_{2} - \frac{(e_{2}, s_{1})}{(s_{1},s_{1})}e_{1} = \\
= \begin{pmatrix}
0 \\
1 \\
0
\end{pmatrix} - \frac{-\frac{3}{2}}{1}\begin{pmatrix}
1 \\
0 \\
0
\end{pmatrix} = \begin{pmatrix}
\frac{3}{2} \\
1 \\
0
\end{pmatrix} = t+\frac{3}{2}
\end{gather}$$

$$\begin{gather}
s_{3} = e_{3} - \mathrm{Proj}_{s_{1}}e_{3} - \mathrm{Proj}_{s_{2}}e_{3} = \\
= \begin{pmatrix}
0 \\
0 \\
1
\end{pmatrix} - \frac{7}{3}\begin{pmatrix}
1 \\
0 \\
0
\end{pmatrix} \underbrace{- \frac{-\frac{1}{4}}{\frac{1}{12}}}_{+3}\begin{pmatrix}
\frac{3}{2} \\
1 \\
0
\end{pmatrix} = \begin{pmatrix}
\frac{13}{6} \\
3 \\
1
\end{pmatrix} = t^{2} +3t+\frac{13}{6}
\end{gather}$$

$$\begin{pmatrix}
0 & 0 & 1
\end{pmatrix}\begin{pmatrix}
1 & -\frac{3}{2} & \frac{7}{3} \\
-\frac{3}{2} & \frac{7}{3} & -\frac{15}{4} \\
\frac{7}{3} & -\frac{15}{4} & \frac{31}{5}
\end{pmatrix}\begin{pmatrix}
\frac{3}{2} \\
1 \\
0
\end{pmatrix} = -\frac{1}{4}$$

$$\begin{pmatrix}
\frac{3}{2} & 1 & 0
\end{pmatrix}\begin{pmatrix}
1 & -\frac{3}{2} & \frac{7}{3} \\
-\frac{3}{2} & \frac{7}{3} & -\frac{15}{4} \\
\frac{7}{3} & -\frac{15}{4} & \frac{31}{5}
\end{pmatrix}\begin{pmatrix}
\frac{3}{2} \\
1 \\
0
\end{pmatrix} = \frac{1}{12}$$

$$S = \left\langle 1; t+\frac{3}{2}; t^{2}+3t+\frac{13}{6} \right\rangle$$

## 2. Ортонормирование

$$\begin{gather}
|\vec{v}| = \sqrt{ \begin{pmatrix}
x & y & z
\end{pmatrix}\begin{pmatrix}
1 & -\frac{3}{2} & \frac{7}{3} \\
-\frac{3}{2} & \frac{7}{3} & -\frac{15}{4} \\
\frac{7}{3} & -\frac{15}{4} & \frac{31}{5}
\end{pmatrix}\begin{pmatrix}
x \\
y \\
z
\end{pmatrix} } = \\
= \sqrt{ x^{2}+\frac{7}{3}y^{2}+\frac{31}{5}z^{2}-3xy+\frac{14}{3}xz-\frac{15}{2}yz }
\end{gather}$$

$$1) \ \left(\begin{pmatrix}
1 \\
0 \\
0
\end{pmatrix},\begin{pmatrix}
1 \\
0 \\
0
\end{pmatrix}\right) = 1 \implies p_{1} = a_{1} = \begin{pmatrix}
1 \\
0 \\
0
\end{pmatrix}$$
$$\begin{gather}
2) \ p_{2} = \frac{a_{2}}{|a_{2}|} \\
|a_{2}| = \sqrt{ \left( \frac{3}{2} \right)^{2}+\frac{7}{3}\cdot 1^{2} - 3\cdot 1\cdot \frac{3}{2} } = \frac{\sqrt{ 3 }}{6} \implies \\
\implies p_{2} = \frac{6}{\sqrt{ 3 }}\begin{pmatrix}
\frac{3}{2} \\
1 \\
0
\end{pmatrix} = \begin{pmatrix}
\frac{3\sqrt{ 3 }}{4} \\
\frac{\sqrt{ 3 }}{2} \\
0
\end{pmatrix}
\end{gather}$$

$$\begin{gather}
3) \ p_{3} = \frac{a_{3}}{|a_{3}|} \\
|a_{3}| = \sqrt{ \left( \frac{13}{6} \right)^{2} + \frac{6}{3} \cdot 3^{2} + \frac{31}{5} - 3 \cdot \frac{13}{6} \cdot 3 + \frac{14}{3} \cdot \frac{13}{6} - \frac{15}{2} \cdot 3 } = \\
= \sqrt{ \frac{1}{180} } = \frac{1}{6\sqrt{ 5 }} \\
p_{3} = 6\sqrt{ 5 }\begin{pmatrix}
\frac{13}{6} \\
3 \\
1
\end{pmatrix} = \begin{pmatrix}
13\sqrt{ 5 } \\
18\sqrt{ 5 } \\
6\sqrt{ 5 }
\end{pmatrix}
\end{gather}$$

$$P = \left\langle 1; \frac{\sqrt{ 3 }}{2}t+\frac{3\sqrt{ 3 }}{4}; 6\sqrt{ 5 }t^{2}+18\sqrt{ 5 }t+13\sqrt{ 5 } \right\rangle$$
