---
tags:
  - seminar
  - 2nd-semester
  - 2024-03-20
  - геома
---

$$\begin{gather}
z = z(x,y) \implies dz = \frac{\partial z}{\partial x} dx + \frac{\partial z}{\partial y} dy \\
x = x(u,v), y = y(u,v)
\end{gather}$$

## Дифференциал функции 2-го порядка

$$\begin{gather}
d^{2}z = d(dz) \\
d\left(\frac{\partial z}{\partial x} dx + \frac{\partial z}{\partial y} dy\right) = d\left( \frac{\partial z}{\partial x} dx \right) + d\left(\frac{\partial z}{\partial y}dy\right) \\
d^{2}z = \frac{\partial^{2}x}{\partial x^{2}} dx^{2} + \frac{\partial^{2} z}{\partial x\partial y}dxdy + \frac{\partial^{2} z}{\partial y\partial x}dydx + \frac{\partial^{2}x}{\partial y^{2}} dy^{2} + \frac{\partial z}{\partial x}d^{2}x + \frac{\partial z}{\partial y}d^{2}y
\end{gather}$$

## 8.132(1)

$$\begin{gather}
z = f(u,v), \ u = xy, \ v = \frac{x}{y} \\
\frac{\partial^{2} z}{\partial x^{2}} = \frac{\partial }{\partial x}\left( \frac{\partial f}{\partial u}\cdot \frac{\partial u}{\partial x} + \frac{\partial f}{\partial v} \cdot\frac{\partial v}{\partial x}  \right) = \\
= y\cdot\frac{\partial}{\partial x}\left( \frac{\partial f}{\partial u} \right) + \frac{1}{y}\cdot \frac{\partial}{\partial x} \left( \frac{\partial f}{\partial v} \right) = \\
= y\cdot \frac{\partial}{\partial u}\left( y\cdot\frac{\partial f}{\partial u} + \frac{1}{y} \cdot \frac{\partial f}{\partial v}\right) + \frac{1}{y} \cdot \frac{\partial}{\partial v}\left( \frac{1}{y}\cdot\frac{\partial f}{\partial v} + y \cdot \frac{\partial f}{\partial u}\right) = \\
= y^{2} \frac{\partial^{2} f}{\partial  u^{2}} + 2\frac{\partial^{2} f}{\partial u\partial v} + \frac{1}{y^{2}} \frac{\partial^{2} f}{\partial v^{2}}
\end{gather}$$ 

## Неявные функции одной и нескольких независимых переменных

$$\begin{gather}
f(x,y) = 0 \\
y'(x) = \frac{dy}{dx} = -\frac{f'_{x}}{f'_{y}} \\
y''(x) = \frac{d}{dx}\left( \frac{dy}{dx} \right) = \frac{d^{2}y}{dx^{2}}
\end{gather}$$

$$\begin{gather}
f(x,y,z) = 0, \ z = z(x,y) \\
\frac{\partial z}{\partial x} = - \frac{f'_{x}}{f'_{z}}, \ \frac{\partial z}{\partial y} = - \frac{f'_{y}}{f'_{z}} \\
f'_{x}dx + f'_{u}dy + f'_{z}dz = 0 \\
dz = - \frac{f'_{x}dx+f'_{y}dy}{f'_{z}}
\end{gather}$$

## 8.146

$$\begin{gather}
\frac{\partial z}{\partial x} ,\frac{\partial z}{\partial y} - ?, \ z\ln(x+z) - \frac{xy}{z} = 0 
\end{gather}$$
