---
tags:
  - seminar
  - 2nd-semester
  - 2024-04-03
  - геома
---

$$\begin{gather}
\begin{cases}
F(x,y,u,v) = 0 \\
G(x,y,u,v) = 0
\end{cases}, \ u = u(x,y), \ v = v(x,y) \\
I = \begin{vmatrix}
\frac{\partial F}{\partial u} & \frac{\partial F}{\partial v} \\
\frac{\partial G}{\partial u} & \frac{\partial G}{\partial v}
\end{vmatrix}
\end{gather}$$

## 8.159

$$\begin{gather}
\begin{cases}
F: \ xu+yv=1 \\
G: \ x+y+u+v=0
\end{cases}
\end{gather}, \ du, \ dv, \ d^{2}u, \ d^{2}v - ?$$

$$\begin{array}{l}
\begin{cases}
udx + xdu + vdy + ydv = 0 \\
dx+dy+du+dv = 0
\end{cases} \implies \\
\implies \begin{cases}
dv = -dx-dy-du \\
udx + xdu + vdy - y(dx+dy+du) = 0
\end{cases} \implies \\
\implies \begin{cases}
dv = -dx-dy-du \\
du = \frac{-udx-vdy+ydx+ydy}{x-y}
\end{cases} \implies \\
\implies \begin{cases}
dv = -dx-dy-\frac{-udx-vdy+ydx+ydy}{x-y} \\
du = \frac{-udx-vdy+ydx+ydy}{x-y}
\end{cases} \implies \\
\implies \begin{cases}
du = \frac{(y-u)dx + (y-v)dy}{x-y} \\
dv = \frac{(x-v)dy+(x-u)dx}{y-x}
\end{cases}
\end{array}$$

$$\begin{gather}
d^{2}v = \frac{d[(y-u)dx + (y-v)dy](x-y) - [(y-u)dx + (y-v)dy]d(x-y)}{(x-y)^{2}} = \\
= \frac{[(dy-du)dx + (dy-dv)dy](x-y) - [(y-u)dx + (y-v)dy](dx-dy)}{(x-y)^{2}}
\end{gather}$$

$$\begin{gather}
d^{2}v = \frac{d[(x-v)dy+(x-u)dx](y-x) - [(x-v)dy+(x-u)dx]d(y-x)}{(y-x)^{2}} = \\
= \frac{[(dx-dv)dy+(dx-du)dx](y-x) - [(x-v)dy+(x-u)dx](dy-dx)}{(y-x)^{2}}
\end{gather}$$

## 8.161

$$\begin{gather}
\begin{cases}
x = u+v \\
y = u-v \\
z = u^{2}v^{2}
\end{cases}, \ \frac{\partial z}{\partial x}, \frac{\partial z}{\partial x} - ?
\end{gather}$$

$$\begin{gather}
\begin{cases}
dx = \frac{\partial x}{\partial u}du + \frac{\partial x}{\partial v}dv \\
dy = \frac{\partial y}{\partial u}du + \frac{\partial y}{\partial v}dv
\end{cases} \\
\begin{cases}
dx = udu + vdv \\
dy = udu - vdv
\end{cases} \\
\begin{cases}
vdv = dx - udu \\
dy = 2udu - dx
\end{cases} \\
\begin{cases}
vdv = dx - udu \\
udu = \frac{dx+dy}{2}
\end{cases} \\
\begin{cases}
dv = \frac{dx-dy}{v2} \\
du = \frac{dx+dy}{u2}
\end{cases} \\
\end{gather}$$

$$\begin{gather}
\begin{cases}
dz = \frac{\partial z}{\partial u}du + \frac{\partial z}{\partial v}dv \\
dz = \frac{\partial z}{\partial x}dx + \frac{\partial z}{\partial y}dy
\end{cases} \\
dz = (2uv^{2}) \frac{dx + dy}{2u} + (2vu^{2}) \frac{dx-dy}{2v} = v^{2}(dx+dy) + u^{2}(dx-dy) \\
\dots
\end{gather}$$