---
tags:
  - homework
  - 2nd-semester
  - 2024-09-14
---
## 1

$$\begin{gather}
\alpha(t) = (a\cos ^{3}t, a\sin ^{3}t)^{T} \\
\dot{\alpha}(t) = (-3a\cos ^{2}t\sin t, 3a\sin ^{2}t\cos t)^{T} \\
y_{k} = \frac{y'_{t}(t_{0})}{x'_{t}(t_{0})}(x-x(t_{0})) + y(t_{0})\\
y_{k} = -\tan t_{0}(x-a\cos ^{3}t_{0}) + a\sin ^{3}t_{0} \\
r = \frac{|\tan t_{0}(x-a\cos ^{3}t_{0}) + a\sin ^{3}t_{0}|}{\sqrt{ 1+\tan ^{2}t_{0} }} \\
r = \frac{|\tan t_{0}a\cos ^{3}t_{0}) + a\sin ^{3}t_{0}|}{\sqrt{ 1+\tan ^{2}t_{0} }} \to \mathrm{max} \\
r = \frac{|a\sin t_{0}|}{\sqrt{ 1+\tan ^{2}t_{0} }} \to \mathrm{max} \\
t_{0} = \frac{\pi}{4} + \frac{\pi n}{4}, \ n \in \mathbb{Z} \\
\dots \\
y = \pm x \pm \frac{a}{2\sqrt{ 2 }}
\end{gather}$$

## 2

$$\begin{gather}
r = a\phi, \phi \in [0, 2\pi) \\
\alpha(t) = (a\cos \phi, a\sin \phi)^{T} \\
\dot{\alpha}(t) = (-a\sin \phi, a\cos \phi)^{T} \\
|\dot{\alpha}(t)| = a \\
L = \int_{0}^{2\pi} a \, d\phi  = 2a\pi
\end{gather}$$

## 3

$$\begin{gather}
\alpha(t) = (a\cos t,a\sin t,bt)^{T} \\
\dot{\alpha}(t) = (-a\sin t,a\cos t,b)^{T} \\
|\dot{\alpha}(t)| = \sqrt{ a^{2} + b^{2} } \\
L = \int_{0}^{2\pi} \sqrt{ a^{2}+b^{2} } \, d\phi = 2\pi\sqrt{ a^{2}+b^{2} }
\end{gather}$$

## 4

$$\begin{gather}
\alpha(t) = (a\cos t,a\sin t,bt)^{T} \\
\dot{\alpha}(t) = (-a\sin t,a\cos t,b)^{T} \\
|\dot{\alpha}(t)| = \sqrt{ a^{2} + b^{2} } \\
\tau(t) = \int_{0}^{t} \sqrt{ a^{2}+b^{2} } \, d\phi = t\sqrt{ a^{2}+b^{2} }\\
\tau^{-1}(t) = \frac{t}{\sqrt{ a^{2}+b^{2} }} \\
\alpha(\tau) = \alpha\left( \frac{t}{\sqrt{ a^{2}+b^{2} }} \right)
\end{gather}$$
