---
tags:
  - homework
  - 2nd-semester
  - 2024-09-27
---

## 190

$$\begin{gather}
\frac{3x^{2}+y^{2}}{y^{2}}dx - \frac{2x^{3}+5y}{y^{3}}dy = 0 \\
\left( \frac{3x^{2}+y^{2}}{y^{2}} \right)'_{y} = \frac{-6x^{2}}{y^{3}} \\
\left( -\frac{2x^{3}+5y}{y^{3}} \right)'_{x} = -\frac{6x^{2}}{y^{3}} \\
F(x,y) = \int \frac{3x^{2}+y^{2}}{y^{2}} \, dx = \frac{3}{y^{2}}\int x^{2} \, dx + x = \frac{x^{3}}{y^{2}} + x + \phi(y) \\
F'_{y} = -\frac{2x^{3}}{y^{3}} +\phi'(y) \\
-\frac{2x^{3}}{y^{3}} +\phi'(y) = -\frac{2x^{3}}{y^{3}} - \frac{5}{y^{2}} \\

\end{gather}$$

## 194

$$\begin{gather}
\left( \frac{x}{\sin y}+2 \right)dx + \frac{(x^{2}+1)\cos y}{\cos 2y - 1}dy = 0
\end{gather}$$