---
tags:
  - homework
  - 2nd-semester
  - 2024-11-04
---

## 1

$$\begin{gather}
\tilde{\omega}_{a} = a_{i}dx^{i}, \ \tilde{\omega}_{b} = \frac{1}{2}b_{ij}dx^{i}\wedge dx^{j}, \ \mathbb{R}^{3} \\
\tilde{\omega}_{a}^{1} \wedge \tilde{\omega}_{b}^{2} = a_{i}b^{i}dx^{1}\wedge dx^{2}\wedge dx^{3}
\end{gather}$$

## 2

$$\begin{gather}
*((dx^{1} - 5dx^{2}) \wedge (dx^{1} + dx^{2})), \ \mathbb{R}^{2}, \ \mathbb{R}^{3} \\
*((dx^{1} - 5dx^{2}) \wedge (dx^{1} + dx^{2})) = \\
= *(dx^{1}\wedge dx^{1} + dx^{1}\wedge dx^{2} -5 dx^{2}\wedge dx^{1} -5 dx^{2}\wedge dx^{2}) = \\
= 6*(dx^{1}\wedge dx^{2}) \\
\mathbb{R}^{2}: \ 6\epsilon^{12} = 6 \\
\mathbb{R}^{3}: \ 6\epsilon^{123}\vec{e_{3}} = 6\vec{e}_{3} \\
\end{gather}$$

## 3

$$\begin{gather}
*((3dx^{1}+ dx^{2}) \wedge (dx^{1} + dx^{2} + dx^{3}) \wedge (dx^{1} - 4dx^{2})), \ \mathbb{R}^{3}, \ \mathbb{R}^{3} \\
*((3dx^{1} + dx^{2}) \wedge (dx^{1} + dx^{2} + dx^{3}) \wedge (dx^{1} - 4dx^{2})) = \\
= *((2dx^{1} \wedge dx^{2} + 3dx^{1} \wedge dx^{3} + dx^{2} \wedge dx^{3}) \wedge (dx^{1} - 4dx^{2})) = \\
= *(dx^{1} \wedge dx^{2} \wedge dx^{3} - 12dx^{1} \wedge dx^{3} \wedge dx^{2}) = \\
= 13 *(dx^{1} \wedge dx^{2} \wedge dx^{3}) \\
\mathbb{R}^{3} : \ 13\epsilon^{123} = 13 \\
\mathbb{R}^{4}: \ 13\epsilon^{1234}\vec{e}_{4} = 13\vec{e}_{4}
\end{gather}$$

## 4

$$\begin{gather}
*\tilde{d} ((x^{1})^{2}dx^{2} \wedge dx^{3} + x^{1}x^{2} dx^{1} \wedge dx^{2} + (x^{2})^{2}x^{3} dx^{1} \wedge dx^{3}), \ \mathbb{R}^{3} \\
*\tilde{d} ((x^{1})^{2}dx^{2} \wedge dx^{3} + x^{1}x^{2} dx^{1} \wedge dx^{2} + (x^{2})^{2}x^{3} dx^{1} \wedge dx^{3}) = \\
*(2x^{1}dx^{1}\wedge dx^{2} \wedge dx^{3} + \underbrace{(x^{1}dx^{2} + x^{2}dx^{1})\wedge dx^{1}\wedge dx^{2}}_{0} + \\
+ ((x^{2})^{2}dx^{3} + 2x^{3}x^{2}dx^{2})\wedge dx^{1} \wedge dx^{3}) = \\
= *(2x^{1} dx^{1} \wedge dx^{2} \wedge dx^{3} + 2x^{2}x^{3} dx^{2} \wedge dx^{1} \wedge dx^{3}) = \\
(2x^{1} - 2x^{2}x^{3})*(dx^{1}\wedge dx^{2} \wedge dx^{3}) \\
\mathbb{R}^{3} : \ (2x^{1} - 2x^{2}x^{3})\epsilon^{123} = 2(x^{1} - x^{2}x^{3}) \\
\end{gather}$$

## 5

$$\begin{gather}
*\tilde{d}*((x^{1})^{2}\vec{e}_{1}+x^{2}\vec{e}_{2} + x^{1}x^{3} \vec{e}_{3}), \ \mathbb{R}^{3} \\
*\tilde{d}*((x^{1})^{2}\vec{e}_{1}+x^{2}\vec{e}_{2} + x^{1}x^{3} \vec{e}_{3}) = \\
= *\tilde{d}((x^{1})^{2}dx^{2} \wedge dx^{3} + x^{2}dx^{1} \wedge dx^{3} + x^{1}x^{3}dx^{1}\wedge dx^{2}) = \\
= *(2x^{1}dx^{1} \wedge dx^{2} \wedge dx^{3} + dx^{2} \wedge dx^{1} \wedge dx^{3} + (x^{1}dx^{3} + x^{3}dx^{1})dx^{1} \wedge dx^{2}) = \\
= (3x^{1} - 1)*(dx^{1} \wedge dx^{2} \wedge dx^{3}) \\
\mathbb{R}^{3}: \ (3x^{1} - 1)\epsilon^{123} = 
\end{gather}$$