---
tags:
  - homework
  - 2nd-semester
  - 2025-02-23
---

1) 3,7
2) 1,3,5
3) 1,3,4
4) 2
5) 2

### 1.3

$$\begin{gather}
\tan iz = \frac{\sin iz}{\cos iz} = -i\frac{e^{i^{2}z} - e^{-i^{2}z}}{e^{i^{2}z} + e^{-i^{2}z}} = -i \frac{e^{-z}-e^{z}}{e^{-z}+e^{z}} = i\frac{\frac{e^{z}-e^{-z}}{2}}{\frac{e^{z}+e^{-z}}{2}} = i \frac{\sinh z}{\cosh z} = i\tanh z
\end{gather}$$

### 2.3
 $$\begin{gather}
\cos z = \frac{e^{iz} + e^{-iz}}{2} = \frac{e^{i(x+yi)} + e^{-i(x+yi)}}{2} = \frac{e^{ix}e^{-y} + e^{-ix}e^{y}}{2} = \\ = \frac{1}{2} \left[ e^{-y}(\cos x + i \sin x) + e^{y}(\cos x - i\sin x) \right] = \\
= \frac{1}{2}(e^{y} + e^{-y})\cos x + \frac{i}{2} (e^{-y} - e^{y}) \sin x = \\ = \cosh y\cos x - i\sinh y\sin x
\end{gather}$$
### 2.7
$$\begin{gather}
\tanh z = \frac{\sinh z}{\cosh z} = \frac{e^{z} - e^{-z}}{e^{z} + e^{-z}} = \frac{e^{x}e^{iy} - e^{-x}e^{-iy}}{e^{x}e^{iy} + e^{-x}e^{-iy}} = \\
= \frac{e^{x}(\cos y + i \sin y) - e^{-x}(\cos y - i\sin y)}{e^{x}(\cos y + i \sin y) + e^{-x}(\cos y - i\sin y)} = \\
= \frac{(e^{x}-e^{-x})\cos y + i(e^{x} + e^{-x})\sin y}{(e^{x}+e^{-x})\cos y + i(e^{x}-e^{-x})\sin y} = \\
= \frac{\sinh x\cos y + i\cosh x \sin y}{\cosh x\cos y + i\sinh x \sin y} = \\
= ..?
\end{gather}$$

### 3.1

$$\begin{gather}
\cos(2+i) = \frac{e^{i(2+i)} + e^{-i(2+i)}}{2} = \\
= \frac{e^{2i-1} + e^{-2i+1}}{2} = \frac{e^{2i}e^{-1}+e^{-2i}e}{2} = \\
= \frac{1}{2}\left[ e^{-1}(\cos 2 + i\sin 2) + e(\cos 2 - i\sin 2) \right] = \\
= \frac{1}{2}\cos 2 (e^{-1}+e) + \frac{i}{2}\sin 2 (e^{-1}-e) = \\
= \cos 2 \cosh 1 - i\sin 2 \sinh 1
\end{gather}$$

### 3.3

$$\begin{gather}
\tan (2-i) = \frac{\sin 4 - i\sinh 2}{\cos 4 + \cosh 2}
\end{gather}$$

### 3.5

$$\begin{gather}
\frac{7}{\sqrt{ 2 }} -\cos \left( \frac{\pi}{4} +i\ln 7\right) = \\
= \dots \\
\cos\left( \frac{\pi}{4} + i \ln 7 \right) = \cos \frac{\pi}{4}\cos i\ln 7 - \sin \frac{\pi}{4} \sin i\ln 7 = \\
= \frac{\sqrt{ 2 }}{2}\cos i \ln 7 - \frac{\sqrt{ 2 }}{2} \sin i \ln 7 = \\
= \frac{\sqrt{ 2 }}{4} \left[ e^{i^{2}\ln 7} + e^{-i^{2}\ln 7} +i (e^{i^{2}\ln 7} - e^{-i^{2} \ln 7}) \right] = \\
= \frac{\sqrt{ 2 }}{4} \left[ \frac{1}{7} + 7 + i \left( \frac{1}{7} - 7 \right) \right] = \\
= \frac{\sqrt{ 2 }}{4} \left( \frac{50}{7} - i \frac{48}{7} \right)  \\
\dots = \frac{7}{\sqrt{ 2 }} - \left( \frac{25}{7\sqrt{ 2 }} - i \frac{24}{7\sqrt{ 2 }} \right) = \\
\dots = \frac{7}{\sqrt{ 2 }} - \frac{25}{7\sqrt{ 2 }} + i \frac{24}{7\sqrt{ 2 }} = \\
= \frac{12\sqrt{ 2 }(1+i)}{7}
\end{gather}$$

### 4.1


$$\begin{gather}
2^{i} = e^{i \mathrm{Ln} \ 2} = e^{i\ln 2} = \cos \ln 2 + i \sin \ln 2
\end{gather}$$

### 4.3

$$\begin{gather}
(3-4i)^{i+1} = e^{(i+1) \mathrm{Ln} \ (3-4i)} = \\
= e^{(i+1)(\ln 5 -i(\arctan 3/4 + 2\pi k))} = \\
= e^{i\ln 5 + (\arctan 3/4 + 2\pi k) + \ln 5 - i(\arctan 3/4 + 2\pi k)} = \\
= 5e^{\arctan 3/4 + 2\pi k}\left( \cos \left[ \ln 5-\arctan \frac{4}{3} + 2\pi k \right] + i \sin \left[ \ln 5-\arctan \frac{4}{3} + 2 \pi k \right] \right) = \\
= 5e^{\arctan 3/4}\left( \cos \left[ \ln 5-\arctan \frac{4}{3} \right] + i \sin \left[ \ln 5-\arctan \frac{4}{3} \right] \right) = \\
\end{gather}$$

### 4.4

$$\begin{gather}
i^{i} = e^{i\mathrm{Ln} \ i} = e^{i(\ln 1 + i(\pi/2 + 2\pi k))} = \\
= e^{i^{2}(\pi/2+2\pi k)} = e^{-\pi/2 + 2\pi k} = e^{-\pi/2}
\end{gather}$$

### 5.2

$$\begin{gather}
w = \mathrm{Arctan} \ z, \ z_{0} = \frac{i}{3} \\
z = \tan w \iff z = -i\cdot \frac{e^{iw} - e^{-iw}}{e^{iw} + e^{iw}} \\
z(e^{iw}+e^{-iw}) = -i(e^{iw} - e^{-iw}) \\
\begin{bmatrix}
t = e^{iw}
\end{bmatrix} \\
z(t+t^{-1}) = -i(t - t^{-1}) \\
zt^{2} + z = -i(t^{2} - 1) \\
(z+i)t^{2} = i-z \\
t^{2} = \frac{i-z}{i+z} \\
t = \pm\sqrt{ \frac{i-z}{i+z} }
\end{gather}$$

$$\begin{gather}
e^{iw} = \pm\sqrt{ \frac{i-z}{i+z} } \\
iw = \mathrm{Ln} \ \left(\pm\sqrt{ \frac{i-z}{i+z} }\right) \\
w = -i\mathrm{Ln} \ \left(\pm\sqrt{ \frac{i-z}{i+z} }\right) \\
\end{gather}$$

$$\begin{gather}
z_{0} = \frac{i}{3} \\
w_{1} = -\frac{i}{2}\mathrm{Ln} \frac{\frac{2i}{3}}{\frac{4i}{3}} = -\frac{i}{2} \mathrm{Ln} \ \frac{1}{2} = \frac{i}{2}\ln 2 \\
w_{2} = -i\mathrm{Ln} \ \left( -\sqrt{ \frac{2}{4} } \right) = \varnothing \\
\end{gather}$$

### 6.2

$$\begin{gather}
\sin z - \cos z = 3 \\
\frac{e^{iz}-e^{-iz}}{2i} - \frac{e^{iz} + e^{-iz}}{2} = 3 \\
e^{iz} - e^{-iz} - ie^{iz} - ie^{-iz} = 6i \\
\begin{bmatrix}
e^{iz} = t
\end{bmatrix} \\
t - t^{-1} -it - it^{-1} = 6i \\
t^{2} - 1 -it^{2} -i = 6it \\
(1-i)t^{2} -6it -1-i = 0 \\
\end{gather}$$

$$\begin{gather}
D = -32 + 4\cdot(1-i)(1+i) = -32 + 8 = -24 \implies \sqrt{ D } = 2\sqrt{ 6 }i \\
t_{1,2} = \frac{6i\pm 2\sqrt{ 6 }i}{2(1-i)} = \frac{3i \pm \sqrt{ 6 }i}{1-i} = \\
= \frac{(3i\pm i\sqrt{ 6 })(1+i)}{2} = \frac{(3i-3) \pm(i\sqrt{ 6 } - \sqrt{ 6 })}{2} = \\
e^{iz} = \begin{cases}
-(3+\sqrt{ 6 }) + (3+\sqrt{ 6 })i \\
\sqrt{ 6 }-3 + (3-\sqrt{ 6 })i \\
\end{cases} \\
|z|e^{iz/|z|} = \begin{cases}
-(3+\sqrt{ 6 }) + (3+\sqrt{ 6 })i \\
\sqrt{ 6 }-3 + (3-\sqrt{ 6 })i \\
\end{cases} \\

\end{gather}$$

### 6.2

$$\begin{gather}
\sin z - \cos z = 3 \\
\frac{\sqrt{ 2 }}{2}\sin z - \frac{\sqrt{ 2 }}{2}\cos z = \frac{3\sqrt{ 2 }}{2} \\
\sin\left( z - \frac{\pi}{4} \right) = \frac{3\sqrt{ 2 }}{2} \\
\frac{1}{2i}\left[ e^{iz-i\pi/4} - e^{-iz+i\pi/4} \right] = \frac{3\sqrt{ 2 }}{2} \\
-\frac{i}{2}\left[ e^{i(-\pi/4)}e^{iz} - e^{i(-z)}e^{i\pi/4} \right]  = \frac{3\sqrt{ 2 }}{2} \\
\end{gather}$$