---
tags:
  - homework
  - 2nd-semester
  - 2025-02-16
---

## I

### 3

$$\begin{gather}
\left( \frac{1+i\sqrt{ 3 }}{1-i} \right)^{20} = \left( \frac{(1+i\sqrt{ 3 })(1+i)}{2} \right)^{20} = \\
= \left( \frac{1-\sqrt{ 3 } + i(1 + \sqrt{ 3 })}{2} \right)^{20} = \\
= \left( \frac{1-\sqrt{ 3 }}{2} + i\frac{1 + \sqrt{ 3 }}{2} \right)^{20} = \\
\end{gather}$$

$$\begin{gather}
= \begin{bmatrix}
r = \frac{\sqrt{ 1-2\sqrt{ 3 }+3+1+2\sqrt{ 3 }+3 }}{2} = \sqrt{ 2 } \\
\phi = \pi+\arctan \frac{1+\sqrt{ 3 }}{1-\sqrt{ 3 }} \\
\arctan \frac{1+\sqrt{ 3 }}{1-\sqrt{ 3 }} = \alpha
\end{bmatrix} = \\
= \left[ \sqrt{ 2 }\left( \cos [\pi+\alpha] + i\sin [\pi +\alpha] \right)  \right]^{20} = \\
\end{gather}$$

$$\begin{gather}
= 1024(\cos \pi \cos\alpha - \sin \pi \sin\alpha + i[\sin \pi \cos\alpha + \cos \pi \sin\alpha])^{20} = \\
= 1024(\cos\alpha + i\sin\alpha)^{20} = \\
= -1024\left( \cos + i\cdot \frac{1+\sqrt{ 3 }}{\sqrt{ 1+ (1+\sqrt{ 3 }) }} \right) \\
= -1024(\cos 20\alpha + i \sin 20\alpha) = \\
\end{gather}$$

$$\begin{gather}
\dots = 512 - (512\sqrt{ 3 })i
\end{gather}$$

### 5

$$\begin{gather}
\sqrt[3]{ -i } = -\sqrt[3]{ i }= \begin{bmatrix}
r = 1 \\
\phi = \frac{\pi}{2} \\
\end{bmatrix} = \sqrt[3]{ \left( \cos \frac{\pi}{2} + i\sin \frac{\pi}{2} \right) } = \\
= \cos \left(\frac{\pi}{6} + \frac{2\pi k}{3}\right) + i\sin \left( \frac{\pi}{6} + \frac{2\pi k}{3} \right) , \ k = 0,1,2 \\
z_{1} = -\frac{\sqrt{ 3 }}{2} - \frac{i}{2} \\
z_{2} = \frac{\sqrt{ 3 }}{2} - \frac{i}{2} \\
z_{3} = i
\end{gather}$$

## II

### 4

$$\begin{gather}
\mathrm{Im} \ \frac{z+1}{z-i} = 0 \\
\frac{z+1}{z-i} = \frac{x+iy+1}{x+iy-i} = \frac{(x+1) + iy}{x+i(y-1)} = \\
= \frac{((x+1)+iy)(x-i(y-1))}{x^{2} + (y-1)^{2}} = \\
\end{gather}$$

$$\begin{gather}
= \frac{x^{2}+x+y^{2}-y + i(-xy+x-y+1 + xy)}{x^{2} + (y-1)^{2}} = \\
= \frac{x^{2} + y^{2} + x - y + i(x-y+1)}{x^{2}+(y-1)^{2}} \\
\mathrm{Im} \ \frac{z+1}{z-i} = \frac{x-y+1}{x^{2}+(y-1)^{2}} = 0 \\
\end{gather}$$

$$\begin{gather}
\begin{cases}
x^{2} + (y-1)^{2} \neq 0 \implies \begin{cases}
x\neq 0 \\
y\neq 1
\end{cases} \\
x-y+1 = 0 \implies y = x+1
\end{cases}
\end{gather}$$

![[2025-02-16 Домашнее задание - ТФКП 2025-02-16 11.56.10.excalidraw]]

### 5

$$\begin{gather}
|z-i| + |z+i| < 4 \\
\sqrt{ x^{2} + (y-1)^{2} } + \sqrt{ x^{2} + (y+1)^{2} } < 4 \\
x^{2} + (y-1)^{2} + x^{2} + (y+1)^{2} + 2\sqrt{ x^{2}+(y-1)^{2} }\sqrt{ x^{2} + (y+1)^{2} } < 16 \\
2x^{2} + 2y^{2} + 2 + 2\sqrt{ x^{4} + x^{2}(y-1)^{2} + x^{2}(y+1)^{2} + (y-1)^{2}(y+1)^{2} } < 16
\end{gather}$$

$$\begin{gather}
x^{2} + y^{2} + 1 + \sqrt{ x^{4} + 2x^{2}y^{2} + 2x^{2} + (y^{2}-1)^{2} } < 8 \\
x^{2} + y^{2} + 1 + \sqrt{ x^{4} + 2x^{2}y^{2} + 2x^{2} + y^{4} - 2y^{2} + 1 } < 8 \\
\end{gather}$$

$$\begin{gather}
x^{2} + y^{2} -7 < - \sqrt{ x^{4} + 2x^{2}(y^{2} + 1) + y^{4} - 2y^{2} + 1 } \\
(x^{2}+y^{2}-7)^{2} > x^{4} + 2x^{2}(y^{2} + 1) + y^{4} - 2y^{2} + 1 \\
x^{4} + 2x^{2}y^{2} - 14x^{2} + y^{4} - 14y^{2} + 49 > x^{4} + 2x^{2}y^{2} + 2x^{2} + y^{4} - 2y^{2} + 1
\end{gather}$$

$$\begin{gather}
-14x^{2} - 14y^{2} + 49 > 2x^{2} - 2y^{2} + 1 \\
16x^{2}+ 12y^{2} - 48 < 0
\end{gather}$$