### [[Предел функции в точке]]
## 1. Домножение на сопряженное
$$
\begin{gather}
\underset{ x \to 1 }{lim} \ \frac{\sqrt{ x } + \sqrt{ x-1 } - 1}{\sqrt{ x^{2}-1 }} = \left[ \frac{0}{0} \right] = \underset{ x \to 1 }{lim} \ \left( \frac{\sqrt{ x } - 1}{\sqrt{ x^{2}-1 }}  + \frac{\sqrt{ x-1 }}{\sqrt{ x^{2}-1 }}\right) = \\
= \underset{ x \to 1 }{lim} \ \left( \frac{x-1}{\sqrt{ x^{2}-1 }(\sqrt{ x }+1)}  + \frac{1}{\sqrt{ x+1 }}\right) = \underset{ x \to 1 }{lim} \ \left( \frac{\sqrt{ x-1 }}{\sqrt{ x+1 }(\sqrt{ x }+1)}  + \frac{1}{\sqrt{ x+1 }}\right) = \\
= \frac{0}{\sqrt{ 2 } \cdot 2} + \frac{1}{\sqrt{ 2 }} = \frac{\sqrt{ 2 }}{2}
\end{gather}
$$
$$
\begin{gather}
\underset{ x \to \infty }{lim} \ (\sqrt{ x+2 } - \sqrt{ x-1 }) = [\infty-\infty] = \underset{ x \to \infty }{lim} \ \frac{(\sqrt{ x+2 } - \sqrt{ x-1 })(\sqrt{ x+2 } + \sqrt{ x-1 })}{\sqrt{ x+2 } - \sqrt{ x-1 }} = \\
 = \underset{ x \to \infty }{lim} \ \frac{(x+2) - (x-1)}{\sqrt{ x+2 } - \sqrt{ x-1 }} = \underset{ x \to \infty }{lim} \ \frac{3}{\sqrt{ x+2 } - \sqrt{ x-1 }} = 0
\end{gather}
$$
## 2. Правило Лопиталя
$$
\begin{gather}
\underset{ x \to 2 }{lim} \ \frac{8 - 2x^{2}}{x^{2} + 4x - 12} = \left[ \frac{0}{0} \right] = \underset{ x \to 2 }{lim} \ \frac{(8 - 2x^{2})'}{(x^{2} + 4x - 12)'} = \underset{ x \to 2 }{lim} \ \frac{-4x}{2x + 4} = -\frac{8}{8} = -1
\end{gather}
$$
## 3. Ряд Тейлора (формулы Маклорена)
$$
\begin{gather}
\underset{ x \to 0 }{lim} \ \frac{e^{x} - e^{-x} - 2x}{x - \sin x} = \left[ \frac{0}{0} \right] = \\
= \underset{ x \to 0 }{lim} \ \frac{\left( 1+\frac{x}{1!}+\frac{x^{2}}{2!}+\dots \right) - \left( 1+\frac{-x}{1!}+\frac{x^{2}}{2!}+\dots \right) - 2x}{x - \left( x-\frac{x^{3}}{3!}+\frac{x^{5}}{5!}-\dots \right)} = \\
= \underset{ x \to 0 }{lim} \ \frac{\frac{2x^{3}}{3!} + \frac{2x^{5}}{5!} + o(x^{5})}{\frac{x^{3}}{3!} - \frac{x^{5}}{5!} + o(x^{5})} = \frac{\frac{2}{3!}}{\frac{1}{3!}} = 2
\end{gather}
$$
## 4. Второй замечательный предел
$$
\begin{gather}
\underset{ x \to \infty }{lim} \ \left( \frac{x-2}{x+1} \right)^{2x+3} = \left[ \frac{\infty}{\infty} \right]^{\infty} = \underset{ x \to \infty }{lim} \ \left( \frac{x+1-3}{x+1} \right)^{2x+3} = \underset{ x \to \infty }{lim} \ \left( 1+\frac{-3}{x+1} \right)^{2x+3} = \\
= e^{\underset{ x \to \infty }{lim} \ \frac{-3(2x+3)}{x+1}} = e^{-6}
\end{gather}
$$
## 5. Эквиватентности
$$
\begin{gather}
\underset{ x \to 0 }{lim} \ \frac{\ln^{3}(1+x)}{arcsin^{2}\left( \frac{x}{3} \right)\sin\left( \frac{x^{2}}{3} \right)} = \underset{ x \to 0 }{lim} \ \frac{x^{3}}{\left( \frac{x}{3} \right)^{2}\frac{x^{2}}{3}} = \underset{ x \to 0 }{lim} \ \frac{x^{3}}{\frac{x^{4}}{27}} = \infty
\end{gather}
$$
