## –û–ø—Ä–µ–¥–µ–ª–µ–Ω–∏–µ

–ü—É—Å—Ç—å –∑–∞–¥–∞–Ω—ã —á–∏—Å–ª–∞ $a, \epsilon \in \mathbb{R}, \epsilon > 0$. –ò–Ω—Ç–µ—Ä–≤–∞–ª $U_\epsilon(a) = (a - \epsilon, a + \epsilon)$ –Ω–∞–∑—ã–≤–∞–µ—Ç—Å—è **$\epsilon$-–æ–∫—Ä–µ—Å—Ç–Ω–æ—Å—Ç—å—é —á–∏—Å–ª–∞ $a$**.

–ü—É—Å—Ç—å –∑–∞–¥–∞–Ω—ã —á–∏—Å–ª–∞ $ùëé, \epsilon \in \mathbb{R}, \epsilon > 0$. –û–±—ä–µ–¥–∏–Ω–µ–Ω–∏–µ –∏–Ω—Ç–µ—Ä–≤–∞–ª–æ–≤ $\mathring{U}_\epsilon(a) = (a - \epsilon, a) \cup (a, a + \epsilon)$ –Ω–∞–∑—ã–≤–∞–µ—Ç—Å—è **–ø—Ä–æ–∫–æ–ª–æ—Ç–æ–π (–≤—ã–∫–æ–ª–æ—Ç–æ–π) $\epsilon$-–æ–∫—Ä–µ—Å—Ç–Ω–æ—Å—Ç—å—é —á–∏—Å–ª–∞ $ùëé$**.

–ü—É—Å—Ç—å –∑–∞–¥–∞–Ω—ã —á–∏—Å–ª–∞ $ùëé, \epsilon \in \mathbb{R}, \epsilon > 0$. –ò–Ω—Ç–µ—Ä–≤–∞–ª $\mathring{X}_\epsilon(a) = (a, a + \epsilon)$ –Ω–∞–∑—ã–≤–∞–µ—Ç—Å—è **–ø—Ä–æ–∫–æ–ª–æ—Ç–æ–π (–≤—ã–∫–æ–ª–æ—Ç–æ–π) $\epsilon$-–æ–∫—Ä–µ—Å—Ç–Ω–æ—Å—Ç—å—é —á–∏—Å–ª–∞ $a$**.