---
tags:
  - seminar
  - 2nd-semester
  - 2024-02-29
  - матан
---

## [[Теорема об итегрировании по частям|Метод интегрирования по частям]]

$$\int \underbrace{P_{n}(x)}_{u(x)} \ \underbrace{\left\{\begin{matrix}
e^{\alpha x} \\
\cos\alpha x \\
\sin\alpha x \\
a^{\alpha x}
\end{matrix} \right\} \, dx }_{dv(x)}$$

$$\int \underbrace{\left\{\begin{matrix}
\arctan\alpha x \\
\arcsin\alpha x \\
\ln\alpha x
\end{matrix}\right\}}_{u(x)} \ \underbrace{P_{n}(x) \, dx }_{dv(x)}$$

$$\int \underbrace{\sqrt{ a^{2}+x^{2} }}_{u(x)} \ \underbrace{dx}_{dv(x)}$$

$$\int \underbrace{e^{\alpha x}}_{u(x)} \ \underbrace{\left\{\begin{matrix}
\sin\beta x \\
\cos\beta x
\end{matrix}\right\} \, dx}_{dv(x)}$$

### Примеры

#### 2.5

$$\begin{gather}
\int (3x-4)e^{-5x} \, dx = \begin{bmatrix}
u = 3x-4 & du = 3dx \\
dv = e^{-5x}dx & v = -\frac{e^{-5x}}{5}
\end{bmatrix} = \\
= -\frac{e^{-5x}(3x-4)}{5} + \int \frac{3e^{-5x}}{5} \, dx  = \\
= -\frac{e^{-5x}(3x-4)}{5} -\frac{3}{25}e^{-5x} + C
\end{gather}$$

#### 2.9

$$\begin{gather}
\int (2x+7)\sin \frac{\pi x}{2} \, dx  = \begin{bmatrix}
u = 2x+7 & du = 2dx \\
dv = \sin \frac{\pi x}{2}dx & v = -\frac{2}{\pi}\cos \frac{\pi x}{2}
\end{bmatrix} = \\
= -\frac{2}{\pi}(2x+7)\cos \frac{\pi x}{2} + \frac{4}{\pi}\int \cos \frac{\pi x}{2} \, dx  = \\
= -\frac{2}{\pi}(2x+7)\cos \frac{\pi x}{2} + \frac{8}{\pi^{2}}\sin \frac{\pi x}{2} + C
\end{gather}$$

#### 2.13

$$\begin{gather}
\int x\arcsin x \, dx = \begin{bmatrix}
u = \arcsin x & du = \frac{1}{\sqrt{ 1-x^{2} }}dx \\
dv = xdx & v = \frac{x^{2}}{2}
\end{bmatrix} = \\
= \frac{x^{2}\arcsin x}{2} - \frac{1}{2}\int \frac{x^{2}}{\sqrt{ 1-x^{2} }} \, dx = \\
= \frac{x^{2}\arcsin x}{2} + \frac{1}{2}\int \frac{-x^{2} + 1 - 1}{\sqrt{ 1-x^{2} }} \, dx = \\
= \frac{x^{2}\arcsin x}{2} - \frac{1}{2}\int \frac{1}{\sqrt{ 1-x^{2} }} \, dx + \frac{1}{2}\underbrace{\int \sqrt{ 1-x^{2} } \, dx}_{I} = \\
= \frac{x^{2}\arcsin x}{2}-\frac{1}{2}\arcsin x + \frac{1}{4}(x\sqrt{ 1-x^{2} } + \arcsin x)
\end{gather}$$

#### 2.17

$$\begin{gather}
I = \int \sqrt{ 1-x^{2} } \, dx = \begin{bmatrix}
u = \sqrt{ 1-x^{2} } & du = -\frac{x}{\sqrt{ 1-x^{2} }}dx \\
dv = dx & v = x
\end{bmatrix} = \\
= x\sqrt{ 1-x^{2} } + \int \frac{x^{2}}{\sqrt{ 1-x^{2} }} \, dx = \\
= x\sqrt{ 1-x^{2} } - \underbrace{\int \frac{-x^{2}+1}{\sqrt{ 1-x^{2} }} \, dx}_{I} + \int \frac{1}{\sqrt{ 1-x^{2} }} \, dx = \\
= x\sqrt{ 1-x^{2} } + \arcsin x - I \implies \\
\implies I = x\sqrt{ 1-x^{2} } + \arcsin x - I \implies \\
\implies I = \frac{x\sqrt{ 1-x^{2} } + \arcsin x}{2}
\end{gather}$$

> [!note] Борис пытался заруинить ))))

## Вывод формулы 

$$\begin{gather}
\int  e^{\alpha x} \cdot \sin \beta x  \cdot  \, dx  = \begin{vmatrix}
u = e^{\alpha x} &  du = e^{\alpha x} \cdot \alpha  \cdot dx \\
dv = \sin \beta x  \cdot  dx & v = -\frac{1}{\beta}\cos \beta x 
\end{vmatrix} = \\ 
= e^{\alpha x} \cdot  -\frac{1}{\beta}\cos \beta x + \frac{\alpha}{ \beta}\int  \cos \beta x  \cdot  e^{\alpha x} \, dx  = \\ 
= \begin{bmatrix}
u=e^{\alpha x} & du-e^{\alpha x} \cdot \alpha  \cdot dx \\
dv = \cos \beta x dx & v = \frac{1}{\beta} \cdot  \sin \beta x 
\end{bmatrix} = \\ 
= e^{\alpha x} \cdot  -\frac{1}{\beta} \cdot \cos\beta x + \frac{\alpha}{\beta}\left( e^{\alpha x} \cdot \frac{1}{\beta} \cdot \sin\beta x \cdot \frac{\alpha}{\beta}\underbrace{ \int \sin\beta x \cdot e^{\alpha x} \, dx }_{ I }  \right) \\
\frac{\beta^{2}}{\beta^{2}}I+ \frac{\alpha^{2}}{\beta^{2}}I=e^{\alpha x}\left( -\frac{1}{\beta} \cdot \cos\beta x+ \frac{\alpha}{\beta^{2}} \cdot  \sin \beta x \right) \\
I\left( \frac{\alpha^{2}+\beta^{2}}{\beta^{2}}\right)=e^{\alpha x}\left( \frac{\alpha}{\beta^{2}}\sin\beta x - \frac{1}{\beta}\cos \beta x \right) 
\end{gather}$$

## Вывод рекурентной формулы

$$\begin{gather}
I_{n} = \int x^{n}e^{\alpha x} \, dx =\begin{bmatrix}
u = x^{n} & du = n \cdot x^{n-1}dx  \\
dv = e^{\alpha x}dx  & v= \frac{1}{\alpha} \cdot e^{\alpha x}
\end{bmatrix}  = \\
= x^{n} \cdot  \frac{e^{\alpha x}}{\alpha}- \int  \frac{e^{\alpha x}}{\alpha} \cdot n  \cdot  x^{n-1} \, dx - \underbrace{ \frac{n}{\alpha}\int  e^{\alpha x} \cdot x^{n-1}  }_{ I_{n-1} }\, dx  \\
I = xn  \cdot  \frac{e^{\alpha x}}{\alpha}- \frac{n}{\alpha} \cdot  I_{n-1}
\end{gather}$$
