---
tags:
  - типовой-расчет
  - 2nd-semester
  - 2025-04-03
---

## СГВМ ТР 2

### Ершов Алексей Геннадьевич КМБО-03-23

### Вариант 5

$$\begin{gather}
A = \begin{pmatrix}
1 & 5 \\
-2 & 3
\end{pmatrix}, \ \vec{x}_{0} = \begin{pmatrix}
-4 \\
-2
\end{pmatrix} \\
\end{gather}$$

### А)

$$\begin{gather}
\begin{pmatrix}
\dot{x} \\
\dot{y}
\end{pmatrix} = \begin{pmatrix}
1 & 5 \\
-2 & 3
\end{pmatrix}\begin{pmatrix}
x \\
y
\end{pmatrix} \\
\begin{cases}
\dot{x} = x+5y \\
\dot{y} = -2x+3y
\end{cases} \\
\end{gather}$$

$$\begin{gather}
\begin{cases}
2\dot{x} = 2x + 10y \\
2\dot{x} = 3\dot{y} - \ddot{y}
\end{cases} \\
3\dot{y} -\ddot{y} = 3y - \dot{y} + 10y \\
\ddot{y} - 4\dot{y} + 13y = 0 \\
\lambda^{2} -4\lambda +13 = 0 \\
\end{gather}$$

$$\begin{gather}
(\lambda-2)^{2} = -9 \\
\lambda_{1,2} = 2\pm 3i \\
y = 2e^{2t}(C_{1}\cos 3t + C_{2}\sin 3t) \\
\end{gather}$$

$$\begin{gather}
2x = 3y - \dot{y} \\
x = \frac{3}{2}y - \frac{\dot{y}}{2} \\
 x = 3e^{2t}(C_{1}\cos 3t + C_{2}\sin 3t) - e^{2t}(C_{1}(2\cos 3t -3\sin 3t) + C_{2}(2\sin 3t + 3\cos 3t)) \\
x = e^{2t}(C_{1}(\cos 3t + 3\sin 3t) + C_{2}(\sin 3t - 3\cos 3t))
\end{gather}$$

$$\begin{gather}
\begin{cases}
x = C_{1}e^{2t}(\cos 3t + 3\sin 3t) + C_{2}e^{2t}(\sin 3t - 3\cos 3t) \\
y = C_{1}2e^{2t}\cos 3t + C_{2}2e^{2t}\sin 3t \\
\end{cases} \\
\begin{cases}
x = e^{2t}((C_{1} -3C_{2})\cos 3t  + (3C_{1} + C_{2})\sin 3t) \\
y = e^{2t}(2C_{1}\cos 3t + 2C_{2}\sin 3t) \\
\end{cases}
\end{gather}$$

$$\begin{gather}
\begin{cases}
C_{1} - 3C_{2} = 1 \\
2C_{1} = 0
\end{cases} \ \begin{cases}
C_{1} - 3C_{2} = 0 \\
2C_{1} = 1
\end{cases} \\
\begin{cases}
C_{1} = 0 \\
C_{2} =  - \frac{1}{3}
\end{cases} \ \begin{cases}
C_{1} = \frac{1}{2} \\
C_{2} = \frac{1}{6}
\end{cases}
\end{gather}$$

$$\begin{gather}
e^{At} = e^{2t}\begin{pmatrix}
-\frac{1}{3}\sin 3t + \cos 3t & \frac{5}{3}\sin 3t \\
-\frac{2}{3}\sin 3t & \cos 3t + \frac{1}{3}\sin 3t
\end{pmatrix}
\end{gather}$$

### Б) 

$$\begin{gather}
e^{At} = \mathcal{L}^{-1}[(pE-A)^{-1}] \\
pE-A = \begin{pmatrix}
p-1 & -5 \\
2 & p-3
\end{pmatrix} \\
\det(pE-A) = p^{2}-4p + 13 = (p-2)^{2} + 9 \\

\end{gather}$$