---
tags:
  - типовой-расчет
  - 2nd-semester
  - 2025-04-03
---

## СГВМ ТР 1

### Ершов Алексей Геннадьевич КМБО-03-23

### Вариант 5

$$A = \begin{pmatrix}
2 & -1 & 5 \\
2 & -1 & 1 \\
-1 & 1 & -4
\end{pmatrix}$$

### A)

$$\begin{gather}
\begin{cases}
\dot{x} = 2x-y+5z \\
\dot{y} = 2x-y+z \\
\dot{z} = -x+y-4z
\end{cases}
\end{gather}$$

$$\begin{gather}
\dot{x} - \dot{y} = 4z \\
\ddot{z} = -\dot{x} +\dot{y} -4\dot{z} \\
\ddot{z} = -4z - 4\dot{z} \\
\ddot{z}+4\dot{z} + 4z = 0 \\
\end{gather}$$

$$\begin{gather}
\lambda^{2} +4\lambda + 4 = 0 \\
(\lambda + 2)^{2} = 0 \\
\lambda_{1,2}  = -2 \\
z = e^{-2t}(C_{1}t + C_{2}) \\
z = C_{1}e^{-2t}t + C_{2}e^{-2t}
\end{gather}$$

$$\begin{gather}
\dot{z} = -x+y-4z \implies y = \dot{z} + x + 4z \\
\dot{x} = 2x -\dot{z} - x - 4z + 5z \\
\dot{x} - x = -\dot{z} + z \\
\dot{x} - x = e^{-2t}(C_{1}t+C_{2}) +2e^{-2t}(C_{1}t+C_{2}) - e^{-2t}C_{1} \\
\dot{x} - x = e^{-2t}(3C_{1} t + (3C_{2} - C_{1}))  \\
\end{gather}$$

$$\begin{gather}
x_{оо} = C_{3}e^{t} \\
x_{чн} = e^{-2t}\cdot R_{m}(x) \\
x_{чн} = e^{-2t} (-C_{1}t -C_{2}) \\
x = -C_{1}e^{-2t}t - C_{2}e^{-2t} + C_{3}e^{t}
\end{gather}$$

$$\begin{gather}
\dot{y} + y = 2x + z \\
x = y-4z-\dot{z} \\
\dot{y} -y = -7z-2\dot{z} \\
\dot{y} - y = -7C_{1}e^{-2t}t -7C_{2}e^{-2t} -2(-2C_{1}e^{-2t}t - 2C_{2}e^{-2t} + C_{1}e^{-2t}) \\
\dot{y}-y = 
\end{gather}$$

$$\begin{gather}
\dot{x} - \dot{y} = 4z \\
\dot{y} = \dot{x} - 4z \\
\dot{y} = 2C_{1}e^{-2t}t - C_{1}e^{-2t} +2C_{2}e^{-2t} + C_{3}e^{t} - 4C_{1}e^{-2t}t - 4C_{2}e^{-2t}) \\
\dot{y} = C_{1}e^{-2t}(-2t -1) -2 C_{2}e^{-2t} + C_{3}e^{t} \\
y = C_{1}e^{-2t}(t+1)  + C_{2}e^{-2t} + C_{3}e^{-2t}
\end{gather}$$

$$\begin{gather}
\text{Ответ}: \begin{cases}
x = -C_{1}e^{-2t}t - C_{2}e^{-2t} + C_{3}e^{t} \\
y = C_{1}e^{-2t}(t+1)  + C_{2}e^{-2t} + C_{3}e^{-2t} \\
z = C_{1}e^{-2t}t + C_{2}e^{-2t}
\end{cases}
\end{gather}$$

### Б)

$$\begin{gather}
\begin{vmatrix}
2-\lambda & -1 & 5 \\
2 & -1-\lambda & 1 \\
-1 & 1 & -4-\lambda
\end{vmatrix} = 0 \\
\begin{vmatrix}
2 & 1 \\
-1 & -4-\lambda
\end{vmatrix} - (1+\lambda)\begin{vmatrix}
2-\lambda & 5 \\
-1 & -4-\lambda
\end{vmatrix} - \begin{vmatrix}
2-\lambda & 5 \\
2 & 1
\end{vmatrix} = 0 \\
-8-2\lambda+1-(1+\lambda)(-3-2\lambda+\lambda^{2}) - 2+\lambda+10 = 0 \\
\lambda^{3} +3\lambda^{2} -4 = 0 \\
(\lambda+2)^{2}(\lambda-1) = 0 \\
\lambda_{1,2} = -2, \    \lambda_{3} = 1
\end{gather}$$

$$\begin{gather}
A_{\lambda,\lambda=1}: \begin{pmatrix}
1 & -1 & 5 \\
2 & -2 & 1 \\
-1 & 1 & -5
\end{pmatrix}\underbrace{\begin{pmatrix}
1 \\
1 \\
0
\end{pmatrix}}_{\vec{x}_{1}} = \vec{0} \\
\end{gather}$$

$$\begin{gather}
A_{\lambda,\lambda=-2}: \begin{pmatrix}
4 & -1 & 5 \\
2 & 1 & 1 \\
-1 & 1 & -2
\end{pmatrix}
\end{gather}$$