---
tags:
  - типовой-расчет
  - 2nd-semester
  - 2024-12-05
---

## ТР 6 СГВМ

### Ершов Алексей Геннадьевич КМБО-03-23

### Вариант 5

![[ТР 6 СГВМ 2024-12-05 14.04.49.excalidraw|300]]

$$F(t) = \frac{1}{1-e^{-pT}} \int_{0}^{T} f(t)e^{-pT} \, dt $$

$$\begin{gather}
f(t) = -\frac{3}{4} \cdot t(t-4) \\
f_{1}(t) = -\frac{3}{4} t(t-4)\theta(t) + \frac{3}{4}t(t-4)\theta(t-4) = \\
-\frac{3}{4}t^{2}\theta(t) + 3t\theta(t) + \frac{3}{4}(t-4 + 4)(t-4)\theta(t-4) = \\
= -\frac{3}{4}t^{2}\theta(t) + 3t\theta(t) + \frac{3}{4}(t-4)^{2}\theta(t-4) + 3(t-4)\theta(t-4)
\end{gather}$$

$$\begin{gather}
f(t) \fallingdotseq F(p) \\
f(t-\tau) \fallingdotseq e^{-p\tau}F(p) \\
t^{n}\theta(t) \fallingdotseq \frac{n!}{p^{n+1}} \\
\end{gather}$$

$$\begin{gather}
F_{1}(p) = -\frac{3}{4} \cdot \frac{2}{p^{3}} + 3\cdot \frac{1}{p^{2}} + \frac{3}{4}\cdot \frac{2e^{-4p}}{p^{3}} + 3\cdot \frac{e^{-4p}}{p^{2}} = \\
= -\frac{3}{2p^{3}} + \frac{3}{4p^{2}} + \frac{3e^{-4p}}{p^{2}} + \frac{3e^{-4p}}{2p^{3}} = \\
= -\frac{3}{2p^{3}}\cdot (1-e^{-4p}) + \frac{3}{p^{2}} \left( \frac{1}{4} + e^{-4p} \right) 
\end{gather}$$

$$\begin{gather}
F(p) = \frac{1}{1-e^{-4p}}\cdot F_{1}(p) = 
\end{gather}$$