---
tags:
  - типовой-расчет
  - 2nd-semester
  - 2024-12-05
---

## ТР 7 СГВМ

### Ершов Алексей Геннадьевич КМБО-03-23

### Вариант 5

$$\begin{gather}
y''-6 y'+10y = e^{-x}, \ y(0) = -1, \ y'(0) = 1 \\
\end{gather}$$

$$\begin{gather}
f(t) \fallingdotseq F(p) \\
f^{(n)} \fallingdotseq p^{n}F - p^{n-1}f(0) - p^{n-2}f'(0) - \dots - f^{(n-1)}(0) \\
\end{gather}$$

$$\begin{gather}
y(x) \fallingdotseq Y(p) \\
y'(x) \fallingdotseq pY(p) + 1 \\
y''(x) \fallingdotseq p^{2}Y(p) + p - 1
\end{gather}$$

$$\begin{gather}
e^{\alpha t}\theta(t) \fallingdotseq \frac{1}{p-\alpha} \\
e^{-x} \fallingdotseq \frac{1}{p+1}
\end{gather}$$

$$\begin{gather}
p^{2}Y + p - 1 -6pY - 6 + 10Y = \frac{1}{p+1} \\
(p^{2}-6p + 10)Y = \frac{1}{p+1} - p + 7 \\
Y = \frac{1}{(p+1)(p-3+i)(p-3-i)} + \frac{7-p}{(p-3+i)(p-3-i)} \\
\end{gather}$$

$$\begin{gather}
Y = \frac{1}{12(p+1)} - \frac{1}{8(p-1)} + \frac{1}{24(p-5)} - \frac{3}{2(p-1)} + \frac{1}{2(p-5)} = \\
= \frac{1}{12(p+1)} - \frac{13}{8(p-1)} + \frac{13}{24(p-5)} \\
y(x) = \frac{1}{12}e^{-x} - \frac{13}{8}e^{x} + \frac{13}{24}e^{5x}
\end{gather}$$
