---
tags:
  - типовой-расчет
  - 2nd-semester
  - 2024-12-05
---

## ТР 7 СГВМ

### Ершов Алексей Геннадьевич КМБО-03-23

### Вариант 5

$$\begin{gather}
y''-6 y'+10y = e^{-x}, \ y(0) = -1, \ y'(0) = 1 \\
\end{gather}$$

$$\begin{gather}
f(t) \fallingdotseq F(p) \\
f^{(n)} \fallingdotseq p^{n}F - p^{n-1}f(0) - p^{n-2}f'(0) - \dots - f^{(n-1)}(0) \\
\end{gather}$$

$$\begin{gather}
y(x) \fallingdotseq Y(p) \\
y'(x) \fallingdotseq pY(p) + 1 \\
y''(x) \fallingdotseq p^{2}Y(p) + p - 1
\end{gather}$$

$$\begin{gather}
e^{\alpha t}\theta(t) \fallingdotseq \frac{1}{p-\alpha} \\
e^{-x} \fallingdotseq \frac{1}{p+1}
\end{gather}$$

$$\begin{gather}
p^{2}Y + p - 1 -6pY - 6 + 10Y = \frac{1}{p+1} \\
(p^{2}-6p + 10)Y = \frac{1}{p+1} - p + 7 \\
Y = \frac{1}{(p+1)(p^{2}-6p + 10)} + \frac{7-p}{p^{2}-6p + 10} = \\
= \frac{1}{17(p+1)} + \frac{7-p}{17(p^{2}-6p+10)} + \frac{7-p}{p^{2}-6p + 10} = \\
\end{gather}$$

$$\begin{gather}
= \frac{1}{17}\left( \frac{1}{p+1} + \frac{18(7-p)}{(p-3)^{2}+1} \right) = \\
= \frac{1}{17}\left( \frac{1}{p+1} - 18\cdot \frac{(p-3) - 4}{(p-3)^{2}+1} \right) = \\
= \frac{1}{17}\left( \frac{1}{p+1} - 18\cdot \frac{p-3}{(p-3)^{2}+1} + 72\cdot \frac{1}{(p-3)^{2} + 1} \right)
\end{gather}$$

$$\begin{gather}
\begin{bmatrix}
\frac{p-\alpha}{(p-\alpha)^{2} + \beta^{2}} \fallingdotseq e^{\alpha t}\cos\beta t \\
\frac{1}{(p-\alpha)^{2} + \beta^{2}} \fallingdotseq \frac{1}{\beta}e^{\alpha t}\sin\beta t \\
\end{bmatrix} \\
y(x) = \frac{1}{17} \left( e^{-x} - 18 e^{3x}\cos x + 72 e^{3x}\sin x \right) 
\end{gather}$$
