---
tags:
  - типовой-расчет
  - 2nd-semester
  - 2024-12-09
---

## ТР 5 СГВМ

### Ершов Алексей Геннадьевич КМБО-03-23

### Вариант 5

$$y'' + 3y' = xe^{x}, \ y(0) = 0, \ y'(0) = 0$$

### а)

$$\begin{gather}
z'' + 3z' = 1, \ z(0) = 0, \ z'(0) = 0 \\
y(x) = xe^{x}*z'(x) \\
z(x) \fallingdotseq
\end{gather}$$

### б)

$$\begin{gather}
y'' + 3y' = xe^{x} \\
\lambda^{2} + 3\lambda = 0 \\
\lambda(\lambda+3) = 0 \\
\lambda_{1} = 0, \ \lambda_{2} = -3 \\
\end{gather}$$

$$\begin{gather}
\phi_{1}(x) = 1, \ \phi_{2}(x) = e^{-3x} \\
y_{оо} = c_{1} + c_{2}e^{-3x}, \ c_{1}, c_{2} = \mathrm{const} \\
y_{он} = c_{1}(x) + c_{2}(x)e^{-3x}
\end{gather}$$

$$\begin{gather}
\begin{cases}
c_{1}'(x) + c_{2}'(x)e^{-3x} = 0 \\
-3c_{2}'(x)e^{-3x} = xe^{x}
\end{cases} \\
\begin{cases}
c_{1}'(x) = \frac{1}{3}xe^{x} \\
c_{2}'(x) = -\frac{1}{3}xe^{4x}
\end{cases} \\
\end{gather}$$

$$\begin{gather}
c_{1}(x) = \frac{1}{3}\int xe^{x} \, dx = \frac{1}{3}e^{x}(x-1) + \tilde c_{1} \\
c_{2}(x)a = -\frac{1}{3}\int xe^{4x} \, dx = -\frac{1}{48}e^{4x}(4x-1) + \tilde c_{2}
\end{gather}$$

$$\begin{gather}
y_{он} = \frac{1}{3}e^{x}(x-1) + \tilde{c}_{1} - \frac{1}{48}e^{4x}(4x-1) \cdot e^{-3x} + e^{-3x}\tilde{c}_{2} = \\
= \frac{1}{3}xe^{x} - \frac{1}{3}e^{x} - \frac{1}{12}xe^{x} + \frac{1}{48}e^{x} + \tilde{c}_{1} + \tilde{c}_{2}e^{-3x} = \\
= \frac{1}{4}xe^{x} - \frac{5}{16}e^{x} + \tilde{c}_{1} + \tilde{c}_{2}e^{-3x}
\end{gather}$$

$$\begin{gather}
\begin{cases}
y(0) = 0 \\
y'(0) = 0 
\end{cases} \implies \begin{cases}
-\frac{5}{16} + \tilde{c}_{1} + \tilde{c}_{2} = 0 \\
-3\tilde{c}_{1} - \frac{1}{16} = 0
\end{cases} \implies \begin{cases}
\tilde{c}_{1} = -\frac{1}{48} \\
\tilde{c}_{2} = \frac{1}{3}
\end{cases}
\end{gather}$$

$$\begin{gather}
y_{ч} = \frac{1}{4}xe^{x} - \frac{5}{16}e^{x} + \frac{1}{3}e^{-3x} - \frac{1}{48}
\end{gather}$$
