---
tags:
  - seminar
  - 2nd-semester
  - 2025-02-26
---

### 1. Можно ли вычичлить по правилу Лейбница $F'(y)$, если $F(y) = \int_{0}^{1} f(x,y) \, dx$,

$$\begin{gather}
f(x,y) = \begin{cases}
\arctan \frac{y}{x} - \frac{xy}{x^{2}+y^{2}}, \ 0< x \leq 1, \ 0 \leq y \leq 1 \\
\frac{\pi}{2}, \ x = 0, \ 0\leq y\leq 1
\end{cases}
\end{gather}$$

$$\begin{gather}
F(y) = \int_{0}^{1} \arctan \frac{y}{x} - \frac{xy}{x^{2}+y^{2}} \, dx = \\
= \int_{0}^{1} \arctan \frac{y}{x} \, dx -\int_{0}^{1} \frac{xy}{x^{2}+y^{2}} \, dx = \\
= \left.x\arctan \frac{y}{x}\right|_{0}^{1} + \int_{0}^{1} \frac{xy}{x^{2}+y^{2}} \, dx - \int_{0}^{1} \frac{xy}{x^{2}+y^{2}} \, dx = \\
= \arctan y \implies F'(y) = \frac{1}{1+y^{2}}, \ F'(0) = 1
\end{gather}$$

$$\begin{gather}
F'(y_{0}) = \int_{0}^{1} \frac{\partial f(x,y)}{\partial y} \, dx \\
\frac{\partial f(x,y)}{\partial y} = \lim_{ y \to 0 } \frac{f(x,y) - f(x,0)}{y} = \left[ \frac{0}{0} \right] = \\
= \dots = 0 \\
1 \neq 0 \implies \text{нельзя}
\end{gather}$$

### 3. 

$$\begin{gather}
I(a) = \int_{0}^{\pi/2} \ln (a^{2}\sin ^{2}x + \cos ^{2}x) \, dx , \ a > 0 \\
f(x,a) = \ln (a^{2}\sin ^{2}x + \cos ^{2}x) \\
\frac{\partial f}{\partial a} = \frac{2a\sin ^{2}x}{a^{2}\sin ^{2}x+\cos ^{2}x} \\
f(x,a) \in C(G), \ G = \left\{  (x;a): \ 0 \leq x \leq \frac{\pi}{2}, \ a_{1} \leq a \leq a_{2} \right\} \\
\end{gather}$$

$$\begin{gather}
I'(a) = \int_{0}^{\pi/2} \frac{\partial f}{\partial a} \, dx = \\
= \int_{0}^{\pi/2} \frac{2a\sin ^{2}x}{a^{2}\sin ^{2}x + \cos ^{2}x} \, dx = \int_{0}^{\pi/2} \frac{2a\tan^{2}x}{a^{2}\tan ^{2} x + 1} \, dx = \begin{bmatrix}
u = \tan x \\
x = \arctan u \\
dx = \frac{du}{1+u^{2}}
0 \mapsto 0 \\
\frac{\pi}{2} \mapsto +\infty
\end{bmatrix} = \\
= \int_{0}^{+\infty} \frac{2au^{2}}{a^{2}u^{2} + 1} \cdot \frac{du}{1+u^{2}} = \\
= 2a\int_{0}^{+\infty} \frac{u^{2}du}{(a^{2}u^{2}+1)(u^{2}+1)}= \\
\end{gather}$$

$$\begin{gather}
= 2a\int_{0}^{+\infty} \left[ \frac{A}{a^{2}u^{2}+1} + \frac{B}{u^{2}+1} \right] \, du = \\
= \frac{2a}{a^{2}-1}\int_{0}^{+\infty} \left[ \frac{1}{u^{2}+1} - \frac{1}{a^{2}u^{2}+1} \right]  \, du = \\
= \frac{2a}{a^{2}-1}\left.\left[ \arctan u - \frac{1}{a}\arctan (au) \right]\right|_{0}^{+\infty} = \frac{2a}{a^{2}-1} \left( \frac{\pi}{2} - \frac{1}{a} \cdot \frac{\pi}{2} \right) = \\
= \frac{\pi}{a+1}
\end{gather}$$

$$\begin{gather}
I'(a) = \frac{\pi}{a+1} \implies I(a) = \pi \ln (a+1) + C \\
a = 1: \ I(a) = \int_{0}^{\pi/2} \ln 1 \, dx = 0 \\
0 = \pi \ln 2 + C \\
C = -\pi \ln 2 \\
I(a) = \pi \ln \frac{a+1}{2}
\end{gather}$$

### And another one

$$\begin{gather}
I(a) = \int_{0}^{a} \frac{\ln (1+ax)}{1+x^{2}} \, dx , \ a>0 \\
I'(a) = \frac{\ln(1+a^{2})}{1+a^{2}} = \int_{0}^{a} \frac{x}{(1+ax)(1+x^{2})} \, dx  = \dots \\
\end{gather}$$

$$\begin{gather}
\mathbf{I} = \frac{1}{1+a^{2}}\int_{0}^{a} \left[ -\frac{a}{1+ax} + \frac{x+a}{1+x^{2}} \right]  \, dx = \\
= \frac{1}{1+a^{2}} \left.\left[ -\ln (ax+1) + \frac{1}{2} \ln(x^{2}+1) + a \arctan x\right]\right|_{0}^{a} = \\
= \frac{1}{1+a^{2}}\left[ -\ln(a^{2}+1) + \frac{1}{2}\ln (a^{2}+1) + a\arctan a \right]
\end{gather}$$

$$\begin{gather}
I'(a) = \frac{1}{2} \cdot \frac{\ln(1+a^{2})}{1+a^{2}} + \frac{a\arctan a}{1+a^{2}} = \\
= \frac{1}{2} \ln (1+a^{2}) (\arctan a)' + \arctan a \cdot \left( \frac{1}{2}\ln(1+a^{2}) \right)' = \\
\left( \frac{1}{2}\ln(1+a^{2})\arctan a \right)' \implies \\
I(a) = \frac{1}{2}\ln(1+a^{2})\arctan a + C
\end{gather}$$

### And another one

$$\begin{gather}
\int_{0}^{1} \sin\left( \ln \frac{1}{x} \right)\cdot \frac{x^{b}-x^{a}}{\ln x} \, dx = \\
= \int_{0}^{1} \sin\left( \ln \frac{1}{x} \right) \left(\int_{a}^{b} x^{y} \, dy\right) \, dx = \\
= \int_{0}^{1}\, dx\int_{a}^{b} x^{y} \sin \left( \ln \frac{1}{x} \right) \, dy = \\
= \int_{a}^{b}\, dy\int_{0}^{1} x^{y} \sin \left( \ln \frac{1}{x} \right) \, dx = \\
\end{gather}$$

$$\begin{gather}
I(y) = \begin{bmatrix}
u = \sin\left( \ln \frac{1}{x} \right) \\
dv = x^{y}dx \\
du = \cos\left( \ln \frac{1}{x} \right)\cdot \left( -\frac{1}{x} \right)dx \\
v = \frac{x^{y+1}}{y+1}
\end{bmatrix} = \\
= \left. \frac{x^{y+1}}{y+1}\sin\left( \ln \frac{1}{x} \right)\right|_{0}^{1} + \int_{0}^{1} \frac{x^{y}}{y+1}\cos\left( \ln \frac{1}{x} \right) \, dx = \\
= \begin{bmatrix}
u = \cos\left( \ln \frac{1}{x} \right) \\
dv = \frac{x^{y}}{y+1}dx \\
du = \sin\left( \ln \frac{1}{x} \right) \frac{1}{x}dx \\
v = \frac{x^{y+1}}{(y+1)^{2}}
\end{bmatrix} = \\
\end{gather}$$

$$\begin{gather}
= \left.\frac{x^{y+1}}{(y+1)^{2}} \cos \left( \ln \frac{1}{x} \right) \right|_{0}^{1} - \int_{0}^{1} \frac{x^{y}}{(y+1)^{2}} \sin \left( \ln \frac{1}{x} \right) \, dx = \\
= \frac{1}{(y+1)^{2}} - \frac{1}{(y+1)^{2}}I(y)
\end{gather}$$

$$\begin{gather}
I(y) = \frac{1}{(y+1)^{2}} - \frac{1}{(y+1)^{2}}I(y) \\
I(y) = \frac{1}{1+(y+1)^{2}}
\end{gather}$$

$$\begin{gather}
\dots = \int_{a}^{b} \frac{d(y+1)}{1+(y+1)^{2}} = \left.\arctan (y+1) \right|_{a}^{b} = \arctan(b+1) - \arctan(a+1)
\end{gather}$$