---
tags:
  - seminar
  - 2nd-semester
  - 2025-04-29
---

## Вычет в конечной точке

$$\begin{gather}
\underset{z=z_{0}}{\mathrm{res}} \ f(z) = c_{-1}
\end{gather}$$

$$\begin{gather}
z_{0} - \mathrm{П1}: \ 
\end{gather}$$

### 2

$$\begin{gather}
f(z) = \frac{1}{z(1-e^{2z})} \\
z_{0} = 0 - \Pi 2 \\
z_{k} = \pi ki - \Pi 1
\end{gather}$$

### 4

$$\begin{gather}
f(z) = \frac{e^{z}}{z^{2}(z^{2} + 9)} \\
z_{1} = 0 - \text{П2} \\
z_{2}  = \pm 3i - \text{П1} \\
\mathrm{res}_{z=z_{0}} f(z) = \frac{1}{(m-1)!} \lim_{ z \to z_{0} } [(z-z_{0})^{m}f(z)]^{m-1} \\
\end{gather}$$
	
### 12

$$\begin{gather}
f(z) = e^{z+1/z}; \ \underset{z=0}{\mathrm{res}} \ f(z) - ? \\
f(z) = e^{z}e^{1/z} = \left( 1 + z + \frac{z^{2}}{2} + \frac{z^{3}}{6} + \frac{z^{4}}{24} + \dots \right) \cdot \\
\left( 1 + \frac{1}{z}  + \frac{1}{2z^{2}} + \frac{1}{6z^{3}} + \frac{1}{24z^{4}} + \dots \right) \\
c_{-1} = 1 + \frac{1}{2} + \frac{1}{2!3!} + \frac{1}{3!4!} + \frac{1}{4!5!} = \sum_{n=0}^{\infty} \frac{1}{n!(n+1)!} \\
\underset{z=0}{\mathrm{res}} \ f(z) = \sum_{n=0}^{\infty} \frac{1}{n!(n+1)!}
\end{gather}$$