---
tags:
  - seminar
  - 2nd-semester
  - 2025-04-02
---

### 7

$$\begin{gather}
\int_{0}^{+\infty} \frac{\sin^{3}x \cos\alpha x}{x^{3}} \, dx , \ \alpha > 3 \\
I(\beta) = \int_{0}^{+\infty} \frac{\sin ^{3} \beta x\cos\alpha x}{x^{3}} \, dx, \\
\sin ^{3}\beta x\cos\alpha x = \frac{1}{4}\left[ \sin\beta x\cos\alpha x - \sin_{3}\beta x\cos\alpha x \right] = \\
= \frac{1}{8} \left[ 3\sin([\beta-\alpha ]x) + 3\sin[(\beta+\alpha)x] - \sin[(3\beta-\alpha) x] - \sin[(3\beta+\alpha) x] \right] \\
\end{gather}$$

$$\begin{gather}
I(\beta) = \frac{1}{8}\int_{0}^{+\infty} \frac{\dots}{x^{3}} \, dx \\
I'(\beta) = \frac{1}{8}\int_{0}^{+\infty} \frac{\dots}{x^{2}} \, dx  \\
I''(\beta) = \frac{1}{8} \int_{0}^{+\infty} \frac{-3\sin[(\beta-\alpha)x] - 3\sin[(\beta+\alpha)x] + 9\sin[(3\beta-\alpha)x] + 9\sin[(3\beta+\alpha)x]}{x} \, dx = \\
= \frac{1}{8} \left[ \frac{3\pi}{2} - \frac{3\pi}{2} - \frac{9\pi}{2} + \frac{9\pi}{2} \right] = 0
\end{gather}$$

$$\begin{gather}
I'(\beta) = C_{1} \\
I'(0) = \frac{1}{8} \cdot 0 \implies C_{1} = 0 \\
I(\beta) = C_{2}, \ I(0) = 0 \implies C_{2} = 0 \implies \\
\mathrm{Ans}: 0
\end{gather}$$

### 13

$$\begin{gather}
\int_{-\infty}^{+\infty} \sin ^{2}x\cos 2\alpha x \, dx = \frac{1}{2}\left[\int_{-\infty}^{+\infty} \sin(x^{2}+2\alpha x) \, dx + \int_{-\infty}^{+\infty} \sin(x^{2} - 2\alpha x) \, dx  \right]= \\
= \dots = d
\end{gather}$$

## Интеграл Фурей

> [!definition] Формула Фурье
> $$\begin{gather}
f(x) = \frac{1}{\pi} \int_{0}^{+\infty} \, dz \int_{-\infty}^{+\infty} f(u) \cos \left[ z(x-u) \right]  \, du \ (1)
\end{gather}$$

Если $f(x)$ - четная, то

$$f(x) = \frac{2}{\pi}\int dz \int f(u) \cos zx\cos zu \, du \ (2)$$

Если $f(x)$ - нечетная, то

$$\begin{gather}
f(x) = \frac{2}{\pi} \int_{0}^{+\infty} dz \int_{0}^{+\infty} \sin xz\sin zu \, du
\end{gather}$$

### 3

$$\begin{gather}
f(x) = \mathrm{sgn}(x-a) - \mathrm{sgn}(x-b), \ b > a \\
f(x) = \begin{cases}
2, \ x \in [a;b] \\
0, \ x \in \mathbb{R} \setminus (a; b)
\end{cases} \\
f(x) = \frac{2}{\pi} \int_{0}^{+\infty} dz \int_{a}^{b}\cos[z(x-u)] \, du = \\
= -\frac{2}{\pi}\int_{0}^{+\infty} \left.\frac{\sin[z(x-u)]}{z}dz \right|_{a}^{b} = \\
= \frac{2}{\pi} \frac{\sin[z(x-a)] - \sin[z(x-b)]}{z} \, dz
\end{gather}$$

