---
tags:
  - seminar
  - 2nd-semester
  - 2025-05-21
---

## Многочлены Чебышева

$$\begin{gather}
T_{n}(x) = \cos (n\arccos x), \ n = 0, 1, 2, \dots \\
1. \ T_{n+1}(x) -2xT_{n}(x) + T_{n-1}(x) = 0, \ n = 1,2,\dots \\
2. \ T_{n}(x) - \text{решение д/у}: \\
(1-x)^{2}y''(x) - xy'(x) + n^{2}y(x) = 0
\end{gather}$$

$$\begin{gather}
3. \ \int_{-1}^{1} T_{n}(x)T_{m}(x) \, \frac{dx}{\sqrt{ 1-x^{2} }}  = \begin{cases}
0, \ m \neq n \\
\frac{\pi}{2}, m = n \neq 0 \\
\pi, m = n = 0
\end{cases} \\
\end{gather}$$

$$\begin{gather}
4. \ \psi(x,t) \frac{1-tx}{1-2tx + t^{2}}, \ x \in [-1;1], \ t \in (-1;1) \\
\end{gather}$$

### Выписать в явном виде $T_{0}(x), \ T_{1}(x), \dots, T_{6}(X)$

$$\begin{gather}
T_{0}(x) = 1 \\
T_{1}(x) = x \\
T_{2}(x) = 2xT_{1}(x) - T_{0}(x) = 2x^{2} - 1 \\
\end{gather}$$

$$\begin{gather}
T_{3}(x) = 2xT_{2}(x) - T_{1}(x) = 4x^{3} - 3x \\
T_{4}(x) = 2xT_{3}(x) - T_{2}(x) = 8x^{4} - 8x^{2} + 1 \\
T_{5}(x) = 2xT_{4}(x) - T_{3}(x) = 16x^{5} - 20x^{3} + 5x
\end{gather}$$

$$\begin{gather}
T_{6}(x) = 32x^{6} - 48x^{4} + 18x^{2} - 1
\end{gather}$$

### 4. Доказать, что $T_{n}(T_{m}(x)) = T_{nm}(x)$

$$\begin{gather}
T_{n}(T_{m}(x)) = \cos(n\arccos(\cos(m\arccos(x)))) = \\
= \cos(n(\pm m\arccos x + 2\pi k)) = \cos(\pm nm \arccos x) = \\
= \cos(nm \arccos x) = T_{nm}(x)
\end{gather}$$
### 5. Доказать, что $T_{n}(2x-1) = T_{2n}(\sqrt{ x })$

$$\begin{gather}
T_{2n}(\sqrt{ x }) = T_{n}(T_{2}(\sqrt{ x })) = T_{n}(2(\sqrt{ x })^{2} - 1) = T_{n}(2x-1)
\end{gather}$$

### 6. Вычислить 

$$\begin{gather}
\int _{-1}^{1} \frac{[xT_{n}(x)]^{2}}{\sqrt{ 1-x^{2} }}\, dx , \ n = 1,2,\dots \\
I = \begin{cases}
\frac{3\pi}{8}, \ n = 1 \\
\frac{\pi}{4}, \ n = 2,3,\dots
\end{cases}
\end{gather}$$

## Многочлены Лагерра

$$\begin{gather}
L_{n}^{\alpha}(x) \frac{1}{n!}(x^{-\alpha})e^{x} \frac{d^{n}}{dx^{n}} [x^{n+\alpha}e^{-x}], \ n=0,1,2, \dots, \ \alpha> -1 \\
\rho(x) = x^{\alpha}e^{-x} \\
\alpha = 0 \implies L_{n}(x) = \frac{1}{n!}e^{x}\frac{d^{n}}{dx^{n}}[x^{n}e^{-x}]
\end{gather}$$

$$\begin{gather}
1. \ \int_{0}^{\infty} x^{\alpha }e^{-x} L_{n}^{\alpha}(x)L_{m}^{\alpha}(x) \, dx = \begin{cases}
0, n \neq m \\
\frac{\Gamma(n+\alpha+1)}{n!}, \ n = m
\end{cases}  \\
2. \ \Psi(x,t) = \frac{1}{(1-t)^{\alpha+1}}e^{-xt/(1-t)}, \ |t| < 1, \ \alpha > -1, \ x > 0 \\
\Psi(x,t) = \sum_{n=1}^{\infty} L_{n}^{\alpha}(x)t^{n} \\
\end{gather}$$

$$\begin{gather}
3. \ (n+1)L_{n+1}^{\alpha}(x) + (x-\alpha-2n-1)L_{n}^{\alpha}(x) + (n+\alpha)L_{n-1}^{\alpha}(x) = 0, \ n = 1,2,\dots
\end{gather}$$

### 1. Найти в явном виде $L_{0}(x), \dots, L_{3}(x)$

$$\begin{gather}
L_{0}(x) = 1 \\
L_{1}(x) = 1-x \\
L_{2}(x) = \dots
\end{gather}$$

$$\begin{gather}
\int_{0}^{+\infty} e^{-x}[xL_{n}(x)]^{2} \, dx, \ n = 0,1,2,\dots
\end{gather}$$