---
tags:
  - seminar
  - 2nd-semester
  - 2025-03-19
---

$$\begin{gather}
\frac{dt}{\cos ^{2}t} = d\tan t \\
\frac{1}{\cos ^{2}t} = 1 + \tan ^{2} t
\end{gather}$$

### 1. Интеграл Дирихле


$$\begin{gather}
\int_{0}^{+\infty} \frac{\sin x}{x}dx = \frac{\pi}{2} \\
\int_{0}^{+\infty} \frac{\sin(xy)}{x} \, dx = \frac{\pi}{2}\mathrm{sgn} \ y
\end{gather}$$

### 2. Интеграл Эйлера-Пуассона

$$\begin{gather}
\int_{0}^{+\infty} e^{-x^{2}} \, dx = \frac{\sqrt{ \pi }}{2} \\
\int_{-\infty}^{+\infty} e^{-x^{2}} \, dx = \sqrt{ \pi } \\
\end{gather}$$

### 1. Вычислить интеграл $\int_{0}^{+\infty} \left( \frac{\sin x}{x} \right)^{2} \, dx$

$$\begin{gather}
I = \int_{0}^{+\infty} \left( \frac{\sin x}{x} \right)^{2} \, dx \\
I(a) = \int_{0}^{+\infty} \frac{\sin^{2}ax}{x^{2}} \, dx \\
I'(a) = 2\int_{0}^{+\infty} \frac{\sin ax \cos ax}{x} \, dx = \int_{0}^{+\infty} \frac{\sin 2ax}{x} \, dx = \frac{\pi}{2} \\
I(a) = \frac{\pi}{2}\int da  = \frac{a\pi}{2} + C \left.=\right|_{a = 1} \frac{\pi}{2} + C \\
I(0) = 0 \implies C = 0 \implies \\
I = \frac{\pi}{2}
\end{gather}$$

### 2

$$\begin{gather}
I = \int_{0}^{+\infty} \frac{\sin x^{2}}{x} \, dx\\
I = \begin{bmatrix}
x^{2} = t \\
dt = 2xdx
dx = \frac{dt}{2x} = \frac{dt}{2\sqrt{ t }}
\end{bmatrix} = \\
= \int_{0}^{+\infty} \frac{\sin t \, dt}{2t} = \frac{1}{2}\int_{0}^{+\infty} \frac{\sin t}{t} \, dx = \frac{1}{2} \cdot \frac{\pi}{2} = \frac{\pi}{4}
\end{gather}$$

### 4

$$\begin{gather}
I = \int_{0}^{+\infty} \frac{\sin x - x\cos x}{x^{3}} \, dx  \\
I(a) = \begin{bmatrix}
\sin x = \sin ax \\
\cos x = \cos ax
\end{bmatrix} = \int_{0}^{+\infty} \frac{\sin ax -ax\cos ax}{x^{3}} \, dx \\
I'(a) = \int_{0}^{+\infty} \frac{x\cos ax - x(\cos ax - \alpha\sin ax)}{x^{3}} \, dx = \\
= \int_{0}^{+\infty} \frac{\alpha x^{2}\sin ax}{x^{3}} \, dx = \\
= \int_{0}^{+\infty} \frac{a \sin ax}{x} \, dx = \frac{a\pi}{2} + C \\
I(0) = 0 \implies C = 0 \\
I(a) = \frac{\pi}{4}\alpha^{2}; \ I(1) = \frac{\pi}{4}
\end{gather}$$

### 6

$$\begin{gather}
\int_{0}^{+\infty} \frac{\sin^{3}\alpha x}{x} \, dx  \\
\left[ \sin 3\phi = 3\sin \phi - 4\sin ^{3}\phi \right]  \\
\sin ^{3} \phi = \frac{3\sin \phi - \sin 3\phi}{4} \\
\end{gather}$$

$$\begin{gather}
I = \frac{1}{4}\int_{0}^{+\infty} \frac{3\sin\alpha x - \sin 3\alpha x}{x}  \, dx = \\
= \frac{1}{4} \left( \frac{3\pi}{2}\mathrm{sgn} \ \alpha - \frac{\pi}{2}\mathrm{sgn} \ \alpha \right) =\frac{\pi}{4} \mathrm{sgn} \ \alpha \\
\end{gather}$$

### 9

$$\begin{gather}
\int_{0}^{+\infty} \frac{\sin x\cos ^{4}x}{x} \, dx = \\
= \dots = \int_{0}^{+\infty} \frac{\sin x (1 + 2\cos 2x + \cos ^{2}2x)}{4x} \, dx = \\
= \dots = \int_{0}^{+\infty} \frac{\sin x (1 + 2\cos 2x + \cos ^{2}2x)}{4x} \, dx = \dots = \\
= 
\end{gather}$$