## 8.4

$$\begin{gather}
\sigma : y^{2} = x^{2}+z^{2} \\
Ц : x^{2}+z^{2}=4x \\
\end{gather}$$

![[ТР 8 Математический анализ 2024-05-30 14.26.25.excalidraw|100%]]

$$\begin{gather}
Ц : (x-2)^{2} +z^{2} = 2^{2} \\
y = \sqrt{ x^{2}-z^{2} } \\
\sigma = \sigma_{1} \cup \sigma_{2} \\
\iint_{\sigma} d\sigma = 2\iint_{\sigma_{1}} d\sigma_{1} = \\ \end{gather}$$

$$\begin{gather}
= 2\iint_{D_{xz}}\sqrt{ 1 + (y'_{x})^{2} + (y'_{z})^{2} } \, dxdz = \\
= 2\iint_{D_{xz}}\sqrt{ 1 + \frac{x^{2}}{x^{2}+z^{2}} + \frac{z^{2}}{x^{2}+z^{2}} } \, dxdz = \\
= 2\iint_{D_{xz}}\sqrt{ 2 } \, dxdz = \\\end{gather}$$

$$\begin{gather}
= 2\sqrt{ 2 }\int_{0}^{4} \, dx \int_{-\sqrt{ 4x-x^{2} }}^{\sqrt{ 4x-x^{2} }} \, dz = 4\sqrt{ 2 }\int_{0}^{4} \sqrt{ 4x-x^{2} } \, dx = \\
= 4\sqrt{ 2 }\int_{0}^{4} \sqrt{ -(x-2)^{2} + 4 } \, dx = \begin{bmatrix}
x-2 = 2\sin t \\
t = \arcsin \frac{x-2}{2} \\
d(x-2) = 2\cos t
\end{bmatrix} = \\\end{gather}$$

$$\begin{gather}
= 16\sqrt{ 2 }\int_{-\pi/2}^{\pi/2} \sqrt{ 1-\sin ^{2}t } \, \cos tdt = 16\sqrt{ 2 }\int_{-\pi/2}^{\pi/2} \cos ^{2}t \, dt = \\
= 4\sqrt{ 2 }\int_{-\pi/2}^{\pi/2} [\cos 2t + 1] \, d(2t) = \\
= 4\sqrt{ 2 }\left.\left[ \sin 2t + 2t \right]\right|_{-\pi/2}^{\pi/2} = 8\sqrt{ 2 }\pi
\end{gather}$$
