---
aliases: 
tags:
  - practice
  - seminar
  - 2nd-semester
---

> Creation time: 14:22

## 1
$$\begin{gather}
a_{n} = \frac{n \sin ^{2} 2n}{\sqrt{ n^{5}+3 }} \leq b_{n} = \frac{n}{^{\frac{5}{2}}}= \frac{1}{n^{\frac{-3}{2}}} - \text{ сходится } \left( \lambda = \frac{3}{2} >1\right)
\end{gather}$$

## 2

$$\begin{gather}
\lim_{ n \to \infty } \frac{a_{n} + 1}{a_{n}}=\lim_{ n \to \infty } \frac{n \ln^{2} n}{(n+1)\ln^{2}(n+1)}
\end{gather}$$

$$\begin{gather}
a_{n} = \frac{\arctan \sqrt{ n+2 }}{n \ln^{2} (n+1)} \\
\frac{\frac{\pi}{3}}{n \ln^{2} (n+1)}\leq a_{n} < \frac{\frac{\pi}{2}}{n \ln^{2} n}=b_{n}, n \geq 2 \\
\lim_{ n \to \infty } \frac{a_{n} +1}{a_{n}}=\lim_{ n \to \infty } \frac{n \ln^{2}n}{(n+1)\ln^{2}(n+1)} \\
\frac{\pi}{2} \int _{2}^{+inf} \, \frac{dx}{x \ln^{2}x} = \\ 
= \frac{\pi}{2}\int _{2}^{+inf} \, \frac{d (\ln x)}{\ln^{2} x} = -\frac{\pi}{2} \frac{1}{\ln x} \left.\begin{array}{\ll}\\\\\end{array}\right|^{+inf}_{2} = \frac{\pi}{2} \cdot  \frac{1}{\ln_{2}} \implies \text{ сх. по инт }  a_{n}
\end{gather}$$

## 4
$$\begin{gather}
\sin \frac{\pi n}{3} : \left\{  0; \frac{\sqrt{ 3 }}{2};   -\frac{\sqrt{ 3 }}{2} \right\}
\end{gather}$$

$$\begin{gather}
a_{n} = \frac{n^{2}+3}{n^{3}\left( 3-2\sin \frac{\pi n}{3} \right)} \\
\frac{n^{2}+3}{n^{3} \cdot (3+\sqrt{ 3 })} < a_{n} < \frac{n^{2}+3}{n^{3}(3-\sqrt{ 3 })}< \frac{n^{2}+3}{n^{3}} \\
\frac{1}{n} - \text{ расх } 
\end{gather}$$

## 7

$$\begin{gather}
a_{n} = n^{5}  \cdot  e^{-\sqrt{ n }} \\
a_{n+1}=(n+1)^{5} \cdot e^{-\sqrt{ n+1 }} \\
\lim_{ n \to \infty } \frac{a_{n+1}}{a_{n}} = \frac{(n+1)^{5} \cdot e^{-\sqrt{ n+1 }}}{n^{5} \cdot e^{-\sqrt{ n }}}=1 \\
f(x) = x^{5} \cdot e^{-\sqrt{ n }} \\
f(x)=5x^{4}e^{-\sqrt{ x }}-e^{\sqrt{ x }} \cdot x^{5} \cdot \frac{1}{2\sqrt{ x }}=x^{4} \cdot e^{-\sqrt{ x }}\left( 5-\frac{x}{2\sqrt{ x }} \right) = \\ 
= x^{4}e^{-\sqrt{ x }}\left( 5- \frac{\sqrt{ x }}{2} \right)
\end{gather}$$

## 9

$$\begin{gather}
a_{n} = (\sqrt{ n^{2} + n }-n)^{n^{2}} \\
\lim_{ n \to \infty } \sqrt[n]{ a_{n} } = \lim_{ n \to \infty } (\sqrt{ n^{2}+n }-n)^{n} \\
= \lim_{ n \to \infty } \left( \frac{n^{2}+n-n^{2}}{\sqrt{ n^{2}+n }+n} \right)^{n} = \lim_{ n \to \infty } \left( \frac{n}{\sqrt{ n^{2}+n }+n} \right)^{n} = \\ 
= \lim_{ n \to \infty } \left( \frac{n}{n\left( \sqrt{ 1+\frac{1}{n} } \right)} \right)^{n}  = \\ 
= \lim_{ n \to \infty } \left( \frac{1}{1+\sqrt{ 1+\frac{1}{n} }} \right)^{n}=\lim_{ n \to \infty } \left( \frac{1}{2} \right)^{n} = \\
= \lim_{ n \to \infty } \frac{1}{2^{n}}=0 < 1 \implies \text{ сх. } 
\end{gather}$$

## 12

$$\begin{gather}
a_{n} = \frac{(2n+2)!}{\pi^{n} \cdot (n!)^{2}}; \\
\lim_{ n \to \infty } \frac{a_{n+1}}{a_{n}} = \lim_{ n \to \infty } \frac{(2n+3)(2n+4)}{\pi(n+1)^{2}}=\frac{4}{\pi} > 1 \implies \text{ расходится } 
\end{gather}$$

## 15

$$\begin{gather}
a_{n} = \frac{(2n)!!}{n!}\arcsin \frac{1}{3^{n}} \sim b_{n} = \frac{(2n)!!}{n!3^{n}} \\
\lim_{ n \to \infty }  \frac{(2n+2)!! n! 3^{n}}{n!(n+1) \cdot 3^{n} \cdot 3 (2n)!!} = \\ 
= \frac{2}{3} < 1 \implies \text{ сходится } 
\end{gather}$$

## 16

$$\begin{gather}
a_{n} = \left( n \arcsin \frac{1}{n} \right)^{n^{3}} \\
1) \text{ По Коши } \lim_{ n \to \infty } \sqrt[n]{ \left( n \arcsin \frac{1}{n} \right)^{n^{3}} } = \\ 
= \lim_{ n \to \infty } \sqrt[n]{ a_{n} } = \lim_{ n \to \infty } \left( n \arcsin \frac{1}{n} \right)^{n^{2}} \\
\end{gather}$$

Разложим по формуле Тейлора

$f(x)=\arcsin x$
$\underbrace{ f(x) }_{ (x\to0) }=f(0)+ \frac{f'(0)}{1!}x+ \frac{f''(0)}{2!}x^{2}+ \frac{f'''(0)}{3!}x^{3} + o(x^{3})$


