---
tags:
  - seminar
  - 2nd-semester
  - 2024-10-30
---

## 1

$$\begin{gather}
(x^{2}+x)y' = (2x+1)y \\
\ln |y| = \ln |x^{2} + x| + \ln |C| \\
y = C(x^{2}+x), \ C = 1\\
y = x^{2} + x
\end{gather}$$

## 2.4

$$\begin{gather}
yy'' - (y')^{2} = 0, \ y(0) = 1, \ y'(0) = 2 \\
\frac{yy''-(y')^{2}}{(y')^{2}} = 0 \\
-\left( \frac{y}{y'} \right)' = 0 \\
\left( \frac{y}{y'} \right)' = 0 \\
\frac{y}{y'} = C_{1} \\
C_{1} = \frac{y(0)}{y'(0)} = \frac{1}{2} \\
\frac{y}{y'} = \frac{1}{2} \\
\frac{y'}{y} = 2 \\
\ln |y| = 2x+ \ln |C_{2}| \\
y = C_{2}e^{2x} \\
1 = C_{2} e^{2\cdot 0} \\
C_{2} = 1 \\
y = e^{2x} \\
\end{gather}$$

## 3.4

$$\begin{gather}
y^{2}y'' + y'^{3} = 0 \\
\begin{bmatrix}
y' = z(y) \\
y'' = z'(y)
\end{bmatrix}\\
\end{gather}$$

## 3.5

$$\begin{gather}
y(y''+y') = y'^{2}(xy^{2}-1) \\
yy'' + y'^{2} = x(yy'')^{2} - yy' \\
(yy')' = x(yy')^{2} - yy' \\
z = yy' \\
z' = xz^{2} - z - \text{бернули} \\
\end{gather}$$

## 4.5

$$\begin{gather}
(y + 2)y'' + (y')^{2} = \cos 2x \\
((y+2)y')' = \left( \frac{\sin 2x}{2} \right) \\
\end{gather}$$

## Линейные уравнения с переменными коэффициентами

### 686

Ищем частное решение в виде многочлена:

$$\begin{gather}
x(x-1)y'' - xy' + y = 0 \\
y_{1} = x^{n} + a_{1}x^{n-1} + a_{2}x^{n-2} + \dots + a_{n} \\
y_{1}' = nx^{n-1} + a_{2}(n-1)x^{n-2} + \dots + a_{n-1} \\
y_{1}'' = n(n-1)x^{n-2} + a_{2}(n-1)(n-2)x^{n-3} + \dots + a_{n-2} \\
n(n-1) - n + n = 0 \\
n(n-1) = 0 \\
n = 0; n = 1 \\
-a_{2}(n-1)(n-2) -a_{2}(n-1) + a_{1}
\end{gather}$$