---
tags:
  - seminar
  - 2nd-semester
  - 2024-10-16
---
## 457

$$\begin{gather}
yy'' = y'(y'+1) \\
\begin{bmatrix}
y' = z(y) \\
y'' = y'z' = z'z
\end{bmatrix} \\
yz'z = z(z+1), \ (z = 0 !) \\
yz' = z+1 \\
y = \frac{z+1}{z'} \\
\frac{1}{y} = \frac{z'}{z+1} \\
\ln |y| = \ln |z+1| + \ln |C_{1}| \\ 
z+1 =  \ln |C_{1}y| \\
y' = C_{1}y - 1 \\
\frac{yy''}{(y'+1)y} = \frac{y'(y'+1)}{(y'+1)y} \\
\frac{y''}{(y'+1)} = \frac{y'}{y} \\
\ln |y'+1| = \ln |y| + \ln |C_{1}| \\
y'+1 = C_{1}y \\
y' = C_{1}y - 1 \\
\frac{y'}{C_{1}y - 1} = 1 \\
\frac{1}{C_{1}} \cdot \frac{C_{1}y'}{C_{1}y - 1} = 1 \\
\frac{1}{C_{1}} \ln |C_{1}y - 1| = x + \frac{\ln C_{2}}{C_{1}} \\
\end{gather}$$

$$\begin{gather}
\ln (C_{1}y-1) = C_{1}x + \ln C_{2} \\
C_{1}y - 1 = C_{2}e^{C_{1}x} \\
y = \frac{C_{2}e^{C_{1}x} + 1}{C_{1}}, \ y = 0, \ y = -x+C \\
\end{gather}$$

## 428

$$\begin{gather}
y''' = y''^{2} \\
\begin{bmatrix}
y'' = z(x) \\
y''' = z' \\
\end{bmatrix} \\
z' = z^{2} \\
\frac{z'}{z^{2}} = 1 \\
-\frac{1}{z} = x + C_{1} \\
-\frac{1}{y''} = x + C_{1} \\
y'' = -\frac{1}{x + C_{1}} \\
y' = \int \frac{dx}{x+C_{1}} \\
y' = \ln (x + C_{1}) + C_{2} \\
y = \int \left( \ln (x+C_{1}) + C_{2} \right)  \, dx  \\
y = C_{2}x - (x+C_{1})\ln (x+C_{1}) - x - C_{1}  + C_{3} \\
\dots
\end{gather}$$

## 448

$$\begin{gather}
y'''y'^{2} = y''^{3} \\
\frac{y'''}{y''} = \frac{y''^{2}}{y'^{2}} \\
\frac{y'''}{y''} = \left(\frac{y''}{y'}\right)^{2} \\
\begin{bmatrix}
y' = z \\
y'' = z' \\
y''' = z''
\end{bmatrix} \\
z''z^{2} = z'^{3} \\
\begin{bmatrix}
z' = p(z) \\
z'' = p'z' = p'p
\end{bmatrix} \\
p'pz^{2} = p^{3}, \ p = 0 \implies y' = C \implies y = Cx + \tilde{C}\\
p'z^{2} = p^{2} \\
\frac{p'}{p^{2}} = \frac{1}{z^{2}} \\
\frac{1}{p} = \frac{1}{z} + C_{1} \\
p = \frac{z}{1 + C_{1}z} \\
z' = \frac{z}{1+C_{1}z} \\
\end{gather}$$

$$\begin{gather}
\frac{z'(1+C_{1}z)}{z} = 1 \\
\ln |z| + C_{1}z = x + C^{2} \\
\ln |y'| + C_{1}y' = x + C^{2} \\
\ln |t| + C_{1}t = z + C^{2}
\end{gather}$$