---
tags:
  - seminar
  - 2nd-semester
  - 2024-09-25
---

## Уравнение в полных дифференциалах

### 193

$$\begin{gather}
3x^{2}(1+\ln y)dx = \left( 2y-\frac{x^{3}}{y} \right) dy \\
(3x^{2}(1+\ln y))'_{y} = \frac{3x^{2}}{y} \\
-\left( 2y-\frac{x^{3}}{y} \right)'_{x} = \frac{3x^{2}}{y} \\
\text{след.} \ \exists F(x,y) \\
dF = \frac{\partial F}{\partial x}dx + \frac{\partial F}{\partial y} dy \\
\frac{\partial F}{\partial x} = 3x^{2}(1+\ln y), \ \frac{\partial F}{\partial y} = -\left( 2y - \frac{x^{3}}{y} \right) \\
F = \int \frac{\partial F}{\partial x} \, dx = 3(1+\ln y)\int x^{2} \, dx = x^{3}(1+\ln y) + \phi(y) \\
F'_{y} = \frac{x^{3}}{y}-2y \\
\frac{x^{3}}{y} + \phi'(y) = -2y + \frac{x^{3}}{y} \\
\phi'(y) = -2y \\
\phi(y) = -y^{2} \\
F(x,y): x^{3}(1+\ln y) -y^{2} = C
\end{gather}$$

### 189

$$\begin{gather}
\frac{y}{x}dx + (y^{3}+\ln x)dy = 0 \\
\left( \frac{y}{x} \right)'_{y} = \frac{1}{x} \\
(y^{3}+\ln x)'_{x} = \frac{1}{x} \\

\end{gather}$$