---
tags:
  - seminar
  - 2nd-semester
  - 2024-09-18
---

## 136

$$\begin{gather}
xy' - 2y = 2x^{4} \\
y' - \frac{2y}{x} = 2x^{3} \\
\begin{bmatrix}
y = uv \\
y' = u'v + uv'
\end{bmatrix} \\
u'v + uv' - \frac{2uv}{x} = 2x^{3} \\
u'v + u\left(  v' - \frac{2v}{x} \right) = 2x^{3} \\
v' - \frac{2v}{x} = 0 \\
\frac{v'}{v} = \frac{2}{x} \\
\ln |v| = 2\ln |x| + \ln |C| \\
v = Cx^{2} \\
C'x^{2} = 2x^{3} \\
C' = 2x \\
C = x^{2} + \tilde{C} \\
y = x^{4} + \tilde{C}x^{2}
\end{gather}$$

## 147

$$\begin{gather}
(\sin ^{2}y + x\cot y)y' = 1 \\
\sin ^{2}y + x\cot y = \frac{1}{y'} \\
\sin ^{2}y + x\cot y = x' \\
x = uv \\
x = u'v+uv' \\
\sin ^{2}y + uv\cot y = u'v+uv' \\
u'v+uv' - uv\cot y - \sin ^{2}y = 0 \\
u'v+u(v' - v\cot y) - \sin ^{2}y = 0 \\
v' - v\cot y = 0 \\
\ln |v| = \int \cot y \, dy \\
\ln |v| = \int \frac{\cos x}{\sin x} \, dy \\
\ln |v| = \ln |\sin x| + \ln |C| \\
v = \sin y \\
u'\sin y - \sin ^{2} y = 0 \\
u' - \sin y = 0 \\
u' = \sin y \\
u = -\cos y + C \\
x = uv = (-\cos y + C)\sin y \\
x = -\frac{1}{2} \sin 2y + C\sin y
\end{gather}$$

## 151

$$\begin{gather}
y' + 2y = y^{2}e^{x} \\
y' = a(x)y +b(x)y^{\alpha}, \ a\neq 0, \alpha\neq 1 \\
y = uv \\
y' = u'v + uv' \\
u'v + uv' + 2uv -2u^{2}v^{2} e^{x} = 0 \\
u'v + u(v' + 2v) - 2y^{2}v^{2}e^{x} = 0 \\
\frac{v'}{v} = -2 \\
\ln |v| = -2x \\ 
v = e^{-2x} \\
u'e^{-2x} - 2u^{2}v^{2}e^{x} = 0
\end{gather}$$